src/goose_lang/lib/channel/chan_spec_multi_base.v
@@ -1,0 +1,3618 @@
+From Perennial.goose_lang Require Import prelude. 
+From Perennial.goose_lang Require Import notation typing.
+From Perennial.goose_lang Require Import proofmode wpc_proofmode array.
+From Perennial.program_proof Require Import proof_prelude.
+From Perennial.program_proof Require Import std_proof.
+From Perennial.goose_lang.automation Require Import extra_tactics.
+From Perennial.goose_lang.lib Require Import
+      persistent_readonly slice slice.typed_slice struct loop lock control map.typed_map time proph rand string typed_mem.
+
+From Perennial.goose_lang.lib.channel Require Import auth_set.
+From Perennial.goose_lang.lib.channel Require Import chan_use_ctr.
+From Goose.github_com.goose_lang.goose Require Import channel.
+From Perennial.goose_lang Require Import lang typing.
+
+
+Section proof.
+Context `{ffi_sem: ffi_semantics} `{!ffi_interp ffi}.
+Context `{hG: heapGS Σ, !ffi_semantics _ _, !ext_types _}. 
+Context `{!closePropTrackerG Σ, !inG Σ (authR (optionUR (prodR fracR natR)))}.
+Context `{!ghost_varG Σ (bool * val)}.
+
+Implicit Types (v:val).
+
+(* Define valid states as an inductive type *)
+Inductive valid_chan_state := 
+  | Valid_start
+  | Valid_receiver_ready
+  | Valid_sender_ready
+  | Valid_receiver_done
+  | Valid_sender_done
+  | Valid_closed.
+
+
+(* Define equality comparison for valid_chan_state *)
+Definition valid_chan_state_eq (vs1 vs2: valid_chan_state) : bool :=
+  match vs1, vs2 with
+  | Valid_start, Valid_start => true
+  | Valid_receiver_ready, Valid_receiver_ready => true
+  | Valid_sender_ready, Valid_sender_ready => true
+  | Valid_receiver_done, Valid_receiver_done => true
+  | Valid_sender_done, Valid_sender_done => true
+  | Valid_closed, Valid_closed => true
+  | _, _ => false
+  end.
+
+(* Notation for equality *)
+Notation "vs1 =?= vs2" := (valid_chan_state_eq vs1 vs2) (at level 70).
+
+
+(* Define word constants to match Go implementation *)
+Definition CS_START_W : w64 := W64 0.
+Definition CS_RECEIVER_READY_W : w64 := W64 1.
+Definition CS_SENDER_READY_W : w64 := W64 2.
+Definition CS_RECEIVER_DONE_W : w64 := W64 3.
+Definition CS_SENDER_DONE_W : w64 := W64 4.
+Definition CS_CLOSED_W : w64 := W64 5.
+
+(* Conversion function from valid state to word representation *)
+Definition valid_to_word (vs: valid_chan_state) : w64 := 
+  match vs with
+    | Valid_start => CS_START_W
+    | Valid_receiver_ready => CS_RECEIVER_READY_W
+    | Valid_sender_ready => CS_SENDER_READY_W
+    | Valid_receiver_done => CS_RECEIVER_DONE_W
+    | Valid_sender_done => CS_SENDER_DONE_W
+    | Valid_closed => CS_CLOSED_W
+  end.
+
+(* Helper function to check if a word corresponds to a valid channel state *)
+Definition is_valid_cs_word (w: w64) : bool :=
+  match word.unsigned w with
+  | 0 | 1 | 2 | 3 | 4 | 5 => true
+  | _ => false
+  end.
+
+(* Helper lemma for valid states *)
+Lemma valid_states_eq_dec : forall (vs1 vs2 : valid_chan_state),
+  {vs1 = vs2} + {vs1 ≠ vs2}.
+Proof.
+  decide equality.
+Qed.
+
+(* Helper functions for state properties *)
+Definition send_ctr_frozen (vs: valid_chan_state): bool :=
+  match vs with 
+    | Valid_closed => true
+    | _ => false
+  end.
+
+Definition recv_ctr_frozen (vs: valid_chan_state) (send_count recv_count: nat): bool :=
+  match vs with
+    | Valid_closed => (send_count =? recv_count)
+    | _ => false
+  end.
+
+Definition full_exchange_token (γ: chan_names): iProp Σ :=
+  ghost_var γ.(unbuffered_state_tracker_name) 1%Qp (true, #()).
+
+Definition exchange_token (γ: chan_names) (sender_initiated: bool) (v: val): iProp Σ :=
+  ghost_var γ.(unbuffered_state_tracker_name) (1/2)%Qp (sender_initiated, v).
+
+(* Half token for sender - contains both flag and value *)
+Definition sender_exchange_token (γ: chan_names) (v: val): iProp Σ :=
+exchange_token γ true v.
+
+(* Half token for receiver - contains only flag *)
+Definition receiver_exchange_token (γ: chan_names): iProp Σ :=
+∃ dummy_v, 
+exchange_token γ false dummy_v.
+
+  Lemma exchange_token_combine γ:
+  ∀ sender_initiated sender_initiated' v v',
+  exchange_token γ sender_initiated v ∗
+  exchange_token γ sender_initiated' v' ==∗
+  full_exchange_token γ.
+Proof.
+  unfold exchange_token, full_exchange_token.
+  iIntros (sender_initated). iIntros (sender_initiated').
+  iIntros (v v').
+  iIntros "[Htok1 Htok2]".
+  iCombine "Htok1 Htok2" as "Htok" gives "%Hvalid".
+  iApply (ghost_var_update (true, #()) with "Htok").
+Qed.
+
+Lemma exchange_token_agree(γ : chan_names) (sender_initiated sender_initiated' : bool) (v v' : val) :
+exchange_token γ sender_initiated v  -∗  exchange_token γ sender_initiated' v' -∗ ⌜ v = v' ∧ sender_initiated = sender_initiated' ⌝ .
+iIntros "H1". iIntros "H2".
+iDestruct (ghost_var_agree with "[$H1] [$H2]") as "%H". iPureIntro. injection H.
+intros H1. intros H2. done.
+Qed.
+
+Lemma exchange_token_split γ sender_initiated v:
+  full_exchange_token γ ==∗
+  exchange_token γ sender_initiated v ∗
+  exchange_token γ sender_initiated v.
+Proof.
+  unfold full_exchange_token, exchange_token.
+  iIntros "Htok".
+  iMod (ghost_var_update (sender_initiated, v) with "Htok") as "Htok".
+  iDestruct "Htok" as "[Htok1 Htok2]".
+  iModIntro. iFrame.
+Qed.
+
+
+Lemma sender_exchange_token_split γ v:
+  full_exchange_token γ ==∗
+  sender_exchange_token γ v ∗
+  sender_exchange_token γ v.
+Proof.
+  unfold  sender_exchange_token. apply exchange_token_split.
+Qed.
+
+(* Receiver token split lemma *)
+Lemma receiver_exchange_token_split γ:
+  full_exchange_token γ ==∗
+  receiver_exchange_token γ ∗
+  receiver_exchange_token γ.
+Proof.
+  unfold receiver_exchange_token, full_exchange_token.
+  iIntros "Htok".
+  iMod (ghost_var_update (false, #()) with "Htok") as "[Htok1 Htok2]".
+  iFrame. done.
+Qed.
+
+(* Combine sender tokens *)
+Lemma sender_exchange_token_combine γ v v':
+  sender_exchange_token γ v ∗ sender_exchange_token γ v' ==∗
+  full_exchange_token γ.
+Proof.
+  unfold sender_exchange_token.
+  iIntros "[Htok1 Htok2]".
+  iApply (exchange_token_combine γ true true v v' with "[Htok1 Htok2]").
+  iFrame.
+Qed.
+
+(* Combine receiver tokens *)
+Lemma receiver_exchange_token_combine γ:
+  receiver_exchange_token γ ∗ receiver_exchange_token γ ==∗
+  full_exchange_token γ.
+Proof.
+  unfold receiver_exchange_token.
+  iIntros "[Htok1 Htok2]".
+  iDestruct "Htok1" as (dummy_v1) "Htok1".
+  iDestruct "Htok2" as (dummy_v2) "Htok2".
+  iApply (exchange_token_combine γ false false dummy_v1 dummy_v2 with "[Htok1 Htok2]").
+  iFrame.
+Qed.
+
+(* Sender token agreement - useful for verification *)
+Lemma sender_exchange_token_agree γ v v':
+  sender_exchange_token γ v -∗ sender_exchange_token γ v' -∗ ⌜v = v'⌝.
+Proof.
+  unfold sender_exchange_token.
+  iIntros "Htok1 Htok2".
+  iDestruct (exchange_token_agree γ true true v v' with "[$Htok1] [$Htok2]") as "(%Hv & _)".
+  iPureIntro. exact Hv.
+Qed.
+
+Definition P (is_single_party: bool) (i:Z)
+ (v: val) (Psingle: (Z -> val -> iProp Σ)) (Pmulti: (val -> iProp Σ)): iProp Σ :=
+ if is_single_party then Psingle i v else Pmulti v.
+
+Definition Q (is_single_party: bool) (z: Z) (Qsingle: (Z -> iProp Σ)) (Qmulti: iProp Σ): iProp Σ := 
+if bool_decide(Z.lt z 0%Z) then True%I else (if is_single_party then Qsingle(z) else Qmulti).
+
+(* Core representation of channel state - pure facts *)
+Definition chan_state_facts (vs: valid_chan_state) (send_count recv_count: nat) (v: val) (chan_type: ty): iProp Σ :=
+  match vs with
+    | Valid_start => ⌜send_count = recv_count⌝
+    | Valid_receiver_ready => ⌜send_count = recv_count⌝
+    | Valid_sender_ready => (⌜send_count = recv_count⌝ ∗ ⌜val_ty v chan_type⌝)
+    | Valid_receiver_done => ⌜recv_count = S send_count⌝ 
+    | Valid_sender_done => (⌜send_count = S recv_count⌝ ∗ ⌜val_ty v chan_type⌝)
+    | Valid_closed => ⌜send_count = recv_count⌝
+  end.
+
+  Definition chan_state_resources (vs: valid_chan_state) (γ: chan_names) (is_single_party: bool)
+  (send_count recv_count: nat) (v: val)
+  (Psingle: Z -> val -> iProp Σ) (Pmulti: val -> iProp Σ)
+  (Qsingle: Z -> iProp Σ) (Qmulti: iProp Σ): iProp Σ :=
+match vs with
+| Valid_start => 
+full_exchange_token γ (* Full token with default value *)
+| Valid_receiver_ready => 
+receiver_exchange_token γ ∗ (* Receiver initiated *)
+Q is_single_party recv_count Qsingle Qmulti
+| Valid_sender_ready => 
+sender_exchange_token γ v ∗ (* Sender initiated *)
+P is_single_party send_count v Psingle Pmulti
+| Valid_receiver_done => 
+sender_exchange_token γ v ∗ (* Receiver will complete *)
+Q is_single_party send_count Qsingle Qmulti
+| Valid_sender_done => 
+receiver_exchange_token γ ∗  (* Sender will complete *)
+P is_single_party recv_count v Psingle Pmulti  
+| Valid_closed => emp
+end.
+
+
+Definition big_sep_seq (start: Z) (size: Z) (Φ : Z → iProp Σ) : iProp Σ :=
+⌜ 0 ≤ size ⌝ ∗ 
+[∗ list] _↦(i:Z) ∈ (seqZ start size), Φ i
+.
+Lemma big_sep_seq_singleton  (Φ : Z → iProp Σ) :
+  ∀ (start: Z),
+  big_sep_seq start 1 Φ  ⊣⊢  (Φ (start)%Z ).
+  Proof.
+    intros Hsize. unfold big_sep_seq.
+    simpl. replace (0%nat + Hsize)%Z with Hsize by lia.
+    {
+      iSplitL "".
+      { iIntros "(%Hsize2 & H &  emp)". done. }
+      { iIntros "H". iFrame. iPureIntro. done. }
+    }
+  Qed.
+
+Lemma big_sep_seq_nil :
+  ∀ start Φ,
+  big_sep_seq start 0 Φ ⊣⊢ emp.
+  Proof.
+     intros start. intros. unfold big_sep_seq.
+     simpl. iFrame. done.
+  Qed.
+  
+Lemma big_sep_seq_snoc (start: Z) (size: Z)   (Φ : Z → iProp Σ) :
+  (0 ≤ size)%Z ->
+  Φ (start + size)%Z ∗ big_sep_seq start size Φ  -∗ big_sep_seq start (size + 1)%Z Φ.
+  Proof.
+    intros H. iIntros "(Hpred & %Hsize & Hsep)".
+    unfold big_sep_seq. 
+    rewrite seqZ_app.
+    {
+      rewrite big_sepL_snoc.
+      iFrame. iPureIntro. lia.
+    }
+    {
+     lia. 
+    }
+    {
+      done. 
+    }
+  Qed.
+
+  Lemma big_sep_seq_cons (start: Z) (size: Z)   (Φ : Z → iProp Σ) :
+  (0 ≤ size)%Z ->
+  big_sep_seq start (size + 1)%Z Φ -∗ Φ (start + size)%Z ∗ big_sep_seq start size Φ.
+  Proof.
+    intros H. iIntros "(%Hsize & Hpred)".
+    unfold big_sep_seq. 
+    rewrite seqZ_app.
+    {
+
+      rewrite big_sepL_app.
+      rewrite big_sepL_singleton.
+
+       simpl.
+       replace (0%nat + (start + size))%Z with (start + size)%Z by lia.
+       iDestruct "Hpred" as "[Hlist Hpred]". iFrame.
+       iPureIntro. lia.
+
+    }
+    {
+     lia. 
+    }
+    {
+      done. 
+    }
+  Qed.
+
+  Lemma big_sep_seq_pop (start: Z) (size: Z)   (Φ : Z → iProp Σ) :
+  1 ≤ size ->
+  big_sep_seq start size%Z Φ -∗ Φ (start)%Z ∗ big_sep_seq (start + 1) (size - 1) Φ.
+  Proof.
+    intros H. iIntros "(%Hsize & Hpred)".
+    unfold big_sep_seq. 
+    rewrite seqZ_cons.
+    {
+
+      rewrite big_sepL_cons.
+      iDestruct "Hpred" as "[Hs Hl]". iFrame. iPureIntro. lia.
+    }
+    {
+      lia.
+    }
+   
+  Qed.
+
+
+  Definition buff_size_inv (count : Z) (first : u64) (size : Z): iProp Σ :=
+  (⌜count <= size⌝ ∗ ⌜word.unsigned first < size⌝ ∗ ⌜size > 0⌝ ∗ ⌜size + 1 < 2 ^ 63⌝
+  ∗ ⌜count + 1 < 2 ^ 63⌝)%I.
+
+Definition valid_elems (slice : list val) (first : u64) (count : u64) : list val :=
+  subslice (uint.nat first) (uint.nat first + uint.nat count) (slice ++ slice).
+
+
+  Lemma add_one_lemma_1 : forall slice (first : u64) (count : u64) (e : val) ,
+  uint.Z (length slice) ≠ 0 ->
+  length slice + 1 < 2 ^ 63 ->
+  uint.Z first < length slice ->
+  uint.Z count < length slice ->
+  subslice (uint.nat first) (uint.nat first + uint.nat count)
+  (<[Z.to_nat (uint.Z (word.add first count) `mod` length slice):=e]>
+     slice ++
+   <[Z.to_nat (uint.Z (word.add first count) `mod` length slice):=e]>
+     slice) = subslice (uint.nat first) (uint.nat first + uint.nat count) (slice ++ slice).
+Proof.
+  intuition.
+  assert (uint.nat first + uint.nat count < length slice ∨ (length slice <= uint.nat first + uint.nat count < length slice + length slice)).
+  { word. }
+  destruct H3.
+  - replace (Z.to_nat(uint.Z (word.add first count) `mod` length slice)) with (uint.nat(uint.nat first + uint.nat count)).
+    + rewrite subslice_take_drop.
+      rewrite subslice_take_drop.
+      rewrite take_app_le.
+      2: { rewrite length_insert. word. }
+      rewrite take_app_le.
+      2: { word. }
+      (* Check take_insert. *)
+      rewrite take_insert.
+      { done. }
+      word.
+    + rewrite Z.mod_small; word.
+  - replace (Z.to_nat(uint.Z (word.add first count) `mod` length slice)) with (uint.nat(uint.nat first + uint.nat count - length slice)).
+    + epose proof (subslice_split_r (uint.nat first) (length slice) _ (_ ++ _)).
+      rewrite H4.
+      2: word.
+      2: { rewrite length_app. rewrite length_insert. word. }
+      epose proof (subslice_split_r (uint.nat first) (length slice) _ (slice ++ slice)).
+      rewrite H5.
+      2: word.
+      2: { rewrite length_app. word. }
+      assert (subslice (uint.nat first) (length slice)
+      (<[uint.nat
+           (uint.nat first + uint.nat count -
+            length slice):=e]> slice ++
+       <[uint.nat
+           (uint.nat first + uint.nat count -
+            length slice):=e]> slice) = subslice (uint.nat first) (length slice)
+            (slice ++ slice)).
+        {
+          rewrite <- subslice_before_app_eq.
+          2: { rewrite length_insert. word. }
+          rewrite <- subslice_before_app_eq.
+          2: word.
+          rewrite subslice_take_drop.
+          rewrite subslice_take_drop.
+          epose proof (length_insert slice (uint.nat (uint.nat first + uint.nat count - length slice)) e).
+          rewrite firstn_all.
+          replace ((take (length slice)
+          (<[uint.nat
+               (uint.nat first + uint.nat count -
+                length slice):=e]> slice))) with (take (length (<[uint.nat
+                (uint.nat first + uint.nat count -
+                 length slice):=e]> slice))
+                (<[uint.nat
+                     (uint.nat first + uint.nat count -
+                      length slice):=e]> slice)).
+          2: { rewrite H6. eauto. }
+          rewrite firstn_all.
+          rewrite drop_insert_gt. 
+          {done. }
+          word.
+        }
+      rewrite H6.
+      rewrite app_inv_head_iff.
+      rewrite subslice_comm.
+      rewrite subslice_comm.
+      rewrite drop_app_length.
+      epose proof (length_insert slice (uint.nat (uint.nat first + uint.nat count - length slice)) e).
+      replace ((drop (length slice)
+                (<[uint.nat (uint.nat first + uint.nat count - length slice):=e]> slice ++
+                <[uint.nat (uint.nat first + uint.nat count - length slice):=e]> slice))) with (drop (length (<[uint.nat
+                (uint.nat first + uint.nat count -
+                 length slice):=e]> slice))
+                 (<[uint.nat (uint.nat first + uint.nat count - length slice):=e]> slice ++
+                 <[uint.nat (uint.nat first + uint.nat count - length slice):=e]> slice)).
+      2: { rewrite H7. eauto. }
+      rewrite drop_app_length.
+      rewrite take_insert.
+      { eauto. }
+      word.
+    + (* NOTE: would be cool if [word] could handle this style of reasoning. *)
+      rewrite -(Z_mod_plus_full _ (-1)).
+      rewrite Z.mod_small; word.
+  Unshelve.
+  { 
+  exact val. }
+  { exact (uint.nat first + uint.nat count)%nat. }
+  { exact (<[uint.nat
+  (uint.nat first + uint.nat count - length slice)%Z:=e]>
+slice). }
+  { exact (<[uint.nat
+  (uint.nat first + uint.nat count - length slice)%Z:=e]>
+slice). }
+  exact (uint.nat first + uint.nat count)%nat.
+Qed.
+
+Lemma add_one_lemma_2 : forall slice (first : u64) (count : u64) (e : val),
+  uint.Z (length slice) ≠ 0 ->
+  length slice + 1 < 2 ^ 63 ->
+  uint.Z first < length slice ->
+  uint.Z count < length slice ->
+  subslice (uint.nat first + uint.nat count) (uint.nat first + Z.to_nat(uint.Z count + 1))
+  (<[Z.to_nat (uint.Z (word.add first count) `mod` length slice):=e]>
+     slice ++
+   <[Z.to_nat (uint.Z (word.add first count) `mod` length slice):=e]>
+     slice) = [e].
+Proof.
+  intuition.
+  assert (uint.nat first + uint.nat count < length slice ∨ (length slice <= uint.nat first + uint.nat count < length slice + length slice)).
+  { word. }
+  destruct H3.
+  - replace (Z.to_nat(uint.Z (word.add first count) `mod` length slice)) with (uint.nat(uint.nat first + uint.nat count)).
+    + rewrite subslice_comm.
+      rewrite drop_app_le.
+      2: { rewrite length_insert. word. }
+      rewrite drop_insert_le.
+      2: { word. }
+      assert ((uint.nat (uint.nat first + uint.nat count)%Z -
+      (uint.nat first + uint.nat count))%nat = uint.nat 0).
+      { word. }
+      rewrite H4.
+      match goal with
+        | |- context [take ?n _] => replace n with 1%nat
+      end.
+      { rewrite insert_take_drop.
+        { rewrite take_0.
+          rewrite app_nil_l.
+          rewrite firstn_cons.
+          rewrite take_0.
+          done.
+        }
+        rewrite length_drop.
+        word.
+      }
+      word.
+    + (* NOTE: would be cool if [word] could handle this style of reasoning. *)
+      rewrite Z.mod_small; word.
+  - replace (Z.to_nat(uint.Z (word.add first count) `mod` length slice)) with (uint.nat(uint.nat first + uint.nat count - length slice)).
+    + rewrite subslice_comm.
+      rewrite drop_app_ge.
+      2: { rewrite length_insert. word. }
+      rewrite length_insert.
+      rewrite drop_insert_le.
+      2: { word. }
+      assert ((uint.nat (uint.nat first + uint.nat count - length slice)%Z -
+      (uint.nat first + uint.nat count - length slice))%nat = uint.nat 0).
+      { word. }
+      rewrite H4.
+      match goal with
+        | |- context [take ?n _] => replace n with 1%nat
+      end.
+      { rewrite insert_take_drop.
+        { rewrite take_0.
+          rewrite app_nil_l.
+          rewrite firstn_cons.
+          rewrite take_0.
+          done.
+        }
+        rewrite length_drop.
+        word.
+      }
+      word.
+    + (* NOTE: would be cool if [word] could handle this style of reasoning. *)
+      rewrite -(Z_mod_plus_full _ (-1)).
+      rewrite Z.mod_small; word.
+Qed.
+
+Theorem add_one : forall slice (first : u64) (count : u64) e, 
+  uint.Z (length slice) ≠ 0 ->
+  length slice + 1 < 2 ^ 63 ->
+  uint.Z first < length slice ->
+  uint.Z count < length slice ->
+  valid_elems (<[uint.nat (word.modu ((word.add) first count) (length slice)):= e]> slice) first (word.add count 1) 
+  = valid_elems slice first count ++ [e].
+Proof.
+  intuition.
+  unfold valid_elems.
+  (* NOTE: needs to carefully do what the old [word_cleanup] would do, so that
+  the statements of [add_one_lemma_1] and [add_one_lemma_2] apply. *)
+  rewrite -> ?word.unsigned_add, ?word.unsigned_sub,
+    ?word.unsigned_modu_nowrap, ?word.unsigned_of_Z; [ | word .. ].
+  rewrite -> !wrap_small by word.
+  replace (uint.Z (W64 (length _))) with (Z.of_nat (length slice)) by word.
+  rewrite (subslice_split_r (uint.nat first) (uint.nat first + uint.nat count) _ (_ ++ _)).
+  - rewrite add_one_lemma_1; eauto.
+    rewrite app_inv_head_iff.
+    apply add_one_lemma_2; eauto.
+  - word.
+  - rewrite length_app.
+    rewrite length_insert.
+    word.
+Qed.
+
+Lemma remove_one_lemma_1 : forall slice (first : u64) (e : val),
+  uint.Z (length slice) ≠ 0 ->
+  length slice + 1 < 2 ^ 63 ->
+  uint.Z first < length slice ->
+  slice !! uint.nat first = Some e -> 
+  subslice (uint.nat first) (uint.nat first + 1) (slice ++ slice) = [e].
+Proof.
+  intuition.
+  rewrite subslice_comm.
+  match goal with
+    | |- context [take ?n _] => replace n with 1%nat
+  end.
+  2: { word. }
+  rewrite drop_app_le.
+  2: word.
+  rewrite <- (take_drop_middle (slice) (uint.nat first) e).
+  2: eauto.
+  rewrite drop_app_length'.
+  2: { rewrite length_take. word. }
+  rewrite firstn_cons.
+  rewrite take_0.
+  done.
+Qed.
+
+Lemma remove_one_lemma_2 : forall (slice : list val) (first : u64) (count : u64) (e : val),
+  uint.Z (length slice) ≠ 0 ->
+  length slice + 1 < 2 ^ 63 ->
+  uint.Z first < length slice ->
+  0 < uint.Z count <= length slice ->
+  subslice (uint.nat first + 1) (uint.nat first + uint.nat count) (slice ++ slice) = 
+  subslice (Z.to_nat
+  (uint.Z (word.add first 1)
+    `mod` length slice))
+  (Z.to_nat
+    (uint.Z (word.add first 1)
+    `mod` length slice) + Z.to_nat (uint.Z count - 1)) (slice ++ slice).
+Proof.
+  intuition.
+  assert (uint.Z first < length slice - 1 ∨ uint.Z first = length slice - 1).
+  { word. }
+  destruct H2.
+  - rewrite Z.mod_small. 2: word.
+    f_equal; word.
+  - rewrite H2.
+    replace (Init.Nat.add (Z.to_nat (Z.sub (Datatypes.length slice) 1)) 1) with ((length slice)).
+    2: word.
+    replace (word.unsigned (word.add first 1)) with (uint.Z (length slice)).
+    2: word.
+    replace ((uint.Z (length slice) `mod` length slice)) with 0.
+    2: { replace (uint.Z _) with (Z.of_nat (length slice)) by word. rewrite Z_mod_same //. word. }
+    rewrite subslice_comm.
+    rewrite drop_app_length.
+    rewrite subslice_comm.
+    rewrite drop_0.
+    rewrite take_app_le. 2: word.
+    f_equal. word.
+Qed.
+
+Theorem remove_one : forall slice (first : u64) (count : u64) e, 
+  uint.Z (length slice) ≠ 0 ->
+  length slice + 1 < 2 ^ 63 ->
+  uint.Z first < length slice ->
+  0 < uint.Z count <= length slice ->
+  slice !! uint.nat first = Some e -> 
+  valid_elems slice first count = e :: valid_elems slice (word.modu ((word.add) first 1) (length slice)) (word.sub count 1).
+Proof.
+  intuition.
+  unfold valid_elems.
+  (* NOTE: needs to carefully do what the old [word_cleanup] would do, so that
+  the statements of [add_one_lemma_1] and [add_one_lemma_2] apply. *)
+  rewrite -> ?word.unsigned_add, ?word.unsigned_sub,
+    ?word.unsigned_modu_nowrap, ?unsigned_U64; [ | word .. ].
+  rewrite -> !wrap_small by word.
+  replace (uint.Z (W64 (length slice))) with (Z.of_nat (length slice)) by word.
+  rewrite (subslice_split_r (uint.nat first) (uint.nat first + 1) _ (_++_)).
+  - rewrite (remove_one_lemma_1 slice first e); eauto.
+    rewrite app_inv_head_iff.
+    apply remove_one_lemma_2; eauto.
+  - word.
+  - rewrite length_app. word.
+Qed.
+
+
+  Definition isBufferedChanLogical (ch: loc) (γ: chan_names) (chan_type: ty) (size: nat) (vs: valid_chan_state) 
+  (is_single_party: bool) (send_count recv_count: nat) (count: Z) 
+  (first: u64) (xs: list val) (Psingle: Z -> val -> iProp Σ) (Pmulti: val -> iProp Σ) 
+  (Qsingle: Z -> iProp Σ) (Qmulti: iProp Σ) (R: nat -> iProp Σ): iProp Σ := 
+   ⌜count = (send_count - recv_count)⌝ ∗
+   ⌜size = length xs⌝ ∗
+   buff_size_inv count first (length xs) ∗
+   ([∗ list] i↦x ∈ valid_elems xs first count, P is_single_party (recv_count + i) x Psingle Pmulti) ∗ 
+   big_sep_seq send_count (size - count) (λ i, Q is_single_party (i - size) Qsingle Qmulti).
+
+Definition isBufferedChan (ch: loc) (γ: chan_names) (chan_type: ty) (size: nat) (vs: valid_chan_state) 
+  (is_single_party: bool) (send_count recv_count: nat) (count: Z) 
+  (buff: Slice.t) (first: u64) (Psingle: Z -> val -> iProp Σ) (Pmulti: val -> iProp Σ) 
+  (Qsingle: Z -> iProp Σ) (Qmulti: iProp Σ) (R: nat -> iProp Σ): iProp Σ := 
+   ∃ (xs: list val), 
+   slice.own_slice_small buff chan_type (DfracOwn 1) xs ∗
+   isBufferedChanLogical ch γ chan_type size vs is_single_party 
+     send_count recv_count count first xs Psingle Pmulti Qsingle Qmulti R.
+
+
+(* Unbuffered channel invariant *)
+Definition isUnbufferedChan (ch: loc) (γ: chan_names) (chan_type: ty) 
+  (v: val) (vs: valid_chan_state) (is_single_party: bool) (send_count recv_count: nat) 
+  (Psingle: Z -> val -> iProp Σ) (Pmulti: val -> iProp Σ) 
+  (Qsingle: Z -> iProp Σ) (Qmulti: iProp Σ) (R: nat -> iProp Σ): iProp Σ := 
+    chan_state_facts vs send_count recv_count v chan_type ∗
+    chan_state_resources vs γ is_single_party send_count recv_count v Psingle Pmulti Qsingle Qmulti.
+
+(* Inner channel invariant with a unified structure *)
+Definition isChanInner (ch: loc) (γ: chan_names) (chan_type: ty) 
+    (size: nat) (is_single_party: bool) (buff: Slice.t) 
+    (Psingle: Z -> val -> iProp Σ) (Pmulti: val -> iProp Σ) 
+    (Qsingle: Z -> iProp Σ) (Qmulti: iProp Σ) (R: nat -> iProp Σ): iProp Σ := 
+  ∃ (vs: valid_chan_state) (count: nat) (first: u64) (v: val) (send_count recv_count: nat),
+    (* Physical state - directly using word representation *)
+    "value" ∷ ch ↦[(Channel chan_type) :: "v"] v ∗ 
+    "chan_state" ∷ ch ↦[(Channel chan_type) :: "state"] #(valid_to_word vs) ∗
+    "count" ∷ ch ↦[(Channel chan_type) :: "count"] #(W64 count) ∗ 
+    (if size =? 0 then emp else "first" ∷ ch ↦[(Channel chan_type) :: "first"] #first) ∗
+    
+    (* Counter resources *)
+    "HSndCtrAuth" ∷ own_send_counter_auth γ send_count (send_ctr_frozen vs) ∗ 
+    "HRcvCtrAuth" ∷ own_recv_counter_auth γ recv_count (recv_ctr_frozen vs send_count recv_count) ∗ 
+    
+    (* Close resources *)
+    "HCloseTokPostClose" ∷ 
+      (match vs with
+        | Valid_closed => 
+           ∃ (n: nat) (close_tok_names: gset gname), 
+             own_closed_tok_post_close γ n close_tok_names ∗ own_send_counter_frag γ n 1
+        | _ => True
+       end) ∗
+
+    (* Buffer vs unbuffered channels *)
+    "HChanState" ∷ 
+      (if size =? 0 then
+        isUnbufferedChan ch γ chan_type v vs is_single_party send_count recv_count 
+        Psingle Pmulti Qsingle Qmulti R
+      else
+        isBufferedChan ch γ chan_type size vs is_single_party send_count recv_count count
+        buff first Psingle Pmulti Qsingle Qmulti R).
+
+Lemma buff_enqueue_logical (ch: loc) (γ: chan_names) (chan_type: ty) 
+        (size: nat) (vs: valid_chan_state) (is_single_party: bool) 
+        (send_count recv_count: nat) (count: nat) (first: u64) 
+        (xs: list val) (new_xs: list val) (v: val) 
+        (Psingle: Z -> val -> iProp Σ) (Pmulti: val -> iProp Σ) 
+        (Qsingle: Z -> iProp Σ) (Qmulti: iProp Σ) (R: nat -> iProp Σ)
+        (i: nat) (q: Qp):
+        
+        val_ty v chan_type ->
+        count < size ->  (* Buffer is not full *)
+        (if is_single_party then q = 1%Qp else (q < 1)%Qp) ->
+        size > 0 ->
+        size + 1 < 2^63 ->
+        count + 1 < 2^63 ->
+        
+        (* Explicitly specify what new_xs is *)
+        new_xs = <[uint.nat (word.modu (word.add first (W64 count)) (W64 size)):=v]> xs ->
+        
+        
+        (* Input resources *)
+        "HBuffChLogical" ∷ isBufferedChanLogical ch γ chan_type size vs is_single_party 
+          send_count recv_count count first xs Psingle Pmulti Qsingle Qmulti R ∗
+        "HP" ∷ P is_single_party i v Psingle Pmulti ∗
+        "HSndCtrAuth" ∷ own_send_counter_auth γ send_count false ∗
+        "HSndPerm" ∷ own_send_counter_frag γ i q
+        
+        ==∗
+        
+        (* Output resources *)
+        "HBuffChLogical" ∷ isBufferedChanLogical ch γ chan_type size vs is_single_party 
+          (S send_count) recv_count (count + 1) first new_xs Psingle Pmulti Qsingle Qmulti R ∗
+        "HQ" ∷ Q is_single_party (send_count - size) Qsingle Qmulti ∗
+        "HSndCtrAuth" ∷ own_send_counter_auth γ (S send_count) false ∗
+        "HSndPerm" ∷ own_send_counter_frag γ (S i) q.
+
+        Proof.
+          intros Hvt Hcount_lt Hsp  Hsize_pos Hsize_bound Hcount_bound Hnew_xs .
+          iIntros "(HBuffChLogical & HP & HSndCtrAuth & HSndPerm)".
+          
+          (* Unfold the logical channel state *)
+          iDestruct "HBuffChLogical" as "(%HBuffCount & %Hsize & Hsizeinv & HPs & HQs)".
+          
+          (* Extract buff_size_inv components *)
+          iDestruct "Hsizeinv" as "(%Hcount_le & %Hfirst_lt & %Hsize_pos_old & %Hsize_bound_old & %Hcount_bound_old)".
+          
+          (* Update the send counter *)
+          destruct is_single_party.
+          
+          - (* Single-party case *)
+            subst q.
+            iDestruct (send_counter_elem with "[$HSndCtrAuth] [$HSndPerm]") as "%Helem".
+            subst i.
+            iMod (send_counter_update γ send_count send_count with "[$HSndCtrAuth $HSndPerm]") as "[HSndCtrAuth HSndPerm]".
+            
+            (* Extract Q from big_sep_seq *)
+            iDestruct (big_sep_seq_pop send_count (size - count) (λ i, Q true (i - size) Qsingle Qmulti) 
+                       with "HQs") as "[HQ HQs]".
+            { lia. }
+            
+            (* Update Ps for the new buffer content *)
+            (* This is the tricky part - we need to relate old and new valid_elems *)
+            
+            (* First, build the separation logic predicate for the updated buffer content *)
+            iAssert ([∗ list] i↦x ∈ valid_elems new_xs first (W64 (count + 1)), 
+                      P true (recv_count + i) x Psingle Pmulti)%I with "[HPs HP]" as "HPs'".
+            {
+
+              subst new_xs.
+              replace size with (length xs).
+              replace (W64 (count + 1)) with (w64_word_instance .(word.add) (W64 count) (W64 1))
+              by word.
+              rewrite (add_one xs first count v).
+              {
+                rewrite big_sepL_snoc. iFrame.
+                replace ((recv_count + length (valid_elems xs first (W64 count))))
+                with (Z.of_nat send_count).
+                {
+                  iFrame.
+                }
+                unfold valid_elems.
+                rewrite subslice_length.
+                {
+                 word. 
+                }
+                rewrite length_app. word.
+              }
+              {
+                word.
+              }
+              {
+               word. 
+              }
+              {
+               word. 
+              }
+              {
+               word. 
+              }
+            }
+            
+            (* Reconstruct buff_size_inv for the new state *)
+            iAssert (⌜count + 1 <= size⌝ ∗ 
+                     ⌜word.unsigned first < size⌝ ∗ 
+                     ⌜size > 0⌝ ∗ 
+                     ⌜size + 1 < 2 ^ 63⌝ ∗
+                     ⌜count + 1 + 1 < 2 ^ 63⌝)%I as "Hsizeinv".
+            {
+              iPureIntro.
+              repeat split; try assumption; try lia.
+            }
+            
+            (* Reassemble the logical channel state *)
+            iModIntro.
+            iSplitL "Hsizeinv HPs' HQs".
+            {
+              unfold isBufferedChanLogical.
+              iFrame.
+              iSplitL "".
+              { iPureIntro. lia. }
+              iSplitL "".
+              { iPureIntro. subst new_xs. rewrite length_insert.
+              done. 
+             }
+              
+              (* Handle HQs *)
+              rewrite Nat2Z.inj_succ. 
+              replace (size - (count + 1)) with (size - count - 1) by lia.
+              iFrame "HQs". iPureIntro. subst new_xs. rewrite length_insert.
+              word.
+            }
+            
+            (* Return the remaining resources *)
+            iFrame "HQ HSndCtrAuth HSndPerm".
+            
+          - (* Multi-party case - similar structure but with different counter checks *)
+            iDestruct (send_counter_lower with "[$HSndCtrAuth] [$HSndPerm]") as "%Hlower".
+            iMod (send_counter_update γ send_count i with "[$HSndCtrAuth $HSndPerm]") as "[HSndCtrAuth HSndPerm]".
+            
+            (* Extract Q from big_sep_seq *)
+            iDestruct (big_sep_seq_pop send_count (size - count) (λ i, Q false (i - size) Qsingle Qmulti) 
+                       with "HQs") as "[HQ HQs]".
+            { lia. }
+            
+            (* Update Ps for the new buffer content - similar to above *)
+            iAssert ([∗ list] i↦x ∈ valid_elems new_xs first (W64 (count + 1)), 
+                      P false (recv_count + i) x Psingle Pmulti)%I with "[HPs HP]" as "HPs'".
+            {
+               (* Similar to single-party case *)
+              subst new_xs.
+              replace size with (length xs).
+              replace (W64 (count + 1)) with (w64_word_instance .(word.add) (W64 count) (W64 1))
+              by word.
+              rewrite (add_one xs first count v).
+              {
+                rewrite big_sepL_snoc. iFrame.
+              }
+              {
+                word.
+              }
+              {
+               word. 
+              }
+              {
+               word. 
+              }
+              {
+               word. 
+              }
+            }
+            
+            (* Reconstruct buff_size_inv for the new state *)
+            iAssert (⌜count + 1 <= size⌝ ∗ 
+                     ⌜word.unsigned first < size⌝ ∗ 
+                     ⌜size > 0⌝ ∗ 
+                     ⌜size + 1 < 2 ^ 63⌝ ∗
+                     ⌜count + 1 + 1 < 2 ^ 63⌝)%I as "Hsizeinv".
+            {
+              iPureIntro.
+              repeat split; try assumption; try lia.
+            }
+            
+            (* Reassemble the logical channel state *)
+            iModIntro.
+            iSplitL "Hsizeinv HPs' HQs".
+            {
+              unfold isBufferedChanLogical.
+              iFrame.
+              iSplitL "".
+              { iPureIntro. lia. }
+              iSplitL "".
+              { iPureIntro.  subst new_xs. rewrite length_insert.
+              done.  }
+              
+              (* Handle HQs *)
+              rewrite Nat2Z.inj_succ.
+              replace (size - (count + 1)) with (size - count - 1) by lia.
+              iFrame "HQs". iPureIntro. subst new_xs. rewrite length_insert.
+              word.
+            }
+            
+            (* Return the remaining resources *)
+            iFrame "HQ HSndCtrAuth HSndPerm".
+        Qed.
+
+        Lemma buff_dequeue_logical (ch: loc) (γ: chan_names) (chan_type: ty) 
+  (size: nat) (vs: valid_chan_state) (is_single_party: bool) 
+  (send_count recv_count: nat) (count: nat) (first: u64) (new_first: u64)
+  (xs: list val) (v: val) 
+  (Psingle: Z -> val -> iProp Σ) (Pmulti: val -> iProp Σ) 
+  (Qsingle: Z -> iProp Σ) (Qmulti: iProp Σ) (R: nat -> iProp Σ)
+  (i: nat) (q: Qp):
+  
+  count > 0 ->  (* Buffer is not empty *)
+  (if is_single_party then q = 1%Qp else (q < 1)%Qp) ->
+  size > 0 ->
+  
+  (* Relate old and new first pointers *)
+  new_first = word.modu (word.add first 1) (W64 size) ->
+  
+  (* The value at the front of the buffer *)
+  xs !! (uint.nat first) = Some v ->
+  
+  (* Input resources *)
+  "HBuffChLogical" ∷ isBufferedChanLogical ch γ chan_type size vs is_single_party 
+    send_count recv_count count first xs Psingle Pmulti Qsingle Qmulti R ∗
+  "HQ" ∷ Q is_single_party i Qsingle Qmulti ∗
+  "HRecvCtrAuth" ∷ own_recv_counter_auth γ recv_count false ∗
+  "HRecvPerm" ∷ own_recv_counter_frag γ i q
+  
+  ==∗
+  
+  (* Output resources *)
+  "HBuffChLogical" ∷ isBufferedChanLogical ch γ chan_type size vs is_single_party 
+    send_count (S recv_count) (count - 1) new_first xs Psingle Pmulti Qsingle Qmulti R ∗
+  "HP" ∷ P is_single_party recv_count v Psingle Pmulti ∗
+  "HRecvCtrAuth" ∷ own_recv_counter_auth γ (S recv_count) false ∗
+  "HRecvPerm" ∷ own_recv_counter_frag γ (S i) q.
+
+  Proof.
+    intros Hcount_gt Hsp Hsize_pos Hnew_first Hv_at_first.
+    iIntros "(HBuffChLogical & HQ & HRecvCtrAuth & HRecvPerm)".
+    
+    (* Unfold the logical channel state *)
+    iDestruct "HBuffChLogical" as "(%HBuffCount & %Hsize & %Hsizeinv & HPs & HQs)".
+    
+    (* Extract buff_size_inv components *)
+    destruct Hsizeinv as (Hcount_le & Hfirst_lt & Hsize_pos_old & Hsize_bound_old & Hcount_bound_old).
+    
+    (* Update recv counter *)
+    destruct is_single_party.
+    
+    - (* Single-party case *)
+      subst q.
+      iDestruct (recv_counter_elem with "[$HRecvCtrAuth] [$HRecvPerm]") as "%Helem".
+      subst i.
+      iMod (recv_counter_update γ recv_count recv_count with "[$HRecvCtrAuth $HRecvPerm]") as "[HRecvCtrAuth HRecvPerm]".
+      
+      (* Add the new Q to the sequence *)
+      iDestruct (big_sep_seq_snoc send_count (size - count) (λ i, Q true (i - size) Qsingle Qmulti) 
+                 with "[HQ HQs]") as "HQs".
+      { lia. }
+      { iFrame "HQs". 
+      replace (Z.of_nat recv_count) with ((send_count + (size - count) - size)) by lia.
+      iFrame.
+      }
+      
+      (* Use remove_one to handle the buffer elements *)
+      assert (Hremove_one: valid_elems xs first (W64 count) = 
+                           v :: valid_elems xs new_first (W64 (count - 1))).
+      {
+        subst new_first.
+      erewrite (remove_one xs first count); eauto;try word. 
+      replace ((w64_word_instance .(word.sub) (W64 count) (W64 1))) with (W64 (count - 1)) by word.
+      replace size with (length xs). done.
+      }
+      
+      (* Extract P for the element we're dequeuing *)
+      rewrite Hremove_one.
+      iDestruct (big_sepL_cons with "HPs") as "[HP HPs']".
+      
+      (* Reconstruct buff_size_inv for the new state *)
+      iAssert (⌜count - 1 <= size⌝ ∗ 
+               ⌜word.unsigned new_first < size⌝ ∗ 
+               ⌜size > 0⌝ ∗ 
+               ⌜size + 1 < 2 ^ 63⌝ ∗
+               ⌜count < 2 ^ 63⌝)%I as "%Hsizeinvnew".
+      {
+        iPureIntro.
+        repeat split.
+        - lia.
+        - subst new_first. word. 
+        - assumption.
+        - lia.
+        - lia.
+      }
+      
+      (* Reassemble the logical channel state *)
+      iModIntro.
+      iSplitL "HPs' HQs".
+      {
+        unfold isBufferedChanLogical.
+        iFrame.
+        iSplitL "".
+        { iPureIntro. lia. }
+        iSplitL "".
+        { iPureIntro. assumption. }
+        
+        (* Handle HQs *)
+        replace (size - (count - 1)) with (size - count + 1) by lia.
+        iFrame "HQs".
+        iSplitL "".
+        { iPureIntro. word. }
+        iFrame.
+        setoid_rewrite big_sepL_proper.
+        {
+        iFrame.
+        }
+        {
+          intros. iSimpl.
+            iSplitL.
+            {
+             iIntros "H". done. 
+            }
+            iIntros "H". done.
+        }
+        {
+        intros. iSimpl.
+            iSplitL.
+            {
+             iIntros "H".  
+              rewrite Z.add_comm. 
+              replace (Z.of_nat k + Z.of_nat (S recv_count)) with (Z.of_nat recv_count + Z.of_nat (S k)) by lia.
+              iFrame.
+            }
+            {
+             iIntros "H".  
+              rewrite Z.add_comm. 
+              replace (Z.of_nat (S k) + Z.of_nat  recv_count) with (Z.of_nat (S recv_count) + Z.of_nat k) by lia.
+              iFrame.
+            }
+        }
+      }
+      replace ((recv_count + 0%nat)) with (Z.of_nat recv_count) by lia.
+      iFrame.
+      
+    - (* Multi-party case *)
+      (* Similar to single-party but with different counter handling *)
+      iDestruct (recv_counter_lower with "[$HRecvCtrAuth] [$HRecvPerm]") as "%Hlower".
+      iMod (recv_counter_update γ recv_count i with "[$HRecvCtrAuth $HRecvPerm]") as "[HRecvCtrAuth HRecvPerm]".
+      
+      (* Add the new Q to the sequence *)
+      iDestruct (big_sep_seq_snoc send_count (size - count) (λ i, Q false (i - size) Qsingle Qmulti) 
+                 with "[HQ HQs]") as "HQs".
+      { lia. }
+      { iFrame "HQs". 
+      replace (Z.of_nat recv_count) with ((send_count + (size - count) - size)) by lia.
+      iFrame.
+        unfold Q.
+        destruct bool_decide eqn: Hbouter.
+        {
+          rewrite bool_decide_eq_true in Hbouter.
+          destruct bool_decide eqn: Hbinner.
+          {
+            done.
+          }
+          {
+            destruct i;first done.
+            done.
+          }
+        }
+        {
+          rewrite bool_decide_eq_false in Hbouter.
+          destruct bool_decide.
+          {
+            done.
+          }
+          iFrame.
+        }
+
+      }
+      
+      (* Use remove_one to handle the buffer elements *)
+      assert (Hremove_one: valid_elems xs first (W64 count) = 
+                           v :: valid_elems xs new_first (W64 (count - 1))).
+      {
+        subst new_first.
+      erewrite (remove_one xs first count); eauto;try word. 
+      replace ((w64_word_instance .(word.sub) (W64 count) (W64 1))) with (W64 (count - 1)) by word.
+      replace size with (length xs). done.
+      }
+      
+      (* Extract P for the element we're dequeuing *)
+      rewrite Hremove_one.
+      iDestruct (big_sepL_cons with "HPs") as "[HP HPs']".
+      
+      (* Reconstruct buff_size_inv for the new state *)
+      iAssert (⌜count - 1 <= size⌝ ∗ 
+               ⌜word.unsigned new_first < size⌝ ∗ 
+               ⌜size > 0⌝ ∗ 
+               ⌜size + 1 < 2 ^ 63⌝ ∗
+               ⌜count < 2 ^ 63⌝)%I as "%Hsizeinv".
+      {
+        iPureIntro.
+        repeat split.
+        - lia.
+        - subst new_first. word. 
+        - assumption.
+        - word.
+        - lia.
+      }
+      
+      (* Reassemble the logical channel state *)
+      iModIntro.
+      iSplitL "HPs' HQs".
+      {
+        unfold isBufferedChanLogical.
+        iFrame "".
+        iSplitL "".
+        { iPureIntro. lia. }
+        iSplitL "".
+        { iPureIntro. assumption. }
+        
+        (* Handle HQs *)
+        replace (size - (count - 1)) with (size - count + 1) by lia.
+        iFrame "HQs".
+        iSplitL "".
+        { iPureIntro. word. }
+        iFrame.
+      }
+      {
+        intros. iSimpl.
+        iFrame.
+      }
+  Qed.
+
+  Lemma wp_Channel__BufferedTrySend (ch: loc) (v: val) (γ: chan_names) (chan_type: ty) 
+  (buff: Slice.t) (is_single_party: bool) (q: Qp) (first: u64) 
+  (size: nat) (count: nat) (vs: valid_chan_state) 
+  (send_count recv_count: nat) (Psingle: Z -> val -> iProp Σ) 
+  (Pmulti: val -> iProp Σ) (Qsingle: Z -> iProp Σ) (Qmulti: iProp Σ) 
+  (R: nat -> iProp Σ) (i: nat):
+
+val_ty v chan_type ->
+(if is_single_party then q = 1%Qp else (q < 1)%Qp) ->
+vs ≠ Valid_closed ->
+(#buff.(Slice.sz) = #(W64 size)) ->
+size > 0 ->
+size + 1 < 2^63 ->
+count + 1 < 2^63 ->
+
+{{{ 
+  "#buff" ∷ ch ↦[(Channel chan_type) :: "buffer"]□ (slice_val buff) ∗
+  "chan_state" ∷ ch ↦[(Channel chan_type) :: "state"] #(valid_to_word vs) ∗  
+  "count" ∷ ch ↦[(Channel chan_type) :: "count"] #(W64 count) ∗ 
+  "first" ∷ ch ↦[(Channel chan_type) :: "first"] #first ∗ 
+  "HP" ∷ P is_single_party i v Psingle Pmulti ∗ 
+  "HSen" ∷ own_send_counter_frag γ i q ∗ 
+  "HSndCtrAuth" ∷ own_send_counter_auth γ send_count false ∗
+  "HCh" ∷ isBufferedChan ch γ chan_type size vs
+            is_single_party send_count recv_count count
+            buff first Psingle Pmulti Qsingle Qmulti R
+}}}
+Channel__BufferedTrySend chan_type #ch v
+{{{ (success: bool), RET #success;
+  "chan_state" ∷ ch ↦[(Channel chan_type) :: "state"] #(valid_to_word vs) ∗
+  
+  if success then
+    (* Successful send - buffer had space *)
+    "count" ∷ ch ↦[(Channel chan_type) :: "count"] #(W64 (S count)) ∗ 
+    "first" ∷ ch ↦[(Channel chan_type) :: "first"] #first ∗ 
+    "HSen" ∷ own_send_counter_frag γ (S i) q ∗ 
+    "HSndCtrAuth" ∷ own_send_counter_auth γ (S send_count) false ∗
+    "HQ" ∷ Q is_single_party (i - size) Qsingle Qmulti ∗ 
+    "HCh" ∷ isBufferedChan ch γ chan_type size vs
+              is_single_party (S send_count) recv_count (S count)
+              buff first Psingle Pmulti Qsingle Qmulti R
+  else
+    (* Failed send - buffer was full *)
+    "count" ∷ ch ↦[(Channel chan_type) :: "count"] #(W64 count) ∗ 
+    "first" ∷ ch ↦[(Channel chan_type) :: "first"] #first ∗ 
+    "HP" ∷ P is_single_party i v Psingle Pmulti ∗ 
+    "HSen" ∷ own_send_counter_frag γ i q ∗ 
+    "HSndCtrAuth" ∷ own_send_counter_auth γ send_count false ∗
+    "HCh" ∷ isBufferedChan ch γ chan_type size vs
+              is_single_party send_count recv_count count
+              buff first Psingle Pmulti Qsingle Qmulti R
+}}}.
+Proof.
+  intros Hvt Hsp  Hnot_closed Hbuff_sz Hsize_pos Hsize_bound Hcount_bound.
+  iIntros (Φ) "Hpre HΦ".
+  iNamed "Hpre".
+  
+  wp_rec. wp_pures.
+  
+  (* Check if channel is closed *)
+  wp_loadField.
+  wp_pures.
+
+  wp_if_destruct.
+  {
+    destruct vs. all: try done.
+  }
+  
+  
+  (* Check if buffer has space *)
+  wp_loadField.
+  wp_loadField.
+  wp_pures.
+  
+  (* Extract buffer channel resources *)
+  iDestruct "HCh" as (xs) "(HBuffSlice & %Hsize & %Hsizeinv & %HBuffcount & HPs & HQs)".
+  destruct HBuffcount as (Hcount_le & Hfirst_lt & Hsize_pos_old & Hsize_bound_old & Hcount_bound_old).
+  
+  (* Get slice size *)
+  iDestruct (slice.own_slice_small_sz with "HBuffSlice") as %Hslice_size.
+  replace buff.(Slice.sz) with (W64 (length xs)) by word.
+  
+  (* Check if count < buffer size *)
+  wp_apply wp_slice_len.
+  wp_if_destruct.
+
+  - (* Case: Buffer has space - can send *)
+    rewrite <- Hsizeinv in Hcount_le.
+    
+      (* Calculate last index and set the value *)
+      wp_loadField.
+      wp_loadField.
+      wp_loadField. wp_apply wp_slice_len.
+      wp_apply wp_ref_to; first val_ty.
+      iIntros (last_ptr) "Hlast_ptr".
+      wp_pures.
+      wp_load.
+      
+      (* Set the value in the slice *)
+      wp_loadField.
+      
+      (* Locate target index in slice *)
+      set (idx := uint.nat (word.modu (word.add first (word.unsigned count)) (word.unsigned size))).
+      
+      (* Use SliceSet to store the value *)
+      wp_apply (slice.wp_SliceSet with "[$HBuffSlice]").
+      { iPureIntro. split.
+        - apply lookup_lt_is_Some_2. word.
+        - exact Hvt.
+      }
+      iIntros "HBuffSlice".
+      
+      (* Update channel count field *)
+      wp_pures.
+      wp_loadField.
+      wp_storeField.
+      
+      (* Return success *)
+      wp_pures.
+
+      (* Build assertion for counter elements *)
+      iAssert (own_send_counter_auth γ send_count false ∗ 
+      own_send_counter_frag γ i q ∗ 
+      ⌜if is_single_party then send_count = i else i <= send_count⌝%I)%I 
+      with "[HSndCtrAuth HSen]" as "(HSndCtrAuth & HSen & %Hispz)".
+      {
+      destruct is_single_party.
+      - subst q.
+      iDestruct (send_counter_elem with "[$HSndCtrAuth] [$HSen]") as "%Hag2".
+      iFrame. iPureIntro. done.
+      - iDestruct (send_counter_lower with "[$HSndCtrAuth] [$HSen]") as "%Hag2".
+      iFrame. iPureIntro. lia.
+      }
+
+      
+      (* Set the new buffer state *)
+      set (new_xs := <[idx:=v]> xs).
+      iMod (buff_enqueue_logical ch γ chan_type size vs is_single_party
+      send_count recv_count count first xs new_xs v
+      Psingle Pmulti Qsingle Qmulti R i q
+      with "[ HPs HQs HP HSndCtrAuth HSen]") as 
+      "IH". all: (try done;try word).
+      {
+        subst idx.
+        subst new_xs.
+        replace (W64 (uint.Z (W64 count))) with (W64 count) by word.
+        replace ((W64 (uint.Z (W64 size)))) with (W64 size) by word.
+        exact.
+      }
+      { 
+       iFrame. iPureIntro. word.
+      }
+      iModIntro. iApply "HΦ".
+      iFrame. iNamed "IH". iFrame.
+            (* First, replace count + 1 with S count *)
+      replace (count + 1)%nat with (S count)%nat by lia.
+
+      (* Replace word.add (W64 count) (W64 1) with W64 (S count) *)
+      replace (w64_word_instance.(word.add) (W64 count) (W64 1)) with (W64 (S count)) by word.
+
+     
+
+      (* Now we can frame everything except HQ *)
+      iFrame.
+      replace (count + 1) with (Z.of_nat (S count)) by lia.
+      subst new_xs. subst idx.
+      replace ((W64 (uint.Z (W64 size)))) with (W64 size) by word.
+      replace ((W64 (uint.Z (W64 count)))) with (W64 count) by word.
+      replace (length xs) with size in Hslice_size.
+      replace (buff .(Slice.sz)) with (W64 size).
+      iFrame. 
+      unfold Q.
+      destruct is_single_party.
+      {
+       subst q. subst send_count. iFrame.
+      }
+      {
+        unfold Q.
+        destruct bool_decide eqn: Hbouter.
+        {
+          rewrite bool_decide_eq_true in Hbouter.
+          destruct bool_decide eqn: Hbinner.
+          {
+            done.
+          }
+          {
+            rewrite bool_decide_eq_false in Hbinner.
+            lia.
+          }
+        }
+        {
+          rewrite bool_decide_eq_false in Hbouter.
+          destruct bool_decide.
+          {
+            done.
+          }
+          iFrame.
+        }
+      }
+ - iModIntro. iApply "HΦ". iFrame. done.
+Qed. 
+
+Lemma wp_Channel__BufferedTryReceiveLocked (ch: loc) (γ: chan_names) (chan_type: ty) 
+  (size: nat) (mu_l: loc) (is_single_party: bool)  (vs: valid_chan_state)
+  (count: nat) (send_count recv_count: nat) (first: u64) (buff: Slice.t)
+  (Psingle: Z -> val -> iProp Σ) (Pmulti: val -> iProp Σ) 
+  (Qsingle: Z -> iProp Σ) (Qmulti: iProp Σ) (R Ri: nat -> iProp Σ)
+  (i: nat) (q: Qp):
+
+has_zero chan_type ->
+(if is_single_party then q = 1%Qp else (q < 1)%Qp) ->
+{{{ 
+  (* Common preconditions for all cases *)
+  "#buff" ∷ ch ↦[(Channel chan_type) :: "buffer"]□ (slice_val buff) ∗
+  "count" ∷ ch ↦[(Channel chan_type) :: "count"] #(W64 count) ∗ 
+  "chan_state" ∷ ch ↦[(Channel chan_type) :: "state"] #(valid_to_word vs) ∗
+  "first" ∷ ch ↦[(Channel chan_type) :: "first"] #first ∗ 
+  "HRcvPerm" ∷ own_recv_perm γ q i Ri ∗
+  "HCh" ∷ isBufferedChan ch γ chan_type size vs is_single_party
+              send_count recv_count count buff first Psingle Pmulti Qsingle Qmulti R ∗  
+
+  (* Conditional resources based on channel state *)
+ 
+    (* Non-closed channel with data or empty *)
+    if (uint.Z (W64 0) <? uint.Z (W64 count)) then
+      (* Channel has data *)
+      "HQ" ∷ Q is_single_party i Qsingle Qmulti ∗
+      "HRecvCtrAuth" ∷ own_recv_counter_auth γ recv_count (recv_ctr_frozen vs send_count recv_count)
+    else
+      match vs with 
+      | Valid_closed => 
+          (* Closed channel case *)
+        ∃ (close_tok_names: gset gname) ,
+        "#HSndCtrAuth" ∷ own_send_counter_auth γ send_count true ∗ 
+        "HRcvCtrAuth" ∷ own_recv_counter_auth γ recv_count (recv_ctr_frozen vs send_count recv_count) ∗
+        "HCloseTokPostClose" ∷ own_closed_tok_post_close γ send_count close_tok_names ∗  
+        "HSc" ∷ own_send_counter_frag γ send_count 1 ∗
+        "%Hct" ∷ ⌜count = 0%nat⌝ 
+      | _ => emp
+  end
+}}}
+Channel__BufferedTryReceiveLocked chan_type #ch
+{{{ (success: bool) (v: val) (has_value: bool), RET (#success, v, #has_value);
+  (* Common postconditions *)
+  "chan_state" ∷ ch ↦[(Channel chan_type) :: "state"] #( valid_to_word vs) ∗
+  
+  (* Case-specific postconditions *)
+  match success, has_value with
+  | true, true =>
+    (* Successful receive with value *)
+    ∃ (new_first: u64),
+    "count" ∷ ch ↦[(Channel chan_type) :: "count"] #(W64 (count - 1)) ∗
+    "first" ∷ ch ↦[(Channel chan_type) :: "first"] #new_first ∗ 
+    "HP" ∷ P is_single_party i v Psingle Pmulti ∗
+    "HRecvPerm" ∷ own_recv_perm γ q (S i) Ri ∗
+    "%HVt" ∷ ⌜val_ty v chan_type⌝ ∗
+    "HCh" ∷ isBufferedChan ch γ chan_type size vs is_single_party
+            send_count (S recv_count) (count - 1) buff new_first 
+            Psingle Pmulti Qsingle Qmulti R ∗
+    "HRecvCtrAuth" ∷ own_recv_counter_auth γ (S recv_count) 
+                    (recv_ctr_frozen vs send_count (S recv_count))
+  | true, false =>
+    (* Successful but channel is closed *)
+    "count" ∷ ch ↦[(Channel chan_type) :: "count"] #(W64 0) ∗
+    "first" ∷ ch ↦[(Channel chan_type) :: "first"] #first ∗ 
+    "HRi" ∷ Ri recv_count ∗
+    "#HScfroz" ∷ own_send_counter_auth γ send_count true ∗
+    "#HRcfroz" ∷ own_recv_counter_auth γ recv_count true ∗
+    "HSc" ∷ own_send_counter_frag γ recv_count 1 ∗
+    ∃ (close_tok_names: gset gname) (γr: gname),
+    "HCloseTokPostCloseNew" ∷ own_closed_tok_post_close γ recv_count (close_tok_names ∖ {[γr]}) ∗
+    ⌜ vs = Valid_closed ⌝ ∗ 
+    ⌜v = zero_val chan_type⌝
+  | false, true =>
+    (* No value available, empty channel *)
+    "count" ∷ ch ↦[(Channel chan_type) :: "count"] #(W64 0) ∗
+    "first" ∷ ch ↦[(Channel chan_type) :: "first"] #first ∗ 
+    "HRcvPerm" ∷ own_recv_perm γ q i Ri ∗  
+  "HCh" ∷ isBufferedChan ch γ chan_type size vs is_single_party
+              send_count recv_count count buff first Psingle Pmulti Qsingle Qmulti R ∗  
+    ⌜v = zero_val chan_type⌝ ∗ 
+    ⌜ W64 count = W64 0 ⌝ ∗ 
+    ⌜vs =?= Valid_closed = false⌝
+  | _, _ =>
+    (* Impossible case *)
+    False
+  end
+}}}.
+Proof.
+  intros Hzero Hsp .
+  iIntros (Φ) "Hpre HΦ".
+  iNamed "Hpre".
+  
+  wp_rec. wp_pures.
+  wp_apply wp_ref_of_zero; first done.
+  iIntros (v_ptr) "Hv_ptr".
+  wp_pures.
+  
+  (* Load channel count *)
+  wp_auto.
+  wp_pures.
+  
+  (* Branch based on count *)
+  wp_if_destruct.
+  
+  - (* Case: channel has data - count > 0 *)
+    simpl. (* All non-closed states with data follow similar pattern *)
+      (* Extract resources for channels with data *)
+      assert (uint.Z (W64 0) <? uint.Z (W64 count) = true) as Hcond.
+      {
+        rewrite Z.ltb_lt. exact Heqb.
+      }
+      rewrite Hcond.
+      iNamed "Hpre".
+      assert (0 < count) by word.
+      (* Access the buffered channel resources *)
+      iDestruct "HCh" as (xs) "(HBuffSlice & %Hsize & %Hsizeinv & %HBuffCount & HPs & HQs)".
+    iPoseProof (slice.own_slice_small_sz with "HBuffSlice") as "%".
+      destruct HBuffCount as (Hcount_le & Hfirst_lt & Hsize_pos & Hsize_bound & Hcount_bound).
+      wp_auto.
+      edestruct (list_lookup_Z_lt xs (uint.Z first)) as [x Hlookup].
+        { word. }
+      wp_apply ((slice.wp_SliceGet _ _ buff chan_type (DfracOwn 1) xs first x  ) with "[$HBuffSlice]").
+      {
+        iPureIntro. done.
+      }
+      iIntros "[HBuffSlice %Hvty]".
+      wp_store. wp_loadField. 
+
+
+
+      wp_auto.
+      assert (send_count ≠ recv_count)%Z by lia.
+
+      
+      (* Calculate new_first *)
+      set (new_first := word.modu (word.add first 1) (W64 size)).
+      iNamed "HRcvPerm".
+      iDestruct "HRcvPerm" as "[HRecvCtrFrag Hctf]".
+      (* Apply buff_dequeue_logical lemma to update the logical buffer state *)
+      iMod (buff_dequeue_logical ch γ chan_type size _ is_single_party
+      send_count recv_count count first new_first xs x
+      Psingle Pmulti Qsingle Qmulti R i q
+      with "[HQ  HPs HQs HRecvCtrAuth HRecvCtrFrag]") as 
+      "IH".
+      (* Prove lemma preconditions *)
+        ++ word. (* count > 0 *)
+        ++ exact Hsp. (* ownership constraint *)
+        ++ lia. (* size > 0 *)
+        ++ reflexivity. (* new_first definition *)
+        ++ exact Hlookup. (* x is at first index *)
+        ++ iFrame. unfold recv_ctr_frozen.  
+        assert ((send_count =? recv_count) = false) as Heq_false.
+        { 
+          rewrite Z.eqb_neq. lia. 
+        }
+        rewrite Heq_false.
+        destruct vs; auto.
+        ++ wp_apply wp_slice_len. wp_auto. 
+        
+     
+      iNamed "IH".
+    
+      (* First, establish the condition as a pure fact *)
+      set (should_freeze := ((count =? 1) && (vs =?= Valid_closed))).
+      (* Now create a conditional assertion for the possibly-frozen counter *)
+      iAssert (bupd(own_recv_counter_auth γ (S recv_count) should_freeze))%I
+        with "[HRecvCtrAuth]" as ">HRecvCtrAuth".
+      {
+        destruct should_freeze.
+        - (* Case: need to freeze *)
+          iMod (recv_counter_freeze γ (S recv_count) with "HRecvCtrAuth") as "HRecvCtrAuth".
+          { done. }
+          iModIntro. iExact "HRecvCtrAuth".
+        - (* Case: no freezing needed *)
+          iModIntro. iExact "HRecvCtrAuth".
+      }
+
+      iModIntro. iApply "HΦ". 
+      
+      (* Update the counters *)
+      destruct is_single_party.
+      {
+        (* Single-party case *)
+        subst q.
+        iDestruct (recv_counter_elem with "[$HRecvCtrAuth] [$HRecvPerm]") as "%Helem".
+        unfold isBufferedChanLogical.
+        iDestruct "HBuffChLogical" as "(%Hct & %Hsz & %Hnewsizeinv & HPs & HQs)".
+        iFrame.
+        replace ((w64_word_instance .(word.sub) (W64 count) (W64 1))) with (W64 (count - 1)) by word. subst new_first.
+        replace size with (length xs) by lia.
+        replace (length xs) with (uint.nat buff .(Slice.sz)) by lia.
+        replace ((W64 (Z.of_nat (uint.nat buff .(Slice.sz))))) with (buff .(Slice.sz)) by word.
+        replace recv_count with i by lia.
+        iFrame. unfold recv_ctr_frozen.
+        destruct should_freeze eqn:Hb.
+        {
+          assert (count = 1%nat) as Hcount_one.
+          {
+            (* From should_freeze = true, we know (count =? 1) && (cs =?= Valid_closed) = true *)
+            (* For a conjunction to be true, both parts must be true *)
+            apply andb_prop in Hb as [Hcount_eq _].
+            lia.
+          }
+          subst count.
+          assert (i = recv_count) as Hi_eq.
+          { injection Helem as Hi_eq. exact Hi_eq. }
+
+          assert (send_count = S recv_count) as Hsend_eq.
+          {
+            simpl in Hct. (* Simplifies 1%nat - 1 to 0 *)
+            (* Now Hct is: 0 = send_count - S recv_count *)
+            lia.
+          }
+
+          assert (send_count = S i) as Hsend_eq_Si.
+          {
+            lia.
+          }
+
+          assert (send_count =? S i = true) as Hresult.
+          {
+            subst recv_count. 
+            rewrite Z.eqb_eq. lia.
+          }
+          rewrite Hresult.
+          assert (vs = Valid_closed) as Hcs_closed.
+          {
+            apply andb_prop in Hb as [_ Hcs_eq].
+            unfold valid_chan_state_eq in Hcs_eq.
+            destruct vs; try discriminate.
+            reflexivity.
+          }
+          subst vs. iFrame. iPureIntro. split;first val_ty. split; first lia. word. 
+        }
+        {
+          iSplitL ""; first done.
+          iSplitL ""; first word.
+          assert (count ≠ 1%nat ∨ vs ≠ Valid_closed) as Hcount_or_cs.
+          {
+            (* For a conjunction to be false, at least one part must be false *)
+            
+            apply not_true_iff_false in Hb.
+
+            rewrite andb_true_iff in Hb.
+            
+            apply Classical_Prop.not_and_or in Hb.
+            destruct Hb as [Hcount_not_eq | Hcs_not_eq].
+            - left. lia.
+            - right. destruct vs;auto.
+          }
+          destruct vs. all: try iFrame.
+          destruct Hcount_or_cs.
+          {
+            assert (send_count ≠ S i) as Hsend_neq_Si.
+            {
+              (* First, establish i = recv_count from Helem *)
+              injection Helem as Hi_eq.
+              lia.
+            }
+           assert ((send_count =? (S i)) = false).
+           {
+            rewrite Z.eqb_neq. lia.
+           }
+           rewrite H3.
+           iFrame.
+          }
+          {
+           done. 
+          }
+      }
+    }
+      {
+        (* Single-party case *)
+        iDestruct (recv_counter_lower with "[$HRecvCtrAuth] [$HRecvPerm]") as "%Helem".
+        unfold isBufferedChanLogical.
+        iDestruct "HBuffChLogical" as "(%Hct & %Hsz & %Hnewsizeinv & HPs & HQs)".
+        iFrame.
+        replace ((w64_word_instance .(word.sub) (W64 count) (W64 1))) with (W64 (count - 1)) by word. subst new_first.
+        replace size with (length xs) by lia.
+        replace (length xs) with (uint.nat buff .(Slice.sz)) by lia.
+        replace ((W64 (Z.of_nat (uint.nat buff .(Slice.sz))))) with (buff .(Slice.sz)) by word.
+        iFrame.
+        destruct should_freeze eqn:Hb.
+        {
+          assert (count = 1%nat) as Hcount_one.
+          {
+            (* From should_freeze = true, we know (count =? 1) && (cs =?= Valid_closed) = true *)
+            (* For a conjunction to be true, both parts must be true *)
+            apply andb_prop in Hb as [Hcount_eq _].
+            lia.
+          }
+          subst count.
+
+          assert (send_count = S recv_count) as Hsend_eq.
+          {
+            simpl in Hct. (* Simplifies 1%nat - 1 to 0 *)
+            (* Now Hct is: 0 = send_count - S recv_count *)
+            lia.
+          }
+
+          unfold recv_ctr_frozen.
+          assert (vs = Valid_closed) as Hcs_closed.
+          {
+            apply andb_prop in Hb as [_ Hcs_eq].
+            unfold valid_chan_state_eq in Hcs_eq.
+            destruct vs; try discriminate.
+            reflexivity.
+          }
+          subst vs. iFrame. assert ((send_count =? S recv_count) = true).
+          { inversion Hsend_eq. lia. }
+          simpl. iSplitL "";first done. iSplitL "";first (iPureIntro;word). rewrite H2. iFrame.
+        }
+        {
+          iSplitL ""; first done.
+          iSplitL ""; first word.
+          assert (count ≠ 1%nat ∨ vs ≠ Valid_closed) as Hcount_or_cs.
+          {
+            (* For a conjunction to be false, at least one part must be false *)
+            
+            apply not_true_iff_false in Hb.
+
+            rewrite andb_true_iff in Hb.
+            
+            apply Classical_Prop.not_and_or in Hb.
+            destruct Hb as [Hcount_not_eq | Hcs_not_eq].
+            - left. lia.
+            - right. destruct vs;auto.
+          }
+          destruct vs. all: try iFrame.
+          destruct Hcount_or_cs.
+          {
+            assert (send_count ≠ S recv_count) as Hsend_neq_Si.
+            {
+              (* First, establish i = recv_count from Helem *)
+              lia.
+            }
+           assert ((send_count =? (S recv_count)) = false).
+           {
+            rewrite Z.eqb_neq. lia.
+           }
+           unfold recv_ctr_frozen.
+           rewrite H3.
+           iFrame.
+          }
+          {
+           done. 
+          }
+      }
+    }
+    
+  - (* Case: channel is empty - count = 0 *)
+    wp_loadField.
+    
+    destruct (vs =?= Valid_closed) eqn: Hc.
+    
+    + (* Empty non-closed channel cases - similar for all non-closed states *)
+      (* Empty case - return false *)
+      assert (uint.Z (W64 0) <? uint.Z (W64 count) = false) as Hcond.
+      {
+        lia.
+      }
+      rewrite Hcond.
+      iNamed "Hpre".
+      assert (vs = Valid_closed) as Hcs_eq.
+      {
+        unfold valid_chan_state_eq in Hc.
+        destruct vs; try discriminate.
+        (* Only the Valid_closed case remains *)
+        reflexivity.
+      }
+      subst vs. iNamed "Hpre".
+      wp_pures. 
+      replace ((W64 5%nat)) with ((W64 5)) by word.
+      wp_pures. wp_load.
+      iSpecialize ("HΦ" $! true (zero_val chan_type) false).
+      (* Return failure due to empty channel *)
+      iNamed "HCloseTokPostClose".
+      iDestruct "HCloseTokPostClose" as "[Hauthset Hset]".
+      iDestruct (send_counter_elem with "[$HSndCtrAuth] [$HSc]") as "%Hag2".
+      iNamed "HRcvPerm". iDestruct "HRcvPerm" as "[HRct HRcvCloseTok]".
+      iDestruct ((own_closed_tok_post_close_pop_raw γ send_count γi Ri close_tok_names) with "[Hset Hauthset HRcvCloseTok]") as ">Hct".
+      {
+       iFrame.
+      }
+      wp_pures.
+      iModIntro.
+      iApply "HΦ".
+      unfold recv_ctr_frozen.
+      iFrame.
+      subst count. iFrame "#".
+      iFrame "count". iFrame. unfold isBufferedChan.
+      iDestruct "HCh" as (xs) "(HBuffSlice & %Hsize & %Hsizeinv & %HBuffCount & HPs & HQs)".
+      assert (send_count = recv_count) by lia.
+      replace recv_count with send_count. iFrame "#".
+       iDestruct "Hct" as "(Hset & Hauthset & Hri)".
+      iFrame. rewrite Z.eqb_refl. iFrame. 
+      iFrame. done.
+    
+    +  
+    assert (uint.Z (W64 0) <? uint.Z (W64 count) = false) as Hcond.
+    {
+      lia.
+    }
+    rewrite Hcond.
+      wp_if_destruct.
+      {
+        unfold valid_to_word in Heqb0. 
+        destruct vs. all: try done.
+      }
+      wp_load. wp_pures. iModIntro.
+      iApply "HΦ".
+       assert ((W64 count) = (W64 0)).
+      {
+        word.
+      }
+      rewrite H.
+      iFrame. done.
+      Unshelve.
+      done.
+Qed.
+      
+      
+(* Top-level channel invariant *)
+Definition isChan (ch: loc) (γ: chan_names) (chan_type: ty) 
+  (size: nat) (is_single_party: bool) (Psingle: Z -> val -> iProp Σ) 
+  (Pmulti: val -> iProp Σ) (Qsingle: Z -> iProp Σ) (Qmulti: iProp Σ) 
+  (R: nat -> iProp Σ): iProp Σ := 
+  ∃ (mu_l: loc) (buff: Slice.t),
+    "#mu" ∷ ch ↦[(Channel chan_type) :: "lock"]□ #mu_l ∗ 
+    "#buff" ∷ ch ↦[(Channel chan_type) :: "buffer"]□ (slice_val buff) ∗
+    "%Hbuffsize" ∷ ⌜#buff.(Slice.sz) = #(W64 size)⌝ ∗
+    "%Hchantyzero" ∷ ⌜has_zero chan_type⌝ ∗
+    "#Hlock" ∷ is_lock (nroot.@"Channel") (#mu_l) 
+      (isChanInner ch γ chan_type size is_single_party buff Psingle Pmulti Qsingle Qmulti R).
+
+(* Helper lemmas for working with channel states *)
+
+(* Lemma for checking if a channel is closed *)
+Lemma is_closed_state (vs: valid_chan_state) :
+  vs = Valid_closed <-> valid_to_word vs = CS_CLOSED_W.
+Proof.
+  split; intros H.
+  - subst vs. reflexivity.
+  - destruct vs; try (inversion H; fail).
+    reflexivity.
+Qed.
+
+(* Example helper lemma for closed channels *)
+Lemma closed_unbuff_eq (ch: loc) (send_count recv_count: nat) (v: val) 
+  (γ: chan_names) (chan_type: ty) (is_single_party: bool) 
+  (Psingle: Z -> val -> iProp Σ) (Pmulti: val -> iProp Σ) 
+  (Qsingle: Z -> iProp Σ) (Qmulti: iProp Σ) (R: nat -> iProp Σ):
+  isUnbufferedChan ch γ chan_type v Valid_closed is_single_party send_count recv_count
+  Psingle Pmulti Qsingle Qmulti R -∗ ⌜send_count = recv_count⌝.
+Proof.
+  iIntros "[%Heq _]". iPureIntro. exact Heq.
+Qed.
+
+(* Lemma for receiver_offer: Valid_start → Valid_receiver_ready *)
+Lemma receiver_offer (ch: loc) (γ: chan_names) (chan_type: ty) 
+  (v: val) (is_single_party: bool) (send_count: nat) (recv_count: nat) 
+  (Psingle: Z -> val -> iProp Σ) (Pmulti: val -> iProp Σ) 
+  (Qsingle: Z -> iProp Σ) (Qmulti: iProp Σ) (R Ri: nat -> iProp Σ)
+  (i: nat) (q: Qp):
+  (if is_single_party then q = 1%Qp else (q < 1)%Qp) ->
+  "HCh" ∷ isUnbufferedChan ch γ chan_type v Valid_start is_single_party send_count recv_count 
+    Psingle Pmulti Qsingle Qmulti R ∗ 
+  "HQ" ∷ Q is_single_party i Qsingle Qmulti ∗ 
+  "HRecvCtrAuth" ∷ own_recv_counter_auth γ recv_count false ∗ 
+  "HRecvPerm" ∷ own_recv_perm γ q i Ri 
+  ==∗ 
+  "HCh" ∷ isUnbufferedChan ch γ chan_type v Valid_receiver_ready is_single_party send_count recv_count 
+    Psingle Pmulti Qsingle Qmulti R ∗ 
+  "HRecvCtrAuth" ∷ own_recv_counter_auth γ recv_count false ∗ 
+  "HRecvPerm" ∷ own_recv_perm γ q i Ri ∗ 
+  "Hsttok" ∷ ghost_var γ.(unbuffered_state_tracker_name) (1/2)%Qp (false,v).
+Proof.
+  intros Hsp.
+  iIntros "IH". iNamed "IH". iNamed "HRecvPerm". 
+  iDestruct "HRecvPerm" as "[HRecvCtrFrag Hrct]".
+  
+  (* Split unbuffered channel into facts and resources *)
+  unfold isUnbufferedChan.
+  iDestruct "HCh" as "[HChanFacts HChanRes]".
+  
+  (* Extract state token from channel resources *)
+  destruct is_single_party.
+  { (* Single-party case *)
+    iDestruct "HChanRes" as "Hsttok".
+    (* Split the token *)
+    iDestruct ((exchange_token_split γ false v) with "[$Hsttok]") as ">[Hsttok1 Hsttok2]".
+    
+    (* Build assertion for counter elements *)
+    iAssert (own_recv_counter_auth γ recv_count false ∗ 
+             own_recv_counter_frag γ i q ∗ 
+             ⌜recv_count = i⌝)%I with "[HRecvCtrAuth HRecvCtrFrag]" as "(HRecvCtrAuth & HRecvCtrFrag & %Hispz)".
+    {
+      subst q.
+      iDestruct (recv_counter_elem with "[$HRecvCtrAuth] [$HRecvCtrFrag]") as "%Hag2".
+      iFrame. iPureIntro. done.
+    }
+    
+    (* Update state field *)
+    iModIntro.
+    
+    (* Reassemble resources *)
+    iFrame "HRecvCtrAuth".
+    iSplitL "HChanFacts HQ Hsttok1".
+    {
+      (* Rebuild channel invariant *)
+      iSplitL "HChanFacts".
+      { (* Facts - unchanged for this transition *) iExact "HChanFacts". }
+      { (* Resources for receiver_ready state *)
+        subst recv_count.
+        iFrame.
+      }
+    }
+    (* Frame remaining resources *)
+    iFrame "HRecvCtrFrag Hrct Hsttok2".
+  }
+  { (* Multi-party case - similar structure *)
+    iDestruct "HChanRes" as "Hsttok".
+    (* Split the token *)
+    iDestruct ((exchange_token_split γ false v) with "[$Hsttok]") as ">[Hsttok1 Hsttok2]".
+    
+    (* Build assertion for counter elements *)
+    iAssert (own_recv_counter_auth γ recv_count false ∗ 
+             own_recv_counter_frag γ i q ∗ 
+             ⌜i <= recv_count⌝%I)%I with "[HRecvCtrAuth HRecvCtrFrag]" as "(HRecvCtrAuth & HRecvCtrFrag & %Hispz)".
+    {
+      iDestruct (recv_counter_lower with "[$HRecvCtrAuth] [$HRecvCtrFrag]") as "%Hag2".
+      iFrame. iPureIntro. lia.
+    }
+    
+    (* Update state field *)
+    iModIntro.
+    
+    (* Reassemble resources *)
+    iFrame "HRecvCtrAuth".
+    iSplitL "HChanFacts HQ Hsttok1".
+    {
+      (* Rebuild channel invariant *)
+      iSplitL "HChanFacts".
+      { (* Facts - unchanged for this transition *) iExact "HChanFacts". }
+      { (* Resources for receiver_ready state *)
+        iFrame.
+        unfold Q.
+        destruct bool_decide eqn: Hbouter.
+        {
+          rewrite bool_decide_eq_true in Hbouter.
+          destruct bool_decide eqn: Hbinner.
+          {
+            done.
+          }
+          {
+            destruct i;first done.
+            done.
+          }
+        }
+        {
+          rewrite bool_decide_eq_false in Hbouter.
+          destruct bool_decide.
+          {
+            done.
+          }
+          iFrame.
+        }
+      }
+    }
+
+    (* Frame remaining resources *)
+    iFrame "HRecvCtrFrag Hrct Hsttok2".
+  }
+Qed.
+
+(* Lemma for receiver_complete: Valid_sender_ready → Valid_receiver_done *)
+Lemma receiver_complete (ch: loc) (γ: chan_names) (chan_type: ty) 
+  (v: val) (is_single_party: bool) (send_count: nat) (recv_count: nat) 
+  (Psingle: Z -> val -> iProp Σ) (Pmulti: val -> iProp Σ) 
+  (Qsingle: Z -> iProp Σ) (Qmulti: iProp Σ) (R Ri: nat -> iProp Σ)
+  (i: nat) (q: Qp):
+  (if is_single_party then q = 1%Qp else (q < 1)%Qp) ->
+  "HCh" ∷ isUnbufferedChan ch γ chan_type v Valid_sender_ready is_single_party send_count recv_count 
+    Psingle Pmulti Qsingle Qmulti R ∗ 
+  "HQ" ∷ Q is_single_party i Qsingle Qmulti ∗ 
+  "HRecvCtrAuth" ∷ own_recv_counter_auth γ recv_count false ∗ 
+  "HRecvPerm" ∷ own_recv_perm γ q i Ri 
+  ==∗ 
+  "HCh" ∷ isUnbufferedChan ch γ chan_type v Valid_receiver_done is_single_party send_count (S recv_count) 
+    Psingle Pmulti Qsingle Qmulti R ∗ 
+  "HRecvCtrAuth" ∷ own_recv_counter_auth γ (S recv_count) false ∗ 
+  "HRecvPerm" ∷ own_recv_perm γ q (S i) Ri.
+Proof.
+  intros Hsp. iIntros "Hpre".
+  iNamed "Hpre".
+  iNamed "HRecvPerm".
+  iDestruct "HRecvPerm" as "[HRecvCtrFrag Hrct]".
+  
+  (* Split unbuffered channel into facts and resources *)
+  unfold isUnbufferedChan.
+  iDestruct "HCh" as "[%HChanFacts HChanRes]".
+  
+  (* Extract state resources *)
+  iDestruct "HChanRes" as "(Hsttok & HP)".
+  
+  (* Build assertion for counter elements *)
+  iAssert (own_recv_counter_auth γ recv_count false ∗ 
+           own_recv_counter_frag γ i q ∗ 
+           ⌜if is_single_party then recv_count = i else i <= recv_count⌝%I)%I 
+    with "[HRecvCtrAuth HRecvCtrFrag]" as "(HRecvCtrAuth & HRecvCtrFrag & %Hispz)".
+  {
+    destruct is_single_party.
+    - subst q.
+      iDestruct (recv_counter_elem with "[$HRecvCtrAuth] [$HRecvCtrFrag]") as "%Hag2".
+      iFrame. iPureIntro. done.
+    - iDestruct (recv_counter_lower with "[$HRecvCtrAuth] [$HRecvCtrFrag]") as "%Hag2".
+      iFrame. iPureIntro. lia.
+  }
+  
+  (* Update counter *)
+  iDestruct (recv_counter_update γ recv_count i with "[$HRecvCtrAuth $HRecvCtrFrag]") 
+    as ">[HRecvCtrAuth HRecvCtrFrag]".
+  
+  (* Update state field *)
+  iModIntro.
+  
+  (* Reassemble resources *)
+  iFrame "HRecvCtrAuth".
+  iSplitL "Hsttok HQ".
+  {
+    (* Rebuild channel invariant *)
+    iSplitL "".
+    {
+      (* Update channel facts for new state *)
+      destruct is_single_party.
+      - subst q. subst recv_count.
+        (* Create facts for receiver_done state *)
+        iPureIntro. lia.
+        (* Other facts that might be needed... *)
+      - (* Similar for multi-party case *)
+        iPureIntro.
+        lia.
+        (* Other facts that might be needed... *)
+    }
+    {
+      (* Resources for receiver_done state *)
+      iFrame.
+      destruct is_single_party.
+      {
+       replace send_count with i by lia.
+       iFrame.
+      }
+      {
+      unfold Q.
+        destruct bool_decide eqn: Hbouter.
+        {
+          rewrite bool_decide_eq_true in Hbouter.
+          destruct bool_decide eqn: Hbinner.
+          {
+            done.
+          }
+          {
+            destruct i;first done.
+            done.
+          }
+        }
+        {
+          rewrite bool_decide_eq_false in Hbouter.
+          destruct bool_decide.
+          {
+            done.
+          }
+          iFrame. 
+        }
+    }
+  }
+}
+  (* Frame remaining resources *)
+  iFrame "HRecvCtrFrag Hrct".
+Qed.
+
+(* Lemma for receiver_rescind: Valid_receiver_ready → Valid_start *)
+Lemma receiver_rescind (ch: loc) (γ: chan_names) (chan_type: ty) 
+  (v: val) (is_single_party: bool) (send_count: nat) (recv_count: nat) 
+  (Psingle: Z -> val -> iProp Σ) (Pmulti: val -> iProp Σ) 
+  (Qsingle: Z -> iProp Σ) (Qmulti: iProp Σ) (R Ri: nat -> iProp Σ)
+  (i: nat) (q: Qp):
+  (if is_single_party then q = 1%Qp else (q < 1)%Qp) ->
+  "HCh" ∷ isUnbufferedChan ch γ chan_type v Valid_receiver_ready is_single_party send_count recv_count 
+    Psingle Pmulti Qsingle Qmulti R ∗ 
+  "HRecvCtrAuth" ∷ own_recv_counter_auth γ recv_count false ∗ 
+  "HRecvPerm" ∷ own_recv_perm γ q i Ri ∗  
+  "Hsttok'" ∷ exchange_token γ false v  
+  ==∗ 
+  "HCh" ∷ isUnbufferedChan ch γ chan_type v Valid_start is_single_party send_count recv_count 
+    Psingle Pmulti Qsingle Qmulti R ∗ 
+  "HQ" ∷ Q is_single_party i Qsingle Qmulti ∗ 
+  "HRecvCtrAuth" ∷ own_recv_counter_auth γ recv_count false ∗ 
+  "HRecvPerm" ∷ own_recv_perm γ q i Ri.
+Proof.
+  intros Hsp.
+  iIntros "Hpre". iNamed "Hpre".
+  iNamed "HRecvPerm".
+  iDestruct "HRecvPerm" as "[HRecvCtrFrag Hrct]".
+  
+  (* Split unbuffered channel into facts and resources *)
+  unfold isUnbufferedChan.
+  iDestruct "HCh" as "[HChanFacts HChanRes]".
+  
+  (* Extract state resources *)
+  iDestruct "HChanRes" as "(Hsttok & HQ)".
+  
+  (* Combine the tokens *)
+  unfold receiver_exchange_token. iNamed "Hsttok".
+  iDestruct ((exchange_token_combine γ) with "[$Hsttok $Hsttok']") as ">Hsttok".
+  
+  (* Build assertion for counter elements *)
+  iAssert (own_recv_counter_auth γ recv_count false ∗ 
+           own_recv_counter_frag γ i q ∗ 
+           ⌜if is_single_party then recv_count = i else i <= recv_count⌝%I)%I 
+    with "[HRecvCtrAuth HRecvCtrFrag]" as "(HRecvCtrAuth & HRecvCtrFrag & %Hispz)".
+  {
+    destruct is_single_party.
+    - subst q.
+      iDestruct (recv_counter_elem with "[$HRecvCtrAuth] [$HRecvCtrFrag]") as "%Hag2".
+      iFrame. done.
+    - iDestruct (recv_counter_lower with "[$HRecvCtrAuth] [$HRecvCtrFrag]") as "%Hag2".
+      iFrame. iPureIntro. lia.
+  }
+  
+  (* Update state field *)
+  iModIntro.
+  
+  destruct is_single_party.
+  {
+    subst recv_count. iFrame.
+  }
+  {
+    iFrame. 
+    unfold Q.
+        destruct bool_decide eqn: Hbouter.
+        {
+          rewrite bool_decide_eq_true in Hbouter.
+          destruct bool_decide eqn: Hbinner.
+          {
+            done.
+          }
+          {
+            lia.
+          }
+        }
+        {
+          rewrite bool_decide_eq_false in Hbouter.
+          destruct bool_decide.
+          {
+            done.
+          }
+          iFrame. 
+        }
+  }
+Qed.
+
+(* Lemma for receiver_complete_second: Valid_sender_done → Valid_start *)
+Lemma receiver_complete_second (ch: loc) (γ: chan_names) (chan_type: ty) 
+  (v: val) (is_single_party: bool) (send_count: nat) (recv_count: nat) 
+  (Psingle: Z -> val -> iProp Σ) (Pmulti: val -> iProp Σ) 
+  (Qsingle: Z -> iProp Σ) (Qmulti: iProp Σ) (R Ri: nat -> iProp Σ)
+  (i: nat) (q: Qp):
+  (if is_single_party then q = 1%Qp else (q < 1)%Qp) ->
+  "HCh" ∷ isUnbufferedChan ch γ chan_type v Valid_sender_done is_single_party send_count recv_count 
+    Psingle Pmulti Qsingle Qmulti R ∗ 
+  "HRecvCtrAuth" ∷ own_recv_counter_auth γ recv_count false ∗ 
+  "HRecvPerm" ∷ own_recv_perm γ q i Ri ∗  
+  "Hsttok'" ∷ exchange_token γ false v 
+  ==∗ 
+  "HCh" ∷ isUnbufferedChan ch γ chan_type v Valid_start is_single_party send_count (S recv_count) 
+    Psingle Pmulti Qsingle Qmulti R ∗ 
+  "HRecvCtrAuth" ∷ own_recv_counter_auth γ (S recv_count) false ∗ 
+  "HRecvPerm" ∷ own_recv_perm γ q (S i) Ri ∗ 
+  "HP" ∷ P is_single_party recv_count v Psingle Pmulti.
+Proof.
+  intros Hsp.
+  iIntros "Hpre". iNamed "Hpre".
+  iNamed "HRecvPerm".
+  iDestruct "HRecvPerm" as "[HRecvCtrFrag Hrct]".
+  
+  (* Split unbuffered channel into facts and resources *)
+  unfold isUnbufferedChan.
+  iDestruct "HCh" as "[%HChanFacts HChanRes]".
+  
+  (* Extract state resources *)
+  iDestruct "HChanRes" as "(Hsttok & HP)".
+  
+  (* Combine the tokens *)
+
+  unfold receiver_exchange_token. iNamed "Hsttok". 
+  iDestruct ((exchange_token_combine γ) with "[$Hsttok $Hsttok']") as ">Hsttok".
+  
+  (* Build assertion for counter elements *)
+  iAssert (own_recv_counter_auth γ recv_count false ∗ 
+           own_recv_counter_frag γ i q ∗ 
+           ⌜if is_single_party then recv_count = i else i <= recv_count⌝%I)%I 
+    with "[HRecvCtrAuth HRecvCtrFrag]" as "(HRecvCtrAuth & HRecvCtrFrag & %Hispz)".
+  {
+    destruct is_single_party.
+    - subst q.
+      iDestruct (recv_counter_elem with "[$HRecvCtrAuth] [$HRecvCtrFrag]") as "%Hag2".
+      iFrame. done.
+    - iDestruct (recv_counter_lower with "[$HRecvCtrAuth] [$HRecvCtrFrag]") as "%Hag2".
+      iFrame. iPureIntro. lia.
+  }
+  
+  (* Update counter *)
+  iDestruct (recv_counter_update γ recv_count i with "[$HRecvCtrAuth $HRecvCtrFrag]") 
+    as ">[HRecvCtrAuth HRecvCtrFrag]".
+  
+  (* Update state field *)
+  
+  (* Reassemble resources *)
+  iFrame. iPureIntro. lia.
+Qed.
+
+(* Define receiver transitions as a simple enum type *)
+Inductive receiver_transition : Type :=
+  | receiver_offer_trans : receiver_transition
+  | receiver_rescind_trans : receiver_transition
+  | receiver_complete_trans : receiver_transition
+  | receiver_complete_second_trans : receiver_transition.
+
+(* Define a relation that checks if a transition is valid between two states *)
+Definition is_valid_transition (tr: receiver_transition) (vs_old vs_new: valid_chan_state) : Prop :=
+  match tr, vs_old, vs_new with
+  | receiver_offer_trans, Valid_start, Valid_receiver_ready => True
+  | receiver_rescind_trans, Valid_receiver_ready, Valid_start => True
+  | receiver_complete_trans, Valid_sender_ready, Valid_receiver_done => True
+  | receiver_complete_second_trans, Valid_sender_done, Valid_start => True
+  | _, _, _ => False
+  end.
+
+(* Define how receiving count changes in each transition *)
+Definition receiver_recv_count_change (tr: receiver_transition) : nat :=
+  match tr with
+  | receiver_complete_trans => 1
+  | receiver_complete_second_trans => 1
+  | _ => 0
+  end.
+
+(* Define whether Q resource is needed for the transition *)
+Definition receiver_needs_Q (tr: receiver_transition) : bool :=
+  match tr with
+  | receiver_offer_trans => true
+  | receiver_complete_trans => true
+  | _ => false
+  end.
+
+(* Define whether additional token is needed for the transition *)
+Definition receiver_needs_token (tr: receiver_transition) : bool :=
+  match tr with
+  | receiver_rescind_trans => true
+  | receiver_complete_second_trans => true
+  | _ => false
+  end.
+
+(* Define whether P resource is produced by the transition *)
+Definition receiver_produces_P (tr: receiver_transition) : bool :=
+  match tr with
+  | receiver_complete_second_trans => true
+  | _ => false
+  end.
+
+(* Define whether token is produced by the transition *)
+Definition receiver_produces_token (tr: receiver_transition) : bool :=
+  match tr with
+  | receiver_offer_trans => true
+  | _ => false
+  end.
+
+  (* General receiver transition lemma *)
+Lemma receiver_transition_general (ch: loc) (γ: chan_names) (chan_type: ty) 
+(v: val) (vs_old vs_new: valid_chan_state) (tr: receiver_transition) 
+(is_single_party: bool) (send_count: nat) (recv_count: nat) 
+(Psingle: Z -> val -> iProp Σ) (Pmulti: val -> iProp Σ) 
+(Qsingle: Z -> iProp Σ) (Qmulti: iProp Σ) (R Ri: nat -> iProp Σ) 
+(i: nat) (q: Qp):
+(* Precondition: transition is valid between states *)
+is_valid_transition tr vs_old vs_new ->
+(* Ownership constraint *)
+(if is_single_party then q = 1%Qp else (q < 1)%Qp) ->
+(* Resources *)
+"HCh" ∷ isUnbufferedChan ch γ chan_type v vs_old is_single_party send_count recv_count 
+   Psingle Pmulti Qsingle Qmulti R ∗
+(if receiver_needs_Q tr then "HQ" ∷ Q is_single_party i Qsingle Qmulti else emp) ∗
+(if receiver_needs_token tr then "Hsttok'" ∷ receiver_exchange_token γ else emp) ∗
+"HRecvCtrAuth" ∷ own_recv_counter_auth γ recv_count false ∗ 
+"HRecvPerm" ∷ own_recv_perm γ q i Ri
+==∗ 
+(* Result resources *)
+"HCh" ∷ isUnbufferedChan ch γ chan_type v vs_new is_single_party send_count
+   (recv_count + receiver_recv_count_change tr) Psingle Pmulti Qsingle Qmulti R ∗
+(if receiver_produces_P tr then "HP" ∷ P is_single_party recv_count v Psingle Pmulti else emp) ∗
+(if negb (receiver_produces_P tr) && negb (receiver_needs_Q tr) 
+ then "HQ" ∷ Q is_single_party i Qsingle Qmulti else emp) ∗
+(if receiver_produces_token tr 
+ then "Hsttok" ∷ exchange_token γ false v else emp) ∗
+"HRecvCtrAuth" ∷ own_recv_counter_auth γ (recv_count + receiver_recv_count_change tr) false ∗ 
+"HRecvPerm" ∷ own_recv_perm γ q (i + receiver_recv_count_change tr) Ri.
+Proof.
+intros Hvalid Hsp.
+iIntros "Hpre".
+
+(* First, destruct by transition type to handle each case specifically *)
+destruct tr; simpl in *; unfold is_valid_transition in Hvalid;
+destruct vs_old, vs_new; try (exfalso; exact Hvalid).
+
+- (* Case: receiver_offer_trans - Valid_start → Valid_receiver_ready *)
+  simpl in *.
+  iNamed "Hpre". iDestruct "Hpre" as "[Hemp Hpre]".
+  iNamed "Hpre".
+  iNamed "HRecvPerm".
+  iDestruct "HRecvPerm" as "[HRecvCtrFrag Hrct]".
+  
+  (* Split unbuffered channel into facts and resources *)
+  unfold isUnbufferedChan.
+  iDestruct "HCh" as "[HChanFacts HChanRes]".
+  
+  (* Handle token splitting *)
+  iDestruct "HChanRes" as "Hsttok".
+  
+  iDestruct ((exchange_token_split γ false v) with "[$Hsttok]") as ">[Hsttok1 Hsttok2]".
+  
+  (* Handle counter verification *)
+  iAssert (own_recv_counter_auth γ recv_count false ∗ 
+           own_recv_counter_frag γ i q ∗ 
+           ⌜if is_single_party then recv_count = i else i <= recv_count⌝%I)%I
+    with "[HRecvCtrAuth HRecvCtrFrag]" as "(HRecvCtrAuth & HRecvCtrFrag & %Hispz)".
+  {
+    destruct is_single_party.
+    - subst q.
+      iDestruct (recv_counter_elem with "[$HRecvCtrAuth] [$HRecvCtrFrag]") as "%Hag2".
+      iFrame. iPureIntro. done.
+    - iDestruct (recv_counter_lower with "[$HRecvCtrAuth] [$HRecvCtrFrag]") as "%Hag2".
+      iFrame. iPureIntro. lia.
+  }
+  
+  (* Finalize *)
+  iModIntro.
+  replace (recv_count + 0)%nat with recv_count by lia.
+  replace (i + 0)%nat with i by lia.
+  iFrame "HRecvCtrAuth".
+  
+  (* Rebuild channel invariant *)
+  iSplitL "HChanFacts HQ Hsttok1".
+  {
+    iSplitL "HChanFacts".
+    { iExact "HChanFacts". }
+    { 
+      destruct is_single_party.
+      - subst recv_count. iFrame.
+      - iFrame.
+        unfold Q.
+        destruct bool_decide eqn:Hbouter.
+        {
+          rewrite bool_decide_eq_true in Hbouter.
+          destruct bool_decide; try lia.  
+        } 
+        rewrite bool_decide_eq_false in Hbouter.
+        destruct bool_decide; try done.
+    }
+  }
+  
+  (* Frame remaining resources *)
+  iFrame "HRecvCtrFrag Hrct Hsttok2".
+
+- (* Case: receiver_rescind_trans - Valid_receiver_ready → Valid_start *)
+  simpl in *.
+  iNamed "Hpre". iDestruct "Hpre" as "[Hemp Hpre]".
+  iNamed "Hpre".
+  iNamed "HRecvPerm".
+  iDestruct "HRecvPerm" as "[HRecvCtrFrag Hrct]".
+  
+  (* Split unbuffered channel into facts and resources *)
+  unfold isUnbufferedChan.
+  iDestruct "HCh" as "[HChanFacts HChanRes]".
+  
+  (* Extract state resources *)
+  iDestruct "HChanRes" as "(Hsttok & HQ')".
+  
+  (* Combine the tokens *)
+  iDestruct ((receiver_exchange_token_combine γ) with "[$Hsttok $Hsttok']") as ">Hsttok".
+  
+  (* Handle counter verification *)
+  iAssert (own_recv_counter_auth γ recv_count false ∗ 
+           own_recv_counter_frag γ i q ∗ 
+           ⌜if is_single_party then recv_count = i else i <= recv_count⌝%I)%I
+    with "[HRecvCtrAuth HRecvCtrFrag]" as "(HRecvCtrAuth & HRecvCtrFrag & %Hispz)".
+  {
+    destruct is_single_party.
+    - subst q.
+      iDestruct (recv_counter_elem with "[$HRecvCtrAuth] [$HRecvCtrFrag]") as "%Hag2".
+      iFrame. iPureIntro. done.
+    - iDestruct (recv_counter_lower with "[$HRecvCtrAuth] [$HRecvCtrFrag]") as "%Hag2".
+      iFrame. iPureIntro. lia.
+  }
+  
+  (* Finalize *)
+  iModIntro.
+  
+  (* Rebuild channel invariant *)
+  iSplitL "HChanFacts Hsttok".
+  {
+    iSplitL "HChanFacts".
+    { replace (recv_count + 0)%nat with recv_count by lia. iExact "HChanFacts". }
+    { iFrame "Hsttok". }
+  }
+  
+  (* Frame remaining resources and handle Q *)
+  destruct is_single_party.
+  + subst recv_count. iFrame. replace (i + 0)%nat with i by lia. iFrame.
+  + replace (recv_count + 0)%nat with recv_count by lia. 
+    (* Handle Q for multi-party case *)
+    unfold Q.
+    destruct bool_decide eqn:Hbouter; try done.
+    {
+    rewrite bool_decide_eq_true in Hbouter.
+    destruct bool_decide; try lia.
+    }
+    rewrite bool_decide_eq_false in Hbouter.
+    destruct bool_decide; try lia.
+    {
+     iFrame. replace (i + 0)%nat with i by lia. iFrame. 
+    }
+    iFrame. replace (i + 0)%nat with i by lia. done. 
+
+- (* Case: receiver_complete_trans - Valid_sender_ready → Valid_receiver_done *)
+  simpl in *.
+  iNamed "Hpre". iDestruct "Hpre" as "[Hemp Hpre]".
+  iNamed "Hpre".
+  iNamed "HRecvPerm".
+  iDestruct "HRecvPerm" as "[HRecvCtrFrag Hrct]".
+  
+  (* Split unbuffered channel into facts and resources *)
+  unfold isUnbufferedChan.
+  iDestruct "HCh" as "[%HChanFacts HChanRes]".
+  
+  (* Extract state resources *)
+  iDestruct "HChanRes" as "(Hsttok & HP)".
+  
+  (* Handle counter verification and update *)
+  iAssert (own_recv_counter_auth γ recv_count false ∗ 
+           own_recv_counter_frag γ i q ∗ 
+           ⌜if is_single_party then recv_count = i else i <= recv_count⌝%I)%I
+    with "[HRecvCtrAuth HRecvCtrFrag]" as "(HRecvCtrAuth & HRecvCtrFrag & %Hispz)".
+  {
+    destruct is_single_party.
+    - subst q.
+      iDestruct (recv_counter_elem with "[$HRecvCtrAuth] [$HRecvCtrFrag]") as "%Hag2".
+      iFrame. iPureIntro. done.
+    - iDestruct (recv_counter_lower with "[$HRecvCtrAuth] [$HRecvCtrFrag]") as "%Hag2".
+      iFrame. iPureIntro. lia.
+  }
+  
+  (* Update counter *)
+  iDestruct (recv_counter_update γ recv_count i with "[$HRecvCtrAuth $HRecvCtrFrag]") 
+    as ">[HRecvCtrAuth HRecvCtrFrag]".
+  
+  (* Finalize *)
+  iModIntro.
+  replace (S recv_count) with (recv_count + 1)%nat by lia.
+replace (S i) with (i + 1)%nat by lia.
+  iFrame "HRecvCtrAuth".
+  
+  (* Rebuild channel invariant *)
+  iSplitL "Hsttok HQ".
+  {
+    iSplitL "".
+    {
+      (* Update facts for new state *)
+      destruct is_single_party.
+      - subst q. subst recv_count. iPureIntro. lia.
+      - iPureIntro. lia.
+    }
+    {
+      (* Resources for receiver_done state *)
+      iFrame.
+      destruct is_single_party.
+      - replace send_count with i by lia. done.
+      - unfold Q.
+        destruct bool_decide eqn:Hbouter.
+        {
+          rewrite bool_decide_eq_true in Hbouter.
+          destruct bool_decide; try done.
+          lia.
+        }
+        rewrite bool_decide_eq_false in Hbouter.
+        destruct bool_decide; try done.
+    }
+  }
+  
+  (* Frame remaining resources *)
+  iFrame "HRecvCtrFrag Hrct".
+
+- (* Case: receiver_complete_second_trans - Valid_sender_done → Valid_start *)
+  simpl in *.
+  iNamed "Hpre". iDestruct "Hpre" as "[Hemp Hpre]".
+  iNamed "Hpre".
+  iNamed "HRecvPerm".
+  iDestruct "HRecvPerm" as "[HRecvCtrFrag Hrct]".
+  
+  (* Split unbuffered channel into facts and resources *)
+  unfold isUnbufferedChan.
+  iDestruct "HCh" as "[%HChanFacts HChanRes]".
+  
+  (* Extract state resources *)
+  iDestruct "HChanRes" as "(Hsttok & HP')".
+  
+  (* Combine the tokens *)
+  iDestruct ((receiver_exchange_token_combine γ) with "[$Hsttok $Hsttok']") as ">Hsttok".
+  
+  (* Handle counter verification and update *)
+  iAssert (own_recv_counter_auth γ recv_count false ∗ 
+           own_recv_counter_frag γ i q ∗ 
+           ⌜if is_single_party then recv_count = i else i <= recv_count⌝%I)%I
+    with "[HRecvCtrAuth HRecvCtrFrag]" as "(HRecvCtrAuth & HRecvCtrFrag & %Hispz)".
+  {
+    destruct is_single_party.
+    - subst q.
+      iDestruct (recv_counter_elem with "[$HRecvCtrAuth] [$HRecvCtrFrag]") as "%Hag2".
+      iFrame. iPureIntro. done.
+    - iDestruct (recv_counter_lower with "[$HRecvCtrAuth] [$HRecvCtrFrag]") as "%Hag2".
+      iFrame. iPureIntro. lia.
+  }
+  
+  (* Update counter *)
+  iDestruct (recv_counter_update γ recv_count i with "[$HRecvCtrAuth $HRecvCtrFrag]") 
+    as ">[HRecvCtrAuth HRecvCtrFrag]".
+  
+  (* Finalize *)
+  iModIntro.
+  
+  (* Rebuild resources *)
+  iSplitL "Hsttok".
+  {
+    iSplitL "".
+    { iPureIntro. lia. }
+    { iFrame "Hsttok". }
+  }
+  iFrame.
+  replace (S recv_count) with (recv_count + 1)%nat by lia.
+replace (S i) with (i + 1)%nat by lia.
+  iFrame.
+Qed.
+
+(* Define word constants for receiver results to match Go implementation *)
+Definition RECEIVER_COMPLETED_WITH_SENDER_W : w64 := W64 0.
+Definition RECEIVER_MADE_OFFER_W : w64 := W64 1.
+Definition RECEIVER_OBSERVED_CLOSED_W : w64 := W64 2.
+Definition RECEIVER_CANNOT_PROCEED_W : w64 := W64 3.
+
+(* Define result type for better type safety and readability *)
+Inductive receiver_result := 
+  | ReceiverCompletedWithSender
+  | ReceiverMadeOffer
+  | ReceiverObservedClosed
+  | ReceiverCannotProceed.
+
+(* Conversion function from result type to word representation *)
+Definition result_to_word (res: receiver_result) : w64 := 
+  match res with
+    | ReceiverCompletedWithSender => RECEIVER_COMPLETED_WITH_SENDER_W
+    | ReceiverMadeOffer => RECEIVER_MADE_OFFER_W
+    | ReceiverObservedClosed => RECEIVER_OBSERVED_CLOSED_W
+    | ReceiverCannotProceed => RECEIVER_CANNOT_PROCEED_W
+  end.
+
+(* Define word constants for offer results to match Go implementation *)
+Definition OFFER_RESCINDED_W : w64 := W64 0.
+Definition COMPLETED_EXCHANGE_W : w64 := W64 1.
+Definition CLOSE_INTERRUPTED_OFFER_W : w64 := W64 2.
+
+(* Define result type for better type safety and readability *)
+Inductive rescind_result := 
+  | OfferRescinded
+  | CompletedExchange
+  | CloseInterruptedOffer.
+
+(* Conversion function from result type to word representation *)
+Definition rescind_to_word (res: rescind_result) : w64 := 
+  match res with
+    | OfferRescinded => OFFER_RESCINDED_W
+    | CompletedExchange => COMPLETED_EXCHANGE_W
+    | CloseInterruptedOffer => CLOSE_INTERRUPTED_OFFER_W
+  end.
+
+  Lemma wp_Channel__ReceiverCompleteOrRescindOffer (ch: loc) (i: nat) (q: Qp) (γ: chan_names) 
+  (chan_type: ty) (buff: Slice.t) (v: val) (send_count: nat) (recv_count: nat) 
+  (vs: valid_chan_state) (size: nat) (is_single_party: bool) 
+  (Psingle: (Z -> val -> iProp Σ)) (Pmulti: (val -> iProp Σ)) 
+  (Qsingle: (Z -> iProp Σ)) (Qmulti: iProp Σ) (R Ri: nat -> iProp Σ):
+(if is_single_party then q = 1%Qp else (q < 1)%Qp) ->
+(#buff.(Slice.sz) = #(W64 0)) ->
+(vs = Valid_receiver_ready \/ vs = Valid_sender_done \/ vs = Valid_closed) ->
+{{{ 
+  "value" ∷ ch ↦[(Channel chan_type) :: "v"] v ∗ 
+  "HCh" ∷ isUnbufferedChan ch γ chan_type v vs is_single_party send_count recv_count Psingle 
+    Pmulti Qsingle Qmulti R ∗ 
+  "chan_state" ∷ ch ↦[(Channel chan_type) :: "state"] #(valid_to_word vs) ∗
+  "HRecvCtrAuth" ∷ own_recv_counter_auth γ recv_count (recv_ctr_frozen vs send_count recv_count) ∗
+  (if (vs =?= Valid_receiver_ready) || (vs =?= Valid_sender_done)
+   then "Hsttok" ∷ exchange_token γ false v
+   else emp) ∗
+  "HRecvPerm" ∷ own_recv_perm γ q i Ri ∗ 
+  "HCloseTokPostClose" ∷ 
+  if (vs =?= Valid_closed)
+  then (∃ (n:nat) (close_tok_names: gset gname),
+  "Hnameset" ∷  own_closed_tok_post_close γ n close_tok_names ∗ 
+ "Hsc" ∷ own_send_counter_frag γ recv_count 1 ∗ 
+  "#HSndCtrAuth" ∷ own_send_counter_auth γ n true 
+  ) else emp
+   
+}}}
+Channel__ReceiverCompleteOrRescindOffer chan_type #ch
+{{{ (res: rescind_result), RET #(rescind_to_word res);
+  match vs, res with
+  | Valid_receiver_ready, OfferRescinded =>
+      "value" ∷ ch ↦[(Channel chan_type) :: "v"] v ∗ 
+      "HCh" ∷ isUnbufferedChan ch γ chan_type v Valid_start is_single_party send_count recv_count Psingle 
+        Pmulti Qsingle Qmulti R ∗ 
+      "chan_state" ∷ ch ↦[(Channel chan_type) :: "state"] #(valid_to_word Valid_start) ∗
+      "HRecvCtrAuth" ∷ own_recv_counter_auth γ recv_count false ∗ 
+      "HRecvPerm" ∷ own_recv_perm γ q i Ri ∗
+      "HQ" ∷ Q is_single_party i Qsingle Qmulti
+      
+  | Valid_sender_done, CompletedExchange =>
+      "value" ∷ ch ↦[(Channel chan_type) :: "v"] v ∗ 
+      "HCh" ∷ isUnbufferedChan ch γ chan_type v Valid_start is_single_party send_count (recv_count + 1) Psingle 
+        Pmulti Qsingle Qmulti R ∗ 
+      "chan_state" ∷ ch ↦[(Channel chan_type) :: "state"] #(valid_to_word Valid_start) ∗
+      "HRecvCtrAuth" ∷ own_recv_counter_auth γ (recv_count + 1) false ∗ 
+      "HRecvPerm" ∷ own_recv_perm γ q (i + 1) Ri ∗
+      "HP" ∷ P is_single_party recv_count v Psingle Pmulti
+      
+  | Valid_closed, CloseInterruptedOffer =>
+      "value" ∷ ch ↦[(Channel chan_type) :: "v"] v ∗
+      "chan_state" ∷ ch ↦[(Channel chan_type) :: "state"] #(valid_to_word Valid_closed) ∗
+      (* Resources for closed channel case *)
+      own_recv_counter_frag γ i q ∗
+      (∃ n: nat, Ri n ∗ own_send_counter_auth γ n true ∗ own_recv_counter_auth γ n true)
+      
+  | _, _ =>
+      False
+  end
+}}}.
+Proof.
+intros Hvt Hbuff_zero Hvs.
+iIntros (Φ) "Hpre HΦ".
+iNamed "Hpre".
+
+wp_rec. wp_pures.
+
+(* Load current state *)
+wp_apply (wp_loadField with "chan_state").
+iIntros "chan_state".
+wp_pures.
+
+(* Cases based on current state *)
+destruct vs.
+
+- destruct Hvs as [Hvs | [Hvs | Hvs]];done.
+- wp_auto. 
+  (* Valid_receiver_ready case: Can rescind offer *)
+  
+  (* Apply transition *)
+  simpl. 
+  iNamed "Hpre".
+  iNamed "HRecvPerm".
+  iDestruct "HRecvPerm" as "[HRecvCtrFrag Hrct]".
+  
+  (* Set up counter verification *)
+  iAssert (own_recv_counter_auth γ recv_count false ∗ 
+           own_recv_counter_frag γ i q ∗ 
+           ⌜if is_single_party then recv_count = i else i <= recv_count⌝%I)%I
+    with "[HRecvCtrAuth HRecvCtrFrag]" as "(HRecvCtrAuth & HRecvCtrFrag & %Hispz)".
+  {
+    destruct is_single_party.
+    {
+      subst q.  
+      iDestruct (recv_counter_elem with "[$HRecvCtrAuth] [$HRecvCtrFrag]") as "%Hag2".
+      iFrame. done.
+    }
+    {
+      iDestruct (recv_counter_lower with "[$HRecvCtrAuth] [$HRecvCtrFrag]") as "%Hag2".
+      iFrame. iPureIntro. lia.
+    }
+  }
+  
+  (* Apply transition using the general lemma *)
+  iMod (receiver_transition_general ch γ chan_type v Valid_receiver_ready Valid_start
+         receiver_rescind_trans is_single_party send_count recv_count
+         Psingle Pmulti Qsingle Qmulti R Ri i q
+         with "[HCh HRecvCtrAuth HRecvCtrFrag Hrct Hsttok]") as 
+         "(HCh & HQ & HRecvCtrAuth & HRecvPerm)".
+  { apply I. }
+  { exact Hvt. }
+  { simpl. iFrame.
+    unfold isUnbufferedChan.
+    unfold chan_state_resources.
+    iDestruct "HCh" as "(%Hcsf & Hgv & HQ)".
+    iFrame. done.
+  }
+  
+  (* Return result *)
+  iModIntro. simpl. 
+  iSpecialize ("HΦ" $! OfferRescinded).
+  iApply "HΦ". 
+  replace (i + 0)%nat with i by lia.
+  replace (recv_count + 0)%nat with recv_count by lia.
+  iDestruct "HRecvPerm" as "(Hemp & Hrcauth & Hrcp)".
+  iFrame. 
+  
+- (* Valid_sender_ready case: Invalid state *)
+  destruct Hvs as [Hvs | [Hvs | Hvs]];done.
+  
+- destruct Hvs as [Hvs | [Hvs | Hvs]];done.
+  
+- (* Valid_sender_done case: Can complete exchange *)
+  wp_auto.
+  
+  (* Complete exchange: sender_done → start *)
+  simpl. iNamed "Hpre". 
+  
+  (* Apply transition *)
+  iNamed "HRecvPerm".
+  iDestruct "HRecvPerm" as "[HRecvCtrFrag Hrct]".
+  
+  (* Set up counter verification *)
+  iAssert (own_recv_counter_auth γ recv_count false ∗ 
+           own_recv_counter_frag γ i q ∗ 
+           ⌜if is_single_party then recv_count = i else i <= recv_count⌝%I)%I
+    with "[HRecvCtrAuth HRecvCtrFrag]" as "(HRecvCtrAuth & HRecvCtrFrag & %Hispz)".
+  {
+    destruct is_single_party.
+    {
+      subst q.  
+      iDestruct (recv_counter_elem with "[$HRecvCtrAuth] [$HRecvCtrFrag]") as "%Hag2".
+      iFrame. done.
+    }
+    {
+      iDestruct (recv_counter_lower with "[$HRecvCtrAuth] [$HRecvCtrFrag]") as "%Hag2".
+      iFrame. iPureIntro. lia.
+    }
+  }
+  
+  (* Apply transition using the general lemma *)
+  iMod (receiver_transition_general ch γ chan_type v Valid_sender_done Valid_start
+  receiver_complete_second_trans is_single_party send_count recv_count
+  Psingle Pmulti Qsingle Qmulti R Ri i q 
+  with "[HCh HRecvCtrAuth HRecvCtrFrag Hrct Hsttok]") as 
+  "(HCh & HP & _ & _ & HRecvCtrAuth & HRecvPerm)".
+  { apply I. }
+  { exact Hvt. }
+  { 
+    iNamed "HCh".
+    iFrame. 
+    destruct is_single_party.
+    {
+      iFrame. simpl. iDestruct "HCh" as "(%Hvt2 & Hsttok & HP)".
+      iFrame. done.
+    }
+    {
+      iDestruct "HCh" as "(%Hvt2 & Hsttok & HP)".
+      iFrame. done.
+    }
+  }
+  
+  (* Return result *)
+  iModIntro. 
+  iSpecialize ("HΦ" $! CompletedExchange).
+  iApply "HΦ".
+  iFrame.
+  
+- (* Valid_closed case: Channel is closed *)
+  simpl. iDestruct "Hpre" as "[_ HRecvPerm]".
+  iNamed "HRecvPerm". iNamed "HRecvPerm".
+  
+  (* Handle closed channel case *)
+  iDestruct "HRecvPerm" as "[HRecvCtrFrag Hrct]".
+  
+  (* Return result *)
+  iSpecialize ("HΦ" $! CloseInterruptedOffer).
+  
+  (* Extract from invariant *)
+  unfold isUnbufferedChan.
+  iDestruct "HCh" as "[%HChanFacts HChanStateResources]".
+  iFrame. iNamed "HCloseTokPostClose". 
+  unfold own_closed_tok_post_close.
+  iDestruct "Hnameset" as "[Hauthset Hset]".
+  iDestruct (send_counter_elem with "[$HSndCtrAuth] [$Hsc]") as "%Hag2".
+  iDestruct ((own_closed_tok_post_close_pop_raw γ n γi Ri close_tok_names) with "[Hset Hauthset Hrct]") as ">(Hset & Hauthset & Hri)".
+  {
+   iFrame.
+  }
+  wp_pures.
+  iDestruct (send_counter_elem with "[$HSndCtrAuth] [$Hsc]") as "%Hag3".
+
+  iApply "HΦ".
+  iFrame "value chan_state HRecvCtrFrag".
+
+  iModIntro. 
+  iExists recv_count. iFrame "#". replace recv_count with n. iFrame. iFrame "#".
+  replace ((send_count =? n)) with true by lia. iFrame.
+Qed.
+Lemma wp_Channel__ReceiverCompleteOrOffer (ch: loc) (i: nat) (q: Qp) (γ: chan_names) (chan_type: ty) (buff: Slice.t)
+  (v: val) (send_count: nat) (recv_count: nat) (vs: valid_chan_state)
+  (size: nat) (is_single_party: bool) (Psingle: (Z -> val -> iProp Σ)) (Pmulti: (val -> iProp Σ)) 
+  (Qsingle: (Z -> iProp Σ)) (Qmulti: iProp Σ) (R Ri: nat -> iProp Σ):
+(if is_single_party then q = 1%Qp else (q < 1)%Qp) ->
+(#buff.(Slice.sz) = #(W64 0)) ->
+{{{ 
+  "value" ∷ ch ↦[(Channel chan_type) :: "v"] v ∗ 
+  "HCh" ∷ isUnbufferedChan ch γ chan_type v vs is_single_party send_count recv_count Psingle 
+    Pmulti Qsingle Qmulti R ∗ 
+  "chan_state" ∷ ch ↦[(Channel chan_type) :: "state"] #(valid_to_word vs) ∗
+  "HQ" ∷ Q is_single_party i Qsingle Qmulti ∗ 
+  "HRecvCtrAuth" ∷ own_recv_counter_auth γ recv_count (recv_ctr_frozen vs send_count recv_count) ∗ 
+  "HRecvPerm" ∷ own_recv_perm γ q i Ri 
+}}}
+Channel__ReceiverCompleteOrOffer chan_type #ch
+{{{ (res: receiver_result), RET #(result_to_word res);
+  match res with 
+  | ReceiverCompletedWithSender =>
+    "value" ∷ ch ↦[(Channel chan_type) :: "v"] v ∗ 
+    "HCh" ∷ isUnbufferedChan ch γ chan_type v Valid_receiver_done is_single_party send_count (recv_count + 1) Psingle 
+      Pmulti Qsingle Qmulti R ∗ 
+    "chan_state" ∷ ch ↦[(Channel chan_type) :: "state"] #(valid_to_word Valid_receiver_done) ∗
+    "HRecvCtrAuth" ∷ own_recv_counter_auth γ (recv_count + 1) false ∗ 
+    "HRecvPerm" ∷ own_recv_perm γ q (i + 1) Ri 
+  | ReceiverMadeOffer =>
+    "value" ∷ ch ↦[(Channel chan_type) :: "v"] v ∗ 
+    "HCh" ∷ isUnbufferedChan ch γ chan_type v Valid_receiver_ready is_single_party send_count recv_count Psingle 
+      Pmulti Qsingle Qmulti R ∗ 
+    "chan_state" ∷ ch ↦[(Channel chan_type) :: "state"] #(valid_to_word Valid_receiver_ready) ∗
+    "HRecvCtrAuth" ∷ own_recv_counter_auth γ recv_count false ∗ 
+    "Hsttok" ∷ receiver_exchange_token γ ∗  
+    "HRecvPerm" ∷ own_recv_perm γ q i Ri 
+  | ReceiverObservedClosed =>
+    "chan_state" ∷ ch ↦[(Channel chan_type) :: "state"] #(valid_to_word Valid_closed)
+  | ReceiverCannotProceed =>
+    "value" ∷ ch ↦[(Channel chan_type) :: "v"] v ∗ 
+    "HCh" ∷ isUnbufferedChan ch γ chan_type v vs is_single_party send_count recv_count Psingle 
+      Pmulti Qsingle Qmulti R ∗ 
+    "chan_state" ∷ ch ↦[(Channel chan_type) :: "state"] #(valid_to_word vs) ∗
+    "HQ" ∷ Q is_single_party i Qsingle Qmulti ∗ 
+    "HRecvCtrAuth" ∷ own_recv_counter_auth γ recv_count false ∗ 
+    "HRecvPerm" ∷ own_recv_perm γ q i Ri 
+  end
+}}}.
+Proof.
+  intros Hsp Hbuffsz.
+  iIntros (Φ) "Hpre HΦ".
+  iNamed "Hpre".
+  
+  wp_rec. wp_pures.
+  
+  (* Cases based on current state *)
+  destruct vs.
+  
+  - (* Valid_start case: Can make an offer *)
+    wp_auto.
+    
+    (* Apply transition *)
+    iNamed "HRecvPerm".
+    iDestruct "HRecvPerm" as "[HRecvCtrFrag Hrct]".
+    
+    (* Apply transition using the general lemma *)
+    iMod (receiver_transition_general ch γ chan_type v Valid_start Valid_receiver_ready 
+           receiver_offer_trans is_single_party send_count recv_count
+           Psingle Pmulti Qsingle Qmulti R Ri i q
+           with "[HCh HQ HRecvCtrAuth HRecvCtrFrag Hrct]") as 
+           "(HCh & _ & _ & Hsttok & HRecStuff)".
+    { apply I. }
+    { exact Hsp. }
+    { iFrame. }
+    iNamed "HRecStuff".
+    iNamed "HCh".
+    
+    iModIntro.
+  iSpecialize ("HΦ" $! ReceiverMadeOffer).
+    iApply "HΦ". 
+    replace (recv_count + 0)%nat with recv_count by lia.
+    replace (i + 0)%nat with i by lia.
+    iFrame. iDestruct "HCh" as "[%Hfacts Hresources]".
+    simpl.
+    iDestruct "Hresources" as "[Htok HQ]".
+    iFrame.
+    iFrame. simpl in Hfacts.
+    replace (i + 0)%nat with i by lia.
+    replace (recv_count + 0)%nat with recv_count by lia.
+    iFrame. unfold receiver_exchange_token. iPureIntro. lia.
+
+    
+  - (* Valid_receiver_ready case: Cannot proceed *)
+    wp_auto. 
+    iSpecialize ("HΦ" $! ReceiverCannotProceed).
+    iApply "HΦ". 
+    iFrame.
+    iModIntro. done.
+    
+  - (* Valid_sender_ready case: Can complete receive *)
+    wp_auto.
+    
+    (* Apply transition *)
+    iNamed "HRecvPerm".
+    iDestruct "HRecvPerm" as "[HRecvCtrFrag Hrct]".
+    
+    (* Apply transition using the general lemma *)
+    iMod (receiver_transition_general ch γ chan_type v Valid_sender_ready Valid_receiver_done 
+           receiver_complete_trans is_single_party send_count recv_count
+           Psingle Pmulti Qsingle Qmulti R Ri i q
+           with "[HCh HQ HRecvCtrAuth HRecvCtrFrag Hrct]") as 
+           "(HCh & _ & _ & _ & HRecvCtrAuth & HRecvPerm)".
+    { apply I. }
+    { exact Hsp. }
+    { iFrame. }
+    
+    iModIntro.
+    iSpecialize ("HΦ" $! ReceiverCompletedWithSender).
+
+    iApply "HΦ". 
+    iFrame.
+    
+  - (* Valid_receiver_done case: Cannot proceed *)
+    wp_auto. 
+    iSpecialize ("HΦ" $! ReceiverCannotProceed).
+    iApply "HΦ". 
+    iFrame.
+    iModIntro. done.
+    
+  - (* Valid_sender_done case: Cannot proceed *)
+    wp_auto. 
+    iSpecialize ("HΦ" $! ReceiverCannotProceed).
+    iApply "HΦ". 
+    iFrame.
+    iModIntro. done.
+    
+  - (* Valid_closed case: Channel is closed *)
+    wp_auto.
+    iSpecialize ("HΦ" $! ReceiverObservedClosed).
+    iApply "HΦ". 
+    iFrame "chan_state".
+    iModIntro. done.
+Qed.
+(* Define word constants for sender results to match Go implementation *)
+Definition SENDER_COMPLETED_WITH_RECEIVER_W : w64 := W64 0.
+Definition SENDER_MADE_OFFER_W : w64 := W64 1.
+Definition SENDER_CANNOT_PROCEED_W : w64 := W64 2.
+
+(* Define result type for better type safety and readability *)
+Inductive sender_result := 
+  | SenderCompletedWithReceiver
+  | SenderMadeOffer
+  | SenderCannotProceed.
+
+(* Conversion function from result type to word representation *)
+Definition sender_result_to_word (res: sender_result) : w64 := 
+  match res with
+    | SenderCompletedWithReceiver => SENDER_COMPLETED_WITH_RECEIVER_W
+    | SenderMadeOffer => SENDER_MADE_OFFER_W
+    | SenderCannotProceed => SENDER_CANNOT_PROCEED_W
+  end.
+
+(* Define sender transitions as a simple enum type *)
+Inductive sender_transition : Type :=
+  | sender_offer_trans
+  | sender_complete_trans
+  | sender_rescind_trans
+  | sender_complete_second_trans.
+
+(* Define a relation that checks if a transition is valid between two states *)
+Definition is_valid_send_transition (tr: sender_transition) (vs_old vs_new: valid_chan_state) : Prop :=
+  match tr, vs_old, vs_new with
+  | sender_offer_trans, Valid_start, Valid_sender_ready => True
+  | sender_complete_trans, Valid_receiver_ready, Valid_sender_done => True
+  | sender_rescind_trans, Valid_sender_ready, Valid_start => True
+  | sender_complete_second_trans, Valid_receiver_done, Valid_start => True
+  | _, _, _ => False
+  end.
+
+(* Define how sending count changes in each transition *)
+Definition sender_send_count_change (tr: sender_transition) : nat :=
+  match tr with
+  | sender_complete_trans => 1
+  | sender_complete_second_trans => 1
+  | _ => 0
+  end.
+
+(* Define whether additional token is needed for the transition *)
+Definition sender_needs_token (tr: sender_transition) : bool :=
+  match tr with
+  | sender_rescind_trans => true
+  | sender_complete_second_trans => true
+  | _ => false
+  end.
+
+(* Define whether token is produced by the transition *)
+Definition sender_produces_token (tr: sender_transition) : bool :=
+  match tr with
+  | sender_offer_trans => true
+  | _ => false
+  end.
+
+(* Define whether P resource is needed for the transition *)
+Definition sender_needs_P (tr: sender_transition) : bool :=
+  match tr with
+  | sender_offer_trans => true
+  | sender_complete_trans => true
+  | _ => false
+  end.
+
+(* Define whether Q resource is produced by the transition *)
+Definition sender_produces_Q (tr: sender_transition) : bool :=
+  match tr with
+  | sender_complete_trans => true
+  | sender_complete_second_trans => true
+  | _ => false
+  end.
+
+(* General sender transition lemma *)
+Lemma sender_transition_general (ch: loc) (γ: chan_names) (chan_type: ty) 
+  (v vold: val) (vs_old vs_new: valid_chan_state) (tr: sender_transition) 
+  (is_single_party: bool) (send_count recv_count: nat) 
+  (Psingle: Z -> val -> iProp Σ) (Pmulti: val -> iProp Σ) 
+  (Qsingle: Z -> iProp Σ) (Qmulti: iProp Σ) (R Ri: nat -> iProp Σ) 
+  (i: nat) (q: Qp):
+  is_valid_send_transition tr vs_old vs_new ->
+  (if is_single_party then q = 1%Qp else (q < 1)%Qp) ->
+  val_ty v chan_type ->
+  (* Resources *)
+  "HCh" ∷ isUnbufferedChan ch γ chan_type vold vs_old is_single_party send_count recv_count 
+     Psingle Pmulti Qsingle Qmulti R ∗
+  (if sender_needs_token tr then "Hsttok'" ∷ exchange_token γ true v else emp ∗ "%Heqv'" ∷  ⌜vold = v ⌝) ∗
+  (if sender_needs_P tr then "HP" ∷ P is_single_party send_count v Psingle Pmulti else emp) ∗
+  "HSndCtrAuth" ∷ own_send_counter_auth γ send_count (send_ctr_frozen vs_old) ∗ 
+  "HSndPerm" ∷ own_send_counter_frag γ i q  
+  ==∗ 
+  (* Result resources *)
+  "HCh" ∷ isUnbufferedChan ch γ chan_type vold vs_new is_single_party 
+     (send_count + sender_send_count_change tr) recv_count
+     Psingle Pmulti Qsingle Qmulti R ∗
+  (if negb (sender_produces_Q tr) && negb (sender_needs_P tr) 
+  then "HP" ∷ P is_single_party send_count v Psingle Pmulti else emp ∗
+    
+  if sender_produces_token tr 
+   then "Hsttok" ∷ exchange_token γ  true v else emp) ∗ "%Heqv"  ∷ ⌜vold = v ⌝  ∗
+  (if sender_produces_Q tr 
+   then "HQ" ∷ Q is_single_party i Qsingle Qmulti else emp) ∗
+  "HSndCtrAuth" ∷ own_send_counter_auth γ (send_count + sender_send_count_change tr) 
+                                         (send_ctr_frozen vs_new) ∗ 
+  "HSndPerm" ∷ own_send_counter_frag γ (i + sender_send_count_change tr) q.
+Proof.
+  intros Hvalid Hsp Hvt.
+  iIntros "( HCh & Htok & HP & HSndCtrAuth & HSndPerm)".
+  
+  (* First, destruct by transition type to handle each case specifically *)
+  destruct tr; simpl in *; unfold is_valid_send_transition in Hvalid;
+  destruct vs_old, vs_new; try (exfalso; exact Hvalid).
+  
+  - (* Case: sender_offer_trans - Valid_start → Valid_sender_ready *)
+    simpl in *.
+    
+    (* Split unbuffered channel into facts and resources *)
+    unfold isUnbufferedChan.
+    iDestruct "HCh" as "[%HChanFacts HChanRes]".
+    
+    (* Extract state resources *)
+    iDestruct "HChanRes" as "Hsttok".
+    
+    (* Handle token splitting *)
+  iDestruct ((exchange_token_split γ true v) with "[$Hsttok]") as ">[Hsttok1 Hsttok2]".
+  iNamed "HSndPerm".
+    
+    (* Handle counter verification *)
+    iAssert (own_send_counter_auth γ send_count false ∗ 
+             own_send_counter_frag γ i q ∗ 
+             ⌜if is_single_party then send_count = i else i <= send_count⌝%I)%I
+      with "[HSndCtrAuth HSndPerm]" as "(HSndCtrAuth & HSndPerm & %Hispz)".
+    {
+      destruct is_single_party.
+      - subst q.
+        iDestruct (send_counter_elem with "[$HSndCtrAuth] [$HSndPerm]") as "%Hag2".
+        iFrame. iPureIntro. done.
+      - iDestruct (send_counter_lower with "[$HSndCtrAuth] [$HSndPerm]") as "%Hag2".
+        iFrame. iPureIntro. lia.
+    }
+    replace (send_count + 0)%nat with (send_count)%nat by lia.
+    replace (i + 0)%nat with i by lia.
+    
+    (* Finalize *)
+    iModIntro.
+    unfold chan_state_resources.
+
+    
+    (* Rebuild resources *)
+    iFrame. simpl. iDestruct "Htok" as "[Hemp %Heqv]". subst v. iFrame. done.
+    
+  - (* Case: sender_complete_trans - Valid_receiver_ready → Valid_sender_done *)
+    simpl in *.
+    
+    (* Split unbuffered channel into facts and resources *)
+    unfold isUnbufferedChan.
+    iDestruct "HCh" as "[%HChanFacts HChanRes]".
+    
+    (* Extract state resources *)
+    iDestruct "HChanRes" as "(Hsttok & HQ)".
+    
+    (* Handle counter verification and update *)
+    iAssert (own_send_counter_auth γ send_count false ∗ 
+             own_send_counter_frag γ i q ∗ 
+             ⌜if is_single_party then send_count = i else i <= send_count⌝%I)%I
+      with "[HSndCtrAuth HSndPerm]" as "(HSndCtrAuth & HSndPerm & %Hispz)".
+    {
+      destruct is_single_party.
+      - subst q.
+        iDestruct (send_counter_elem with "[$HSndCtrAuth] [$HSndPerm]") as "%Hag2".
+        iFrame. iPureIntro. done.
+      - iDestruct (send_counter_lower with "[$HSndCtrAuth] [$HSndPerm]") as "%Hag2".
+        iFrame. iPureIntro. lia.
+    }
+    
+    (* Update counter *)
+    iDestruct (send_counter_update γ send_count i with "[$HSndCtrAuth $HSndPerm]") 
+      as ">[HSndCtrAuth HSndPerm]".
+    
+    (* Finalize *)
+    iModIntro.
+    iDestruct "Htok" as "[Hemp %Heqv]". 
+    (* Rebuild resources *)
+    iFrame.
+    replace (send_count + 1)%nat with (S send_count)%nat by lia.
+    replace (i + 1)%nat with (S i) by lia.
+    iFrame. iNamed "HP". replace recv_count with send_count. iFrame.
+    destruct is_single_party.
+    {
+     subst i. iFrame.
+     iFrame. subst v. iFrame. done.
+    }
+    {
+      subst v.
+      iFrame.
+      unfold Q.
+      destruct (bool_decide (i < 0)%Z) eqn:?; simpl; [done|].
+      iFrame.
+       destruct bool_decide.
+       {
+        word.
+       }
+       destruct bool_decide eqn:?;simpl.
+       {
+        apply bool_decide_eq_true in Heqb0.
+        lia.
+       }
+       { 
+       iFrame. iPureIntro. done.
+       } 
+    }
+    
+  - (* Case: sender_rescind_trans - Valid_sender_ready → Valid_start *)
+    simpl in *.
+    
+    (* Split unbuffered channel into facts and resources *)
+    unfold isUnbufferedChan.
+    iDestruct "HCh" as "[%HChanFacts HChanRes]".
+    
+    (* Extract state resources *)
+    iDestruct "HChanRes" as "(Hsttok & HP')".
+  iDestruct ((exchange_token_agree) with "[$Hsttok] [$Htok]") as "%Heq".
+    
+    (* Combine the tokens *)
+  iDestruct ((exchange_token_combine) with "[$Hsttok $Htok]") as ">Hsttok".
+    
+    (* Handle counter verification *)
+    iAssert (own_send_counter_auth γ send_count false ∗ 
+             own_send_counter_frag γ i q ∗ 
+             ⌜if is_single_party then send_count = i else i <= send_count⌝%I)%I
+      with "[HSndCtrAuth HSndPerm]" as "(HSndCtrAuth & HSndPerm & %Hispz)".
+    {
+      destruct is_single_party.
+      - subst q.
+        iDestruct (send_counter_elem with "[$HSndCtrAuth] [$HSndPerm]") as "%Hag2".
+        iFrame. iPureIntro. done.
+      - iDestruct (send_counter_lower with "[$HSndCtrAuth] [$HSndPerm]") as "%Hag2".
+        iFrame. iPureIntro. lia.
+    }
+    
+    (* Finalize *)
+    iModIntro.
+    
+    (* Rebuild resources *)
+    replace (send_count + 0)%nat with (send_count)%nat by lia.
+    replace (i + 0)%nat with i by lia.
+    iFrame.
+    unfold chan_state_resources. iFrame.
+    destruct Heq as [Heq _].
+    rewrite Heq.
+    iFrame.
+    iPureIntro. destruct HChanFacts as [H1 H2]. done.
+    
+    
+  - (* Case: sender_complete_second_trans - Valid_receiver_done → Valid_start *)
+    simpl in *.
+    
+    (* Split unbuffered channel into facts and resources *)
+    unfold isUnbufferedChan.
+    iDestruct "HCh" as "[%HChanFacts HChanRes]".
+    
+    (* Extract state resources *)
+    iDestruct "HChanRes" as "(Hsttok & HQ)".
+    
+    (* Combine the tokens *)
+  iDestruct ((exchange_token_agree) with "[$Hsttok] [$Htok]") as "%Heq".
+  iDestruct ((exchange_token_combine γ) with "[$Hsttok $Htok]") as ">Hsttok".
+    
+    (* Handle counter verification *)
+    iAssert (own_send_counter_auth γ send_count false ∗ 
+             own_send_counter_frag γ i q ∗ 
+             ⌜if is_single_party then send_count = i else i <= send_count⌝%I)%I
+      with "[HSndCtrAuth HSndPerm]" as "(HSndCtrAuth & HSndPerm & %Hispz)".
+    {
+      destruct is_single_party.
+      - subst q.
+        iDestruct (send_counter_elem with "[$HSndCtrAuth] [$HSndPerm]") as "%Hag2".
+        iFrame. iPureIntro. done.
+      - iDestruct (send_counter_lower with "[$HSndCtrAuth] [$HSndPerm]") as "%Hag2".
+        iFrame. iPureIntro. lia.
+    }
+
+    iDestruct (send_counter_update γ send_count i with "[$HSndCtrAuth $HSndPerm]") 
+      as ">[HSndCtrAuth HSndPerm]".
+    
+    (* Finalize *)
+    iModIntro.
+    
+    (* Rebuild resources *)
+    iFrame .
+    
+    (* Rebuild channel invariant *)
+    iSplitL "".
+    {
+      iPureIntro. replace (send_count + 1)%nat with (S send_count) by lia.
+      done.
+    }
+    destruct is_single_party.
+    {
+      subst i. iFrame.
+      replace (send_count + 1)%nat with (S send_count) by lia.
+    iFrame. destruct Heq as [Heq _]. done.
+    }
+    {
+      unfold Q.
+      replace (i + 1)%nat with (S i) by lia.
+      replace (send_count + 1)%nat with (S send_count) by lia.
+      destruct (bool_decide (i < 0)%Z) eqn:?; simpl.
+      {
+       iFrame.  
+       iPureIntro. destruct Heq as [Heq _]. done.
+      }
+      iFrame.
+       destruct bool_decide.
+       {
+        word.
+       }
+       destruct bool_decide eqn:?;simpl.
+       {
+        apply bool_decide_eq_true in Heqb0.
+        lia.
+       }
+       destruct Heq as [Heq _].
+       iFrame.
+       done.
+    }
+Qed.
+
+Lemma sender_token_state_agree γ ch v vs send_count recv_count v0 chan_type
+  is_single_party Psingle Pmulti Qsingle Qmulti R :
+  vs ≠ Valid_closed ->
+  sender_exchange_token γ v -∗
+  isUnbufferedChan ch γ chan_type v0 vs is_single_party send_count recv_count 
+    Psingle Pmulti Qsingle Qmulti R -∗
+  ⌜(vs = Valid_sender_ready ∨ vs = Valid_receiver_done) ∧ v = v0⌝.
+Proof.
+  intros Hvs.
+  iIntros "Htok HChan".
+  unfold isUnbufferedChan, chan_state_resources.
+  iDestruct "HChan" as "[HChanFacts HChanRes]". unfold chan_state_facts.
+  
+  destruct vs.
+  
+  - (* Valid_start *)
+    iDestruct "HChanRes" as "Hfull".
+    unfold sender_exchange_token, exchange_token, full_exchange_token.
+    iDestruct (ghost_var_valid_2 with "[$Htok] [$Hfull]") as "%Hvalid".
+    (* Contradiction: can't have 1/2 + 1 = 1 *)
+    iPureIntro. destruct Hvalid as [H1 H2].
+    apply Qp.not_add_le_r in H1.
+    contradiction.
+    
+  - (* Valid_receiver_ready *)
+    iDestruct "HChanRes" as "[Hrec HQ]".
+    unfold sender_exchange_token, exchange_token, receiver_exchange_token.
+    iDestruct "Hrec" as (dummy_v) "Hrec".
+    iDestruct (ghost_var_valid_2 with "[$Htok] [$Hrec]") as "%Hvalid".
+    (* Contradiction: (true, v) ≠ (false, dummy_v) *)
+    iPureIntro.
+    destruct Hvalid as [_ Heq].
+    inversion Heq. 
+    
+  - (* Valid_sender_ready *)
+    iDestruct "HChanRes" as "[Hsnd HP]".
+    unfold sender_exchange_token.
+    iDestruct (ghost_var_agree with "[$Htok] [$Hsnd]") as "%Heq".
+    (* Success: v = v0 *)
+    iPureIntro. 
+    split; [left; reflexivity | injection Heq; intros; subst; reflexivity].
+    
+  - (* Valid_receiver_done *)
+    iDestruct "HChanRes" as "[Hsnd HQ]".
+    unfold sender_exchange_token.
+    iDestruct (ghost_var_agree with "[$Htok] [$Hsnd]") as "%Heq".
+    (* Success: v = v0 *)
+    iPureIntro.
+    split; [right; reflexivity | injection Heq; intros; subst; reflexivity].
+    
+  - (* Valid_sender_done *)
+    iDestruct "HChanRes" as "[Hrec HP]".
+    unfold sender_exchange_token, exchange_token, receiver_exchange_token.
+    iDestruct "Hrec" as (dummy_v) "Hrec".
+    iDestruct (ghost_var_valid_2 with "[$Htok] [$Hrec]") as "%Hvalid".
+    (* Contradiction: (true, v) ≠ (false, dummy_v) *)
+    iPureIntro.
+    destruct Hvalid as [_ Heq].
+    inversion Heq. 
+    
+  - done. (* Valid_closed *)
+    
+Qed.
+
+Lemma wp_Channel__SenderCheckOfferResult (ch: loc) (v: val) (γ: chan_names) (chan_type: ty) (buff: Slice.t)
+  (send_count: nat) (recv_count: nat) (vs: valid_chan_state)
+  (size: nat) (is_single_party: bool) (Psingle: (Z -> val -> iProp Σ)) (Pmulti: (val -> iProp Σ)) 
+  (Qsingle: (Z -> iProp Σ)) (Qmulti: iProp Σ) (R Ri: nat -> iProp Σ)
+  (i: nat) (q: Qp):
+  (#buff.(Slice.sz) = #(W64 0)) ->
+  (if is_single_party then q = 1%Qp else (q < 1)%Qp) ->
+  vs ≠ Valid_closed ->
+  (vs = Valid_receiver_done \/ vs = Valid_sender_ready) ->
+  {{{ 
+    "value" ∷ ch ↦[(Channel chan_type) :: "v"] v ∗ 
+    "HCh" ∷ isUnbufferedChan ch γ chan_type v vs is_single_party send_count recv_count Psingle 
+      Pmulti Qsingle Qmulti R ∗ 
+    "chan_state" ∷ ch ↦[(Channel chan_type) :: "state"] #(valid_to_word vs) ∗
+    "HSndCtrAuth" ∷ own_send_counter_auth γ send_count (send_ctr_frozen vs) ∗ 
+    "Hsttok" ∷ exchange_token γ true v ∗
+    "HSndPerm" ∷ own_send_counter_frag γ i q
+  }}}
+  Channel__SenderCheckOfferResult chan_type #ch
+  {{{ (res: rescind_result), RET #(rescind_to_word res);
+    match vs, res with
+    | Valid_receiver_done, CompletedExchange =>
+      "value" ∷ ch ↦[(Channel chan_type) :: "v"] v ∗ 
+      "HCh" ∷ isUnbufferedChan ch γ chan_type v Valid_start is_single_party (S send_count) recv_count Psingle 
+        Pmulti Qsingle Qmulti R ∗ 
+      "chan_state" ∷ ch ↦[(Channel chan_type) :: "state"] #(valid_to_word Valid_start) ∗
+      "HSndCtrAuth" ∷ own_send_counter_auth γ (S send_count) false ∗ 
+      "HSndPerm" ∷ own_send_counter_frag γ (i + 1) q ∗
+      "HQ" ∷ Q is_single_party i Qsingle Qmulti
+      
+    | Valid_sender_ready, OfferRescinded =>
+      "value" ∷ ch ↦[(Channel chan_type) :: "v"] v ∗ 
+      "HCh" ∷ isUnbufferedChan ch γ chan_type v Valid_start is_single_party send_count recv_count Psingle 
+        Pmulti Qsingle Qmulti R ∗ 
+      "chan_state" ∷ ch ↦[(Channel chan_type) :: "state"] #(valid_to_word Valid_start) ∗
+      "HSndCtrAuth" ∷ own_send_counter_auth γ send_count false ∗ 
+      "HP" ∷  P is_single_party send_count v Psingle Pmulti ∗ 
+      "HSndPerm" ∷ own_send_counter_frag γ i q
+      
+    | _, _ =>
+      False
+    end
+  }}}.
+Proof.
+  intros Hbuffsz Hsp Hnot_closed Hvs.
+  iIntros (Φ) "Hpre HΦ".
+  iNamed "Hpre".
+  
+  wp_rec. wp_pures.
+  
+  (* Check if channel is closed *)
+  wp_apply (wp_loadField with "chan_state").
+  iIntros "chan_state".
+  wp_pures.
+    iDestruct (struct_field_pointsto_ty with "[$value]") as "%H".
+    {
+     simpl. done. 
+    }
+  
+  (* Cases based on vs ≠ Valid_closed *)
+  destruct vs.
+  
+  - (* Valid_start case: Not a valid state *)
+    destruct Hvs as [Hvs | Hvs]; discriminate.
+    
+  - (* Valid_receiver_ready case: Not a valid state *)
+    destruct Hvs as [Hvs | Hvs]; discriminate.
+    
+  - (* Valid_sender_ready case: Can rescind offer *)
+    destruct Hvs as [Hvs | Hvs]; try discriminate.
+    wp_auto.
+    unfold isUnbufferedChan.
+    iDestruct "HCh" as "[%Hfacts Hres]".
+    unfold chan_state_resources.
+    iDestruct "Hres" as "[Hgv HP]".
+    
+    (* Apply sender_transition_general *)
+    iMod (sender_transition_general ch γ chan_type v v Valid_sender_ready Valid_start 
+           sender_rescind_trans is_single_party send_count recv_count
+           Psingle Pmulti Qsingle Qmulti R Ri i q with 
+          "[HSndCtrAuth HSndPerm Hgv Hsttok HP]") as 
+          "IH".
+    { (* Prove valid transition *)
+      unfold is_valid_send_transition.
+      destruct Valid_sender_ready, Valid_start; try done.
+    }
+    { (* Ownership constraint *)
+      exact Hsp.
+    }
+    { (* Value type check *)
+      val_ty.
+    }
+    {
+      simpl.
+      iFrame. done.
+    }
+    
+    
+    (* Finalize *)
+    iModIntro.
+    iSpecialize ("HΦ" $! OfferRescinded).
+    
+    iApply "HΦ". iNamed "IH". simpl. iNamed "IH". 
+    iFrame. simpl. iNamed "HCh". iDestruct "IH" as "[H1 H2]".
+    replace (send_count + 0)%nat with send_count by lia.
+    replace (i + 0)%nat with i by lia.
+    iFrame.
+    
+  - (* Valid_receiver_done case: Can complete exchange *)
+    destruct Hvs as [Hvs | Hvs]; try discriminate.
+    wp_auto.
+    
+    (* Apply sender_transition_general *)
+    iMod (sender_transition_general ch γ chan_type v v  Valid_receiver_done Valid_start 
+           sender_complete_second_trans is_single_party send_count recv_count
+           Psingle Pmulti Qsingle Qmulti R Ri i q with 
+          "[HCh HSndCtrAuth HSndPerm Hsttok]") as 
+          "(HCh & HQ & HSndCtrAuth & HSndPerm)".
+    { (* Prove valid transition *)
+      unfold is_valid_send_transition.
+      destruct Valid_receiver_done, Valid_start; try done.
+    }
+    { (* Ownership constraint *)
+      exact Hsp.
+    }
+    { (* Value type check *)
+      val_ty.
+    }
+    { 
+      iFrame.
+      (* Need to supply HP if needed *)
+      destruct (sender_needs_P sender_complete_second_trans).
+      + simpl. unfold isUnbufferedChan. simpl. unfold chan_state_resources.
+      iDestruct "HCh" as "(%Hp & Hgv & HP)". iFrame. done.
+      + simpl. unfold isUnbufferedChan. simpl. unfold chan_state_resources.
+      iDestruct "HCh" as "(%Hp & Hgv & HP)". iFrame. done.
+    }
+    
+    (* Finalize *)
+    iModIntro.
+    iSpecialize ("HΦ" $! CompletedExchange).
+    iApply "HΦ". 
+    iNamed "HCh".
+    iFrame. simpl. iNamed "HCh". iDestruct "HSndPerm" as "(HnQ & H1 & H2)".
+    replace (send_count + 0)%nat with send_count by lia.
+    replace (send_count + 1)%nat with (S send_count) by lia.
+    replace (i + 0)%nat with i by lia.
+    iFrame. 
+    
+  - (* Valid_sender_done case: Not a valid state *)
+    destruct Hvs as [Hvs | Hvs]; discriminate.
+    
+  - (* Valid_closed case *)
+    exfalso.
+    apply Hnot_closed. reflexivity.
+Qed.
+
+Lemma wp_Channel__SenderCompleteOrOffer (ch: loc) (v vold: val) (γ: chan_names) (chan_type: ty) 
+  (buff: Slice.t) (vs: valid_chan_state) (send_count recv_count: nat) (size: nat) 
+  (is_single_party: bool) (Psingle: Z -> val -> iProp Σ) (Pmulti: val -> iProp Σ) 
+  (Qsingle: Z -> iProp Σ) (Qmulti: iProp Σ) (R Ri: nat -> iProp Σ) (i: nat) (q: Qp):
+  val_ty v chan_type ->
+  val_ty vold chan_type ->
+  (#buff.(Slice.sz) = #(W64 0)) ->
+  vs ≠ Valid_closed ->
+  (if is_single_party then q = 1%Qp else (q < 1)%Qp) ->
+  {{{ 
+    "value" ∷ ch ↦[(Channel chan_type) :: "v"] vold ∗ 
+    "HCh" ∷ isUnbufferedChan ch γ chan_type vold vs is_single_party send_count recv_count Psingle 
+      Pmulti Qsingle Qmulti R ∗ 
+    "chan_state" ∷ ch ↦[(Channel chan_type) :: "state"] #(valid_to_word vs) ∗
+    "HP" ∷ P is_single_party i v Psingle Pmulti ∗
+    "HSndCtrAuth" ∷ own_send_counter_auth γ send_count (send_ctr_frozen vs) ∗ 
+    "HSndPerm" ∷ own_send_counter_frag γ i q
+  }}}
+  Channel__SenderCompleteOrOffer chan_type #ch v
+  {{{ (res: sender_result), RET #(sender_result_to_word res);
+    match res, vs with
+    | SenderCompletedWithReceiver, Valid_receiver_ready =>
+      "value" ∷ ch ↦[(Channel chan_type) :: "v"] v ∗ 
+      "HCh" ∷ isUnbufferedChan ch γ chan_type v Valid_sender_done is_single_party (send_count + 1) recv_count Psingle 
+        Pmulti Qsingle Qmulti R ∗ 
+      "chan_state" ∷ ch ↦[(Channel chan_type) :: "state"] #(valid_to_word Valid_sender_done) ∗
+      "HSndCtrAuth" ∷ own_send_counter_auth γ (send_count + 1) false ∗ 
+      "HSndPerm" ∷ own_send_counter_frag γ (i + 1) q ∗
+      "HQ" ∷ Q is_single_party i Qsingle Qmulti
+      
+    | SenderMadeOffer, Valid_start =>
+      "value" ∷ ch ↦[(Channel chan_type) :: "v"] v ∗ 
+      "HCh" ∷ isUnbufferedChan ch γ chan_type v Valid_sender_ready is_single_party send_count recv_count Psingle 
+        Pmulti Qsingle Qmulti R ∗ 
+      "chan_state" ∷ ch ↦[(Channel chan_type) :: "state"] #(valid_to_word Valid_sender_ready) ∗
+      "HSndCtrAuth" ∷ own_send_counter_auth γ send_count false ∗ 
+      "HSndPerm" ∷ own_send_counter_frag γ i q ∗
+      "Hsttok" ∷ exchange_token γ true v
+      
+    | SenderCannotProceed, _ =>
+      "value" ∷ ch ↦[(Channel chan_type) :: "v"] vold ∗ 
+      "HCh" ∷ isUnbufferedChan ch γ chan_type vold vs is_single_party send_count recv_count Psingle 
+        Pmulti Qsingle Qmulti R ∗ 
+      "chan_state" ∷ ch ↦[(Channel chan_type) :: "state"] #(valid_to_word vs) ∗
+      "HP" ∷ P is_single_party i v Psingle Pmulti ∗
+      "HSndCtrAuth" ∷ own_send_counter_auth γ send_count (send_ctr_frozen vs) ∗ 
+      "HSndPerm" ∷ own_send_counter_frag γ i q
+      
+    | _, _ => False
+    end
+  }}}.
+Proof.
+  intros Hval_ty Hval_tynew Hbuffsz Hnot_closed Hsp.
+  iIntros (Φ) "Hpre HΦ".
+  iNamed "Hpre".
+  
+  wp_rec. wp_pures.
+  
+  (* Check if channel is closed *)
+  wp_apply (wp_loadField with "chan_state").
+  iIntros "chan_state".
+  wp_pures.
+  
+  (* Cases based on vs ≠ Valid_closed *)
+  destruct vs.
+  
+  - (* Valid_start case: Can make an offer *)
+    wp_auto.
+    (* Handle counter verification and update *)
+    iAssert (own_send_counter_auth γ send_count false ∗ 
+             own_send_counter_frag γ i q ∗ 
+             ⌜if is_single_party then send_count = i else i <= send_count⌝%I)%I
+      with "[HSndCtrAuth HSndPerm]" as "(HSndCtrAuth & HSndPerm & %Hispz)".
+    {
+      destruct is_single_party.
+      - subst q.
+        iDestruct (send_counter_elem with "[$HSndCtrAuth] [$HSndPerm]") as "%Hag2".
+        iFrame. iPureIntro. done.
+      - iDestruct (send_counter_lower with "[$HSndCtrAuth] [$HSndPerm]") as "%Hag2".
+        iFrame. iPureIntro. lia.
+    }
+    
+    (* Apply transition using the general lemma *)
+    iMod (sender_transition_general ch γ chan_type v v  Valid_start Valid_sender_ready 
+           sender_offer_trans is_single_party send_count recv_count
+           Psingle Pmulti Qsingle Qmulti R Ri i q with 
+          "[HCh HSndCtrAuth HSndPerm HP]") as 
+          "(HCh & Hsttok & _ & _ &  HSndCtrAuth & HSndPerm)".
+    { (* Prove valid transition *)
+      unfold is_valid_send_transition.
+      destruct Valid_start, Valid_sender_ready; try done.
+    }
+    { (* Ownership constraint *)
+      exact Hsp.
+    }
+    { (* Value type check *)
+      exact Hval_ty.
+    }
+    { 
+      simpl.
+      unfold isUnbufferedChan. unfold chan_state_resources.
+      iFrame.
+      unfold P.
+      destruct is_single_party.
+      {
+        subst. iFrame.
+        done.
+        }
+        (* Supply HP for this transition *)
+        iFrame.
+        done.
+    }
+    
+    (* Finalize *)
+    iModIntro.
+    iSpecialize ("HΦ" $! SenderMadeOffer).
+    iApply "HΦ". simpl.
+    replace (send_count + 0)%nat with send_count by lia.
+    replace (i + 0)%nat with i by lia.
+    iFrame.
+    iDestruct "Hsttok" as "[_ Hsttok]". iFrame. 
+    
+  - (* Valid_receiver_ready case: Can complete exchange *)
+    wp_auto.
+    iAssert (own_send_counter_auth γ send_count false ∗ 
+             own_send_counter_frag γ i q ∗ 
+             ⌜if is_single_party then send_count = i else i <= send_count⌝%I)%I
+      with "[HSndCtrAuth HSndPerm]" as "(HSndCtrAuth & HSndPerm & %Hispz)".
+    {
+      destruct is_single_party.
+      - subst q.
+        iDestruct (send_counter_elem with "[$HSndCtrAuth] [$HSndPerm]") as "%Hag2".
+        iFrame. iPureIntro. done.
+      - iDestruct (send_counter_lower with "[$HSndCtrAuth] [$HSndPerm]") as "%Hag2".
+        iFrame. iPureIntro. lia.
+    }
+    
+    (* Apply transition using the general lemma *)
+    unfold isUnbufferedChan. unfold chan_state_resources.
+    iMod (sender_transition_general ch γ chan_type v v Valid_receiver_ready Valid_sender_done 
+           sender_complete_trans is_single_party send_count recv_count
+           Psingle Pmulti Qsingle Qmulti R Ri i q with 
+          "[HCh HSndCtrAuth HSndPerm HP]") as 
+          "(HCh & _ & HQ & HSndCtrAuth & HSndPerm)".
+    { (* Prove valid transition *)
+      unfold is_valid_send_transition.
+      destruct Valid_receiver_ready, Valid_sender_done; try done.
+    }
+    { (* Ownership constraint *)
+      exact Hsp.
+    }
+    { (* Value type check *)
+    done.
+    }
+    { 
+      iFrame.
+      simpl.
+      unfold P.
+      destruct is_single_party.
+      {
+        subst. iFrame. done.
+
+      }
+      (* Supply HP for this transition *)
+      iFrame.
+     done. 
+    }
+    
+    (* Finalize *)
+    iModIntro.
+    iSpecialize ("HΦ" $! SenderCompletedWithReceiver).
+    iApply "HΦ". 
+    iFrame. done.
+    
+  - (* Valid_sender_ready case: Cannot proceed *)
+    wp_auto.
+    iSpecialize ("HΦ" $! SenderCannotProceed).
+    iApply "HΦ". 
+    iFrame. iModIntro. done.
+    
+  - (* Valid_receiver_done case: Cannot proceed *)
+    wp_auto.
+    iSpecialize ("HΦ" $! SenderCannotProceed).
+
+    iApply "HΦ". 
+    iFrame. iModIntro. done.
+    
+  - (* Valid_sender_done case: Cannot proceed *)
+    wp_auto.
+    iSpecialize ("HΦ" $! SenderCannotProceed).
+    iApply "HΦ". 
+    iFrame. iModIntro. done.
+    
+  - (* Valid_closed case *)
+    exfalso.
+    apply Hnot_closed. reflexivity.
+Qed.
+
+
+End proof.
