src/goose_lang/lib/channel/chan_spec_multi_sender.v
@@ -1,0 +1,1138 @@
+From Perennial.goose_lang Require Import prelude. 
+From Perennial.goose_lang Require Import notation typing.
+From Perennial.goose_lang Require Import proofmode wpc_proofmode array.
+From Perennial.program_proof Require Import proof_prelude.
+From Perennial.program_proof Require Import std_proof.
+From Perennial.goose_lang.automation Require Import extra_tactics.
+From Perennial.goose_lang.lib Require Import
+      persistent_readonly slice slice.typed_slice struct loop lock control map.typed_map time proph rand string typed_mem.
+
+From Perennial.goose_lang.lib.channel Require Import auth_set.
+From Perennial.goose_lang.lib.channel Require Import chan_use_ctr.
+From Perennial.goose_lang.lib.channel Require Import chan_spec_multi_base.
+From Goose.github_com.goose_lang.goose Require Import channel.
+From Perennial.goose_lang Require Import lang typing.
+
+
+Section proof.
+Context `{ffi_sem: ffi_semantics} `{!ffi_interp ffi}.
+Context `{hG: heapGS Σ, !ffi_semantics _ _, !ext_types _}. 
+Context `{!closePropTrackerG Σ, !inG Σ (authR (optionUR (prodR fracR natR)))}.
+Context `{!ghost_varG Σ (bool * val)}.
+
+Implicit Types (v:val).
+
+Notation "vs1 =?= vs2" := (valid_chan_state_eq vs1 vs2) (at level 70).
+    
+Lemma wp_Channel__TryReceive (ch: loc) (i: nat) (q: Qp) (γ: chan_names) (chan_type: ty) 
+(size: nat) (is_single_party: bool) (Psingle: (Z -> val -> iProp Σ)) (Pmulti: (val -> iProp Σ)) 
+(Qsingle: (Z -> iProp Σ)) (Qmulti: iProp Σ) (R Ri:nat -> iProp Σ) :
+(if is_single_party then q = 1%Qp else (q < 1)%Qp) ->
+{{{ 
+  "HCh" ∷ isChan ch γ chan_type size is_single_party Psingle Pmulti Qsingle Qmulti R ∗
+  "HQ" ∷ Q is_single_party i Qsingle Qmulti ∗ 
+  "HRecvPerm" ∷ own_recv_perm γ q i Ri 
+}}}
+Channel__TryReceive chan_type #ch
+{{{ (v: val) (ok: bool) (selected: bool), RET (#selected,v,#ok); 
+  if selected then 
+    (if ok then 
+      ((P is_single_party i v Psingle Pmulti ∗ own_recv_perm γ q (i + 1) Ri ∗ ⌜ok⌝ ∗ ⌜val_ty v chan_type⌝))
+    else
+      (own_recv_counter_frag γ i q ∗ ⌜v = (zero_val chan_type)⌝ ∗ ⌜ok = false⌝
+       ∗ ∃ n, (Ri n) ∗ own_send_counter_auth γ n true ∗ own_recv_counter_auth γ n true))
+  else 
+    (Q is_single_party i Qsingle Qmulti ∗ own_recv_perm γ q i Ri)
+}}}.
+Proof.
+  intros Hsp.
+  iIntros (Φ) "Hpre HΦ".
+  iNamed "Hpre".
+  
+  wp_rec. wp_pures.
+  
+  (* Decide if channel is buffered or unbuffered *)
+  iNamed "HCh".
+  wp_loadField.
+  wp_apply wp_slice_len.
+
+  wp_if_destruct.
+
+  
+  (* Case: Buffered channel (size > 0) *)
+  - 
+    assert (size > 0)%nat as Hsize_pos by word.
+    (* Handle buffered case based on count and channel state *)
+    assert ((size =? 0) = false) by lia.
+  
+  (* Call BufferedTryReceive *)
+    wp_rec.
+    wp_loadField.
+    wp_apply (wp_Mutex__Lock with "Hlock").
+    iIntros "[Hlocked HisChanInner]". wp_pures.
+    unfold isChanInner. iNamed "HisChanInner".
+   (* destruct (vs =?= Valid_closed) eqn: Hc.
+    {
+      assert (vs = Valid_closed).
+      { destruct vs. all: done. }
+      replace vs with Valid_closed.
+      subst vs. rewrite H. iNamed "HisChanInner".
+    } *)
+    
+    (* Extract inner channel details *)
+    iNamed "HisChanInner".
+    
+    (* Assert that size > 0 *)
+    rewrite H. iNamed "HisChanInner".
+    destruct (uint.Z (W64 0) <? uint.Z (W64 count)) eqn: Hb.
+    {
+    + (* Case: Buffered channel (size > 0) with data available *)
+      wp_apply (wp_Channel__BufferedTryReceiveLocked ch γ chan_type size mu_l is_single_party vs
+               count send_count recv_count first buff
+               Psingle Pmulti Qsingle Qmulti R Ri i q
+               with "[buff count chan_state HChanState first HRecvPerm HQ HRcvCtrAuth]").
+      *  done.
+      * done.
+      * rewrite Hb. iFrame. iFrame "#".
+      * iIntros (success). iIntros (v0). iIntros (has_value). iIntros "Hres".
+        wp_loadField. 
+       
+        wp_pures.
+        
+        (* Unlock mutex *)
+        destruct success eqn: Hqs, has_value eqn: Hqb.
+        { iNamed "Hres". iNamed "Hres".
+        wp_apply (wp_Mutex__Unlock with "[$Hlock HCh HRecvCtrAuth first count chan_state value HSndCtrAuth HCloseTokPostClose  $Hlocked]").
+        {
+            iModIntro.
+            unfold isChanInner. 
+            iExists vs, (count - 1)%nat, new_first, v, send_count, (S recv_count).
+            iFrame. replace (W64 (count - 1)%nat) with (W64 (count-1)) by word.
+            iFrame.    replace (Z.of_nat count - 1) with (Z.of_nat (count-1)) by word. iFrame.
+        }
+        {
+         wp_pures. iModIntro. iApply "HΦ". iFrame. replace (i + 1)%nat with (S i) by lia. iFrame. done.
+        }
+        }
+        {
+          iNamed "Hres".
+          iNamed "Hres". iDestruct "Hres" as "[%Hvs %Hvz]". subst vs.
+          iNamed "HCloseTokPostClose". iDestruct "HCloseTokPostClose" as "[Hct1 Hct2]".
+          iDestruct (own_valid_2 with "[$Hct2] [$HSc]") as "%Hvalid". 
+          apply auth_frag_op_valid_1 in Hvalid.
+          rewrite <- (Some_op (1%Qp, n) (1%Qp, recv_count)) in Hvalid.
+          rewrite Some_valid in Hvalid.
+          rewrite <- (pair_op 1%Qp 1%Qp n recv_count) in Hvalid.
+          rewrite pair_valid in Hvalid. destruct Hvalid as [Hqvalid _].
+          rewrite frac_op in Hqvalid.
+          assert (((1 + q)%Qp ≤ 1)%Qp) by done.
+          apply Qp.not_add_le_l in H0.
+          contradiction.
+        }
+        {
+          iNamed "Hres". 
+          iDestruct "Hres" as "(_ & %Hcontra & _ )". replace (W64 count) with (W64 0) in Hb by word.
+          word.
+        }
+        {
+          iNamed "Hres". iNamed "Hres". done.
+        }
+    }
+    {
+    + (* Case: Buffered channel (size = 0) with no data available *)
+      destruct (vs =?= Valid_closed) eqn: Hc.
+      {
+        assert (vs = Valid_closed). {
+          destruct vs. all: try done. 
+        }
+        subst vs.
+        unfold recv_ctr_frozen. simpl. 
+        (* TODO: use buffered lemma thing *)
+        assert ((send_count =? recv_count) = true) by admit.
+        rewrite H0. iDestruct "HSndCtrAuth" as "#HSndCtrAuth". 
+        iDestruct "HRcvCtrAuth" as "#HRcvCtrAuth".
+
+      wp_apply (wp_Channel__BufferedTryReceiveLocked ch γ chan_type size mu_l is_single_party Valid_closed
+               count send_count recv_count first buff
+               Psingle Pmulti Qsingle Qmulti R Ri i q
+               with "[buff count chan_state HChanState first HRecvPerm HCloseTokPostClose]").
+      *  done.
+      * done.
+      * rewrite Hb. unfold own_recv_perm. iFrame. iFrame "#". iNamed "HCloseTokPostClose". iFrame.
+      simpl. rewrite H0. iFrame "#".
+      iDestruct "HCloseTokPostClose" as "[Hctc HSen]".
+        iDestruct (send_counter_elem with "[$HSndCtrAuth] [$HSen]") as "%Hag2". subst n.
+        iFrame. iPureIntro. assert((W64 count) = (W64 0)) by word. 
+        Search "unsigned_inj".
+          assert (count + 1 < 2 ^ 63) by admit.
+          word.
+      * 
+        
+      iFrame.
+       iIntros (success). iIntros (v0). iIntros (has_value). iIntros "Hres".
+        wp_loadField. 
+        wp_pures.
+        destruct success eqn: Hqs, has_value eqn: Hqb.
+        {
+          iNamed "Hres". iNamed "Hres". unfold isBufferedChan. unfold isBufferedChanLogical.
+          iNamed "HCh". unfold buff_size_inv.
+          assert((W64 count) = (W64 0)) by word.
+          assert (count + 1 < 2 ^ 63) by admit.
+          assert (count = 0%nat) by word. 
+          subst count. iDestruct "HCh" as "[Hoss HRest]".
+       replace (0%nat - 1)%nat with (0%nat) by admit.
+          iDestruct "HRest" as "(%H3 & %H4 & H5)". word.
+          "[(Hoss & %Hsc & %Hsz & %Hl & %Hnf & %Hlx & %Hlxl & _)Hb]".
+          word.
+        wp_apply (wp_Mutex__Unlock with "[$Hlock HCh chan_state count value first HRecvCtrAuth HQ  $Hlocked]").
+        {
+            iModIntro.
+            unfold isChanInner. 
+            iExists vs, (count - 1)%nat, new_first, v, send_count, (S recv_count).
+            iFrame. replace (W64 (count - 1)%nat) with (W64 (count-1)) by word.
+            iFrame.    replace (Z.of_nat count - 1) with (Z.of_nat (count-1)) by word. iFrame.
+        }
+  
+      (* Call BufferedTryReceive *)
+        wp_loadField.
+        wp_apply (wp_Mutex__Lock with "Hlock").
+        iIntros "[Hlocked HisChanInner]". wp_pures.
+        unfold isChanInner. iNamed "HisChanInner".
+       (* destruct (vs =?= Valid_closed) eqn: Hc.
+        {
+          assert (vs = Valid_closed).
+          { destruct vs. all: done. }
+          replace vs with Valid_closed.
+          subst vs. rewrite H. iNamed "HisChanInner".
+        } *)
+        
+        (* Extract inner channel details *)
+        iNamed "HisChanInner".
+
+    }
+   
+        
+            
+          - (* Channel closed but tried to receive *)
+            iNamed "Hres".
+            iModIntro.
+            iExists vs, 0%nat, first, v, send_count, recv_count.
+            iFrame. rewrite H. iFrame. unfold recv_ctr_frozen. iFrame "#".
+            iExists recv_count, (close_tok_names ∖ {[γr]}).
+            iFrame "HScfroz HRcfroz HSc HCloseTokPostClose".
+            rewrite Hsize_zero. iFrame.
+            
+          - (* No data available but channel not closed *)
+            iDestruct "Hres" as "(Hchan_state & Hcount & Hfirst & HRcvPerm & HCh & %Hzero)".
+            iModIntro.
+            iExists vs, 0%nat, first, (zero_val chan_type), send_count, recv_count.
+            iFrame "Hchan_state Hcount Hfirst HCh HRcvCtrAuth HSndCtrAuth HCloseTokPostClose".
+            rewrite Hsize_zero. iFrame.
+            
+          - (* Impossible case *)
+            by iDestruct "Hres" as "%contra".
+        }
+        
+        wp_pures.
+        
+        (* Return appropriate results based on what happened *)
+        destruct success, has_value.
+        
+        -- (* Successful receive with value *)
+           iModIntro.
+           iApply ("HΦ" $! v true true).
+           iDestruct "Hres" as "(Hchan_state & %new_first & Hcount & Hfirst & HP & HRecvPerm & %HVt &
+                                HCh & HRecvCtrAuth)".
+           iFrame "HP HRecvPerm".
+           iPureIntro. split; done.
+        
+        -- (* Channel closed but tried to receive *)
+           iModIntro.
+           iApply ("HΦ" $! (zero_val chan_type) false true).
+           iDestruct "Hres" as "(Hchan_state & Hcount & Hfirst & HRi & #HScfroz & #HRcfroz & HSc & 
+                                %close_tok_names & %γr & HCloseTokPostClose & %Hzero)".
+           
+           (* Extract the recv_counter_frag from HRcvPerm *)
+           iNamed "HRcvPerm".
+           iDestruct "HRcvPerm" as "[HRecvFrag HTok]".
+           iFrame "HRecvFrag".
+           iSplitR; first done.
+           iSplitR; first done.
+           iExists recv_count.
+           iFrame "HRi HScfroz HRcfroz".
+        
+        -- (* No data available but channel not closed *)
+           iModIntro.
+           iApply ("HΦ" $! (zero_val chan_type) true false).
+           iDestruct "Hres" as "(Hchan_state & Hcount & Hfirst & HRcvPerm & HCh & %Hzero)".
+           iFrame "HQ HRcvPerm".
+        
+        -- (* Impossible case *)
+           iDestruct "Hres" as "%contra".
+           contradiction.
+
+Lemma wp_Channel__TryReceive (ch: loc) (i: nat) (q: Qp) (γ: chan_names) (chan_type: ty) 
+  (size: nat) (is_single_party: bool) (Psingle: (Z -> val -> iProp Σ)) (Pmulti: (val -> iProp Σ)) 
+  (Qsingle: (Z -> iProp Σ)) (Qmulti: iProp Σ) (R Ri: nat -> iProp Σ) :
+  (if is_single_party then q = 1%Qp else (q < 1)%Qp) ->
+  {{{ 
+    "HCh" ∷ isChan ch γ chan_type size is_single_party Psingle Pmulti Qsingle Qmulti R ∗
+    "HQ" ∷ Q is_single_party i Qsingle Qmulti ∗ 
+    "HRecvPerm" ∷ own_recv_perm γ q i Ri 
+  }}}
+  Channel__TryReceive chan_type #ch
+  {{{ (v: val) (ok: bool) (selected: bool), RET (#selected, v, #ok); 
+    if selected then 
+      (if ok then 
+        ((P is_single_party i v Psingle Pmulti ∗ own_recv_perm γ q (i + 1) Ri ∗ ⌜ok⌝ ∗ ⌜val_ty v chan_type⌝))
+      else
+        (own_recv_counter_frag γ i q ∗ ⌜v = (zero_val chan_type)⌝ ∗ ⌜ok = false⌝
+         ∗ ∃ n, (Ri n) ∗ own_send_counter_auth γ n true ∗ own_recv_counter_auth γ n true))
+    else 
+      (Q is_single_party i Qsingle Qmulti ∗ own_recv_perm γ q i Ri)
+  }}}.
+Proof.
+  intros Hsp.
+  iIntros (Φ) "Hpre HΦ".
+  iNamed "Hpre".
+  
+  wp_rec. wp_pures.
+  iNamed "HCh".
+  wp_loadField.
+  
+  (* Decide if channel is buffered or unbuffered *)
+  wp_apply wp_slice_len.
+  wp_if_destruct.
+  
+  (* Case: Buffered channel *)
+  - wp_rec. 
+    wp_pures.
+    
+    (* Lock channel *)
+    wp_loadField.
+    wp_apply (wp_Mutex__Lock with "Hlock").
+    iIntros "[Hlocked HisChanInner]".
+    
+    (* Extract inner channel details *)
+    iNamed "HisChanInner".
+    
+    (* Check if channel has data (count > 0) *)
+    wp_loadField.
+    wp_pures.
+    
+    destruct (decide (word.unsigned count > 0)).
+    + (* Case: Data available - successful receive *)
+      wp_if_destruct; first last; [contradiction|].
+      
+      (* Extract value and update channel state *)
+      wp_loadField.
+      wp_loadField.
+      wp_apply (wp_SliceGet with "[$HBuffUnbuff]"); first val_ty.
+      { destruct size; [done|]. iNamed "HBuffUnbuff". done. }
+      iIntros "HBuffUnbuff".
+      
+      wp_store.
+      wp_loadField.
+      wp_loadField.
+      wp_loadField.
+      wp_op.
+      wp_loadField.
+      wp_apply wp_slice_len.
+      wp_op.
+      wp_storeField.
+      
+      wp_loadField.
+      wp_op.
+      wp_storeField.
+      
+      (* Load value and return *)
+      wp_load.
+      wp_pures.
+      
+      (* Update state and release lock *)
+      iAssert (∃ v0, P is_single_party i v0 Psingle Pmulti ∗ ⌜val_ty v0 chan_type⌝)%I
+        with "[HBuffUnbuff]" as (v0) "[HP #Hvty]".
+      { destruct size; [done|].
+        iNamed "HBuffUnbuff".
+        unfold isBufferedChan.
+        iDestruct "HBuffUnbuff" as "[Hbuff HLogical]".
+        iDestruct "HLogical" as "(%Hcount & %Hsize & %Hfirst & HPs & HQs)".
+        iDestruct (array_cons with "HPs") as "[HP HPs']".
+        iExists _. iFrame. iPureIntro. done. }
+      
+      (* Unlock mutex *)
+      wp_loadField.
+      wp_apply (wp_Mutex__Unlock with "[$Hlock $Hlocked value chan_state count first HSndCtrAuth HRcvCtrAuth HCloseTokPostClose HBuffUnbuff]").
+      { iModIntro. iExists vs, (word.sub count (W64 1)), first, v0, send_count, (recv_count + 1).
+        iFrame. destruct vs; try iFrame "#"; done. }
+      
+      wp_pures.
+      iModIntro.
+      iApply ("HΦ" $! v0 true true).
+      iSplitL "HP".
+      * iFrame "HP". iSplitL "HRecvPerm".
+        -- replace (i + 1)%nat with (S i) by lia. iFrame.
+        -- iPureIntro. split; done.
+      * iFrame.
+      
+    + (* Case: No data available *)
+      wp_if_destruct; first [|contradiction].
+      
+      (* Check if channel is closed *)
+      wp_loadField.
+      wp_pures.
+      
+      destruct (decide (vs = Valid_closed)).
+      * (* Channel is closed *)
+        wp_if_destruct; first [|subst vs; contradiction].
+        wp_load.
+        wp_pures.
+        
+        (* Extract closed channel resources *)
+        iAssert (∃ n close_tok_names,
+          own_closed_tok_post_close γ n close_tok_names ∗
+          own_send_counter_frag γ n 1 ∗
+          own_send_counter_auth γ n true)%I
+          with "[HCloseTokPostClose]" as (n close_tok_names) "(Htok & Hsnd & #Hauth)".
+        { subst vs. iNamed "HCloseTokPostClose". iExists n, close_tok_names. iFrame. iFrame "#". }
+        
+        (* Release lock *)
+        wp_loadField.
+        wp_apply (wp_Mutex__Unlock with "[$Hlock $Hlocked value chan_state count first HSndCtrAuth HRcvCtrAuth HBuffUnbuff]").
+        { iModIntro. iExists Valid_closed, count, first, v, send_count, recv_count.
+          iFrame. iExists n, close_tok_names. iFrame. iFrame "#". }
+        
+        wp_pures.
+        iModIntro.
+        iApply ("HΦ" $! (zero_val chan_type) false true).
+        
+        (* Return resources for closed channel *)
+        iNamed "HRecvPerm".
+        iDestruct "HRecvPerm" as "[Hfrag Htok']".
+        iFrame "Hfrag".
+        iSplitL ""; first done.
+        iSplitL ""; first done.
+        iExists n. iFrame "Htok' Hauth".
+        
+        (* Need to derive recv_counter_auth for n *)
+        iAssert (own_recv_counter_auth γ n true)%I as "#Hrecv_auth".
+        { (* This would come from channel invariant when n = recv_count *) admit. }
+        
+        iFrame "Hrecv_auth".
+      
+      * (* Channel not closed but empty *)
+        wp_if_destruct; first [contradiction|].
+        wp_load.
+        wp_pures.
+        
+        (* Release lock *)
+        wp_loadField.
+        wp_apply (wp_Mutex__Unlock with "[$Hlock $Hlocked value chan_state count first HSndCtrAuth HRcvCtrAuth HCloseTokPostClose HBuffUnbuff]").
+        { iModIntro. iExists vs, count, first, v, send_count, recv_count.
+          iFrame. destruct vs; try iFrame "#"; done. }
+        
+        wp_pures.
+        iModIntro.
+        iApply ("HΦ" $! (zero_val chan_type) true false).
+        iFrame.
+  
+  (* Case: Unbuffered channel *)
+  - wp_apply wp_ref_of_zero; first done.
+    iIntros (local_val) "Hval".
+    wp_pures.
+    
+    (* Extract channel components *)
+    iNamed "HCh".
+    
+    (* Lock channel *)
+    wp_loadField.
+    wp_apply (wp_Mutex__Lock with "Hlock").
+    iIntros "[Hlocked HisChanInner]".
+    
+    (* Extract inner channel details *)
+    iNamed "HisChanInner".
+    
+    (* Assert size = 0 for unbuffered channel *)
+    assert (size = 0)%nat as Hsize0.
+    { destruct size; [done|]. simpl in Heqb. discriminate. }
+    rewrite Hsize0 in *.
+    
+    (* Apply ReceiverCompleteOrOffer *)
+    wp_pures.
+    wp_apply (wp_Channel__ReceiverCompleteOrOffer ch i q γ chan_type buff v send_count recv_count vs 0%nat is_single_party Psingle Pmulti Qsingle Qmulti R Ri
+              with "[chan_state value HQ HRecvPerm HRcvCtrAuth HBuffUnbuff]").
+    { exact Hsp. }
+    { rewrite Hsize0. simpl. done. }
+    { iFrame. rewrite Hsize0 in HBuffUnbuff. iFrame. }
+    
+    iIntros (res) "Hres".
+    wp_pures.
+    
+    (* Handle result from ReceiverCompleteOrOffer *)
+    wp_apply wp_ref_to; first val_ty.
+    iIntros (ok_ptr) "Hok".
+    
+    wp_pures.
+    wp_op.
+    
+    destruct res.
+    
+    + (* ReceiverCompletedWithSender *)
+      wp_if_destruct; first [|contradiction].
+      wp_apply wp_ref_to; first val_ty.
+      iIntros (selected_ptr) "Hselected".
+      wp_pures.
+      wp_op.
+      wp_op.
+      wp_if_destruct; first [|contradiction].
+      
+      (* Load value from channel *)
+      wp_loadField.
+      wp_store.
+      wp_pures.
+      
+      (* Unlock mutex *)
+      wp_loadField.
+      wp_apply (wp_Mutex__Unlock with "[$Hlock $Hlocked Hres]").
+      { iNamed "Hres". iModIntro. iExists Valid_receiver_done, count, first, v, send_count, (recv_count + 1).
+        iFrame. rewrite Hsize0. iFrame. }
+      
+      wp_pures.
+      wp_load.
+      wp_pures.
+      wp_load.
+      wp_load.
+      wp_pures.
+      
+      iModIntro.
+      iApply ("HΦ" $! v true true).
+      iNamed "Hres".
+      
+      iAssert (P is_single_party i v Psingle Pmulti)%I with "[HCh]" as "HP".
+      { unfold isUnbufferedChan in HCh.
+        iDestruct "HCh" as "[%HFacts HRes]".
+        destruct HFacts.
+        unfold chan_state_resources in HRes.
+        destruct is_single_party; simpl in *; iFrame. }
+      
+      iFrame "HP HRecvPerm".
+      iPureIntro. split; [done|].
+      destruct vs; try done.
+    
+    + (* ReceiverMadeOffer *)
+      wp_if_destruct; first [contradiction|].
+      wp_apply wp_ref_to; first val_ty.
+      iIntros (selected_ptr) "Hselected".
+      wp_pures.
+      wp_op.
+      wp_op.
+      wp_if_destruct; first [contradiction|].
+      
+      (* Unlock mutex *)
+      wp_loadField.
+      wp_apply (wp_Mutex__Unlock with "[$Hlock $Hlocked Hres]").
+      { iNamed "Hres". iModIntro. iExists Valid_receiver_ready, count, first, v, send_count, recv_count.
+        iFrame. rewrite Hsize0. iFrame. }
+      
+      wp_pures.
+      wp_if_destruct; first [|contradiction].
+      
+      (* Lock channel to check offer result *)
+      wp_loadField.
+      wp_apply (wp_Mutex__Lock with "Hlock").
+      iIntros "[Hlocked HisChanInner]".
+      
+      (* Apply ReceiverCompleteOrRescindOffer *)
+      wp_pures.
+      wp_apply (wp_Channel__ReceiverCompleteOrRescindOffer ch i q γ chan_type buff v send_count recv_count Valid_receiver_ready 0%nat is_single_party Psingle Pmulti Qsingle Qmulti R Ri
+                with "[chan_state value HisChanInner Hsttok]").
+      { exact Hsp. }
+      { rewrite Hsize0. simpl. done. }
+      { left. done. }
+      { iNamed "Hres".
+        iNamed "HisChanInner".
+        iFrame "chan_state value".
+        iAssert (isUnbufferedChan ch γ chan_type v Valid_receiver_ready is_single_party send_count recv_count
+                Psingle Pmulti Qsingle Qmulti R)%I with "[HCh]" as "HCh".
+        { iFrame. }
+        iFrame "HCh HRecvCtrAuth Hsttok HRecvPerm".
+        iSplitL ""; first done. }
+      
+      iIntros (offer_res) "Hoffer".
+      wp_pures.
+      
+      destruct offer_res.
+      
+      * (* OfferRescinded *)
+        wp_if_destruct; first [contradiction|].
+        
+        (* Unlock mutex *)
+        wp_loadField.
+        wp_apply (wp_Mutex__Unlock with "[$Hlock $Hlocked Hoffer]").
+        { iNamed "Hoffer". iModIntro. iExists Valid_start, count, first, v, send_count, recv_count.
+          iFrame. rewrite Hsize0. iFrame. }
+        
+        wp_pures.
+        wp_load.
+        wp_load.
+        wp_load.
+        wp_pures.
+        
+        iModIntro.
+        iApply ("HΦ" $! (zero_val chan_type) true false).
+        iNamed "Hoffer".
+        iFrame "HQ HRecvPerm".
+      
+      * (* CompletedExchange *)
+        wp_if_destruct; first [|contradiction].
+        
+        (* Load value from channel *)
+        wp_loadField.
+        wp_store.
+        wp_pures.
+        wp_store.
+        
+        (* Unlock mutex *)
+        wp_loadField.
+        wp_apply (wp_Mutex__Unlock with "[$Hlock $Hlocked Hoffer]").
+        { iNamed "Hoffer". iModIntro. iExists Valid_start, count, first, v, send_count, (recv_count + 1).
+          iFrame. rewrite Hsize0. iFrame. }
+        
+        wp_pures.
+        wp_load.
+        wp_load.
+        wp_load.
+        wp_pures.
+        
+        iModIntro.
+        iApply ("HΦ" $! v true true).
+        iNamed "Hoffer".
+        iFrame "HP HRecvPerm".
+        iPureIntro. split; done.
+      
+      * (* CloseInterruptedOffer - impossible case *)
+        iNamed "Hoffer".
+        done.
+    
+    + (* ReceiverObservedClosed *)
+      wp_if_destruct; first [contradiction|].
+      wp_apply wp_ref_to; first val_ty.
+      iIntros (selected_ptr) "Hselected".
+      wp_pures.
+      wp_op.
+      wp_op.
+      wp_if_destruct; first [|contradiction].
+      
+      (* Load zero value *)
+      wp_loadField.
+      wp_store.
+      wp_pures.
+      
+      (* Extract closed channel resources *)
+      iAssert (∃ n close_tok_names,
+        own_closed_tok_post_close γ n close_tok_names ∗
+        own_send_counter_frag γ n 1 ∗
+        own_send_counter_auth γ n true)%I
+        with "[HCloseTokPostClose]" as (n close_tok_names) "(Htok & Hsnd & #Hauth)".
+      { iNamed "HCloseTokPostClose". iExists n, close_tok_names. iFrame. iFrame "#". }
+      
+      (* Unlock mutex *)
+      wp_loadField.
+      wp_apply (wp_Mutex__Unlock with "[$Hlock $Hlocked chan_state]").
+      { iModIntro. iExists Valid_closed, count, first, v, send_count, recv_count.
+        iFrame "chan_state". iExists n, close_tok_names. iFrame "Htok Hsnd". iFrame "#". }
+      
+      wp_pures.
+      wp_if_destruct; first [contradiction|].
+      wp_load.
+      wp_load.
+      wp_load.
+      wp_pures.
+      
+      iModIntro.
+      iApply ("HΦ" $! (zero_val chan_type) false true).
+      
+      (* Return resources for closed channel *)
+      iNamed "HRecvPerm".
+      iDestruct "HRecvPerm" as "[Hfrag Htok']".
+      iFrame "Hfrag".
+      iSplitL ""; first done.
+      iSplitL ""; first done.
+      iExists n. iFrame "Htok' Hauth".
+      
+      (* Need to derive recv_counter_auth for n *)
+      iAssert (own_recv_counter_auth γ n true)%I as "#Hrecv_auth".
+      { (* This would come from channel invariant when n = recv_count *) admit. }
+      
+      iFrame "Hrecv_auth".
+    
+    + (* ReceiverCannotProceed *)
+      wp_if_destruct; first [contradiction|].
+      wp_apply wp_ref_to; first val_ty.
+      iIntros (selected_ptr) "Hselected".
+      wp_pures.
+      wp_op.
+      wp_op.
+      wp_if_destruct; first [contradiction|].
+      
+      (* Unlock mutex *)
+      wp_loadField.
+      wp_apply (wp_Mutex__Unlock with "[$Hlock $Hlocked Hres]").
+      { iNamed "Hres". iModIntro. iExists vs, count, first, v, send_count, recv_count.
+        iFrame. rewrite Hsize0. iFrame. }
+      
+      wp_pures.
+      wp_if_destruct; first [contradiction|].
+      wp_load.
+      wp_load.
+      wp_load.
+      wp_pures.
+      
+      iModIntro.
+      iApply ("HΦ" $! (zero_val chan_type) true false).
+      iNamed "Hres".
+      iFrame.
+Admitted.
+
+Lemma wp_Channel__TrySend (ch: loc) (i: nat) (v: val) (q: Qp) (γ: chan_names) (chan_type: ty) 
+(size: nat) (is_single_party: bool) (Psingle: (Z -> val -> iProp Σ)) (Pmulti: (val -> iProp Σ)) 
+(Qsingle: (Z -> iProp Σ)) (Qmulti: iProp Σ) (R:nat -> iProp Σ) :
+
+val_ty v chan_type -> 
+#ch ≠ #null ->
+(if is_single_party then q = 1%Qp else (q < 1)%Qp) ->
+size + 1 < 2 ^ 63 ->
+
+{{{ 
+  "HCh" ∷ isChan ch γ chan_type size is_single_party Psingle Pmulti Qsingle Qmulti R ∗
+  "HP" ∷ P is_single_party i v Psingle Pmulti ∗ 
+  "HSc" ∷ own_send_counter_frag γ i q
+}}}
+Channel__TrySend chan_type #ch v
+{{{ (selected: bool), RET #selected; 
+  if selected then 
+    (Q is_single_party (i - size) Qsingle Qmulti ∗ own_send_counter_frag γ (i + 1)%nat q)
+  else 
+    (P is_single_party i v Psingle Pmulti ∗ own_send_counter_frag γ i q)
+}}}.
+Proof.
+  intros Hvt Hnn Hsp Hsgt64.
+  iIntros (Φ) "Hpre HΦ".
+  iNamed "Hpre".
+  iNamed "HCh".
+  
+  wp_rec. wp_pures.
+  wp_loadField. wp_pures.
+  wp_apply wp_slice_len.
+  wp_apply wp_ref_to; first val_ty.
+  iIntros (buffer_size_ptr) "Hbuffer_size".
+  wp_pures. wp_load.
+  
+  wp_if_destruct.
+  
+  - (* Case: Buffered channel (size > 0) *)
+    wp_loadField.
+    wp_apply (wp_Mutex__Lock with "Hlock").
+    iIntros "[Hlocked HisChanInner]". wp_pures.
+    
+    (* Extract the inner channel details *)
+    iDestruct "HisChanInner" as (vs count' first' v' send_count' recv_count') 
+      "(Hvalue & Hchan_state & Hcount & Hfirst & HSndCtrAuth' & HRecvCtrAuth & HCloseTokPostClose & HChanState)".
+    
+    (* Verify that the channel is not closed *)
+    iAssert (⌜ vs ≠ Valid_closed ⌝%I ) as "%Hnot_closed".
+    {
+     
+       destruct vs; try done.
+      (* Proof by contradiction - if closed, we get an ownership conflict *)
+      iDestruct "HCloseTokPostClose" as (n close_tok_names) "[HCloseTokPost HSendCtrFrag]".
+      iCombine "HSendCtrFrag" "HSc" as "H" gives "%Hvalid". 
+     apply auth_frag_op_valid_1 in Hvalid.
+               rewrite <- (Some_op (1%Qp, n) (q, i)) in Hvalid.
+               rewrite Some_valid in Hvalid.
+               rewrite <- (pair_op 1%Qp q n i) in Hvalid.
+               rewrite pair_valid in Hvalid. destruct Hvalid as [Hqvalid Hivalid].
+               rewrite frac_op in Hqvalid.
+
+               assert (((1 + q)%Qp ≤ 1)%Qp).
+               { 
+                done. 
+               }
+               apply Qp.not_add_le_l in H.
+               contradiction.
+    }
+    
+    (* Identify channel state as buffered *)
+    assert (size > 0)%nat as Hsize_pos by word.
+    assert ((size =? 0) = false) by lia.
+    rewrite H. iNamed "HChanState". unfold isBufferedChan.
+    iNamed "HChanState". iDestruct "HChanState" as "(Hoss & Hfax)".
+    unfold isBufferedChanLogical.
+    iDestruct "Hfax" as "(%Hct & %Hsz & %Hbs & HPs & HQs )".
+
+    wp_apply (wp_Channel__BufferedTrySend ch v  γ chan_type buff is_single_party q first' size count'
+                  vs send_count' recv_count' Psingle Pmulti Qsingle Qmulti R i with 
+                  "[HP HSc HSndCtrAuth' Hchan_state Hcount HPs HQs Hoss  Hfirst]").
+                  all: try done.
+        { inversion Hbuffsize. done. }
+        { word. }
+        { word.  }
+        { iFrame. iFrame "#".  unfold send_ctr_frozen. 
+        destruct vs. all: try (iFrame;iPureIntro;word).
+        exfalso. apply Hnot_closed. done.
+        }
+        iIntros (success) "IH". 
+        destruct success.
+        {
+          
+         iNamed "IH". wp_pures. wp_loadField.
+         wp_apply (wp_Mutex__Unlock with
+          "[$Hlock chan_state count first Hvalue HRecvCtrAuth HSndCtrAuth HCh $Hlocked]").
+        { iModIntro. unfold isChanInner. iExists vs, (S count'), first', v', (S send_count'), recv_count'. unfold send_ctr_frozen. rewrite H. iFrame. unfold recv_ctr_frozen.
+        destruct (vs =?= Valid_closed) eqn: H0.
+        {
+         assert (vs = Valid_closed).
+         { destruct vs. all: try done. }
+         subst vs. contradiction. 
+        }
+        destruct vs. all: try iFrame;done.
+        }
+        wp_pures.
+        iApply "HΦ". iModIntro.
+        replace (i + 1)%nat with (S i) by lia.
+        iFrame.
+        }
+        {
+          iNamed "IH".
+
+        iAssert (own_send_counter_auth γ send_count' false ∗ 
+                own_send_counter_frag γ i q ∗ 
+                ⌜if is_single_party then send_count' = i else i <= send_count'⌝%I)%I
+          with "[HSndCtrAuth HSen]" as "(HSndCtrAuth & HSen & %Hispz)".
+        {
+          destruct is_single_party.
+          - subst q.
+            iDestruct (send_counter_elem with "[$HSndCtrAuth] [$HSen]") as "%Hag2".
+            iFrame. iPureIntro. done.
+          - iDestruct (send_counter_lower with "[$HSndCtrAuth] [$HSen]") as "%Hag2".
+            iFrame. iPureIntro. lia.
+        }
+           
+          wp_pures. wp_loadField.
+         wp_apply (wp_Mutex__Unlock with
+          "[$Hlock chan_state count first Hvalue HRecvCtrAuth HSndCtrAuth HCh $Hlocked]").
+          { 
+            iModIntro. unfold isChanInner. iExists vs, (count'), first', v', (send_count'), recv_count'. unfold send_ctr_frozen. rewrite H. iFrame. unfold recv_ctr_frozen.
+        destruct (vs =?= Valid_closed) eqn: H0.
+        {
+        assert (vs = Valid_closed).
+        { destruct vs. all: try done. }
+        subst vs. contradiction. 
+       }
+       destruct vs. all: try iFrame;done.
+       }
+       wp_pures.
+       iApply "HΦ". iModIntro.
+       replace (i + 1)%nat with (S i) by lia.
+       iFrame.
+
+        }
+
+
+  - (* Case: Unbuffered channel (size = 0) *)
+    wp_loadField.
+    wp_apply (wp_Mutex__Lock with "Hlock").
+    iIntros "[Hlocked HisChanInner]". wp_pures.
+    
+    (* Extract the inner channel details *)
+    iDestruct "HisChanInner" as (vs count' first' v' send_count' recv_count') 
+      "(Hvalue & Hchan_state & Hcount & Hfirst & HSndCtrAuth' & HRecvCtrAuth & HCloseTokPostClose & HChanState)".
+    
+    (* Verify that the channel is not closed *)
+    iAssert (⌜ vs ≠ Valid_closed ⌝%I ) as "%Hnot_closed".
+    {
+     
+       destruct vs; try done.
+      (* Proof by contradiction - if closed, we get an ownership conflict *)
+      iDestruct "HCloseTokPostClose" as (n close_tok_names) "[HCloseTokPost HSendCtrFrag]".
+      iCombine "HSendCtrFrag" "HSc" as "H" gives "%Hvalid". 
+     apply auth_frag_op_valid_1 in Hvalid.
+               rewrite <- (Some_op (1%Qp, n) (q, i)) in Hvalid.
+               rewrite Some_valid in Hvalid.
+               rewrite <- (pair_op 1%Qp q n i) in Hvalid.
+               rewrite pair_valid in Hvalid. destruct Hvalid as [Hqvalid Hivalid].
+               rewrite frac_op in Hqvalid.
+
+               assert (((1 + q)%Qp ≤ 1)%Qp).
+               { 
+                done. 
+               }
+               apply Qp.not_add_le_l in H.
+               contradiction.
+    }
+    
+    (* Identify channel is unbuffered *)
+    assert ((size =? 0) = true).
+    {
+      word.
+    }
+    assert (size = 0)%nat as Hsize_zero.
+    {
+      word.
+    }
+    destruct (decide (size = 0%nat)); last by (exfalso; lia).
+    
+    (* Apply SenderCompleteOrOffer *)
+    iDestruct "HChanState" as "HUnbuffCh".
+    
+    wp_pures.
+    iDestruct (struct_field_pointsto_ty with "[$Hvalue]") as "%Hvty".
+    {
+     simpl. done. 
+    }
+    wp_apply (wp_Channel__SenderCompleteOrOffer ch v v' γ chan_type buff vs
+              send_count' recv_count' 0%nat is_single_party Psingle Pmulti
+              Qsingle Qmulti R _ i q with "[Hvalue HUnbuffCh Hchan_state HP HSndCtrAuth' HSc]").
+              all: (try done;try word; try lia; try iFrame).
+    { replace ((W64 0)) with ((W64 0%nat)) by word.  inversion Hbuffsize.
+    subst size. inversion H1. done.
+    }
+    { rewrite H.  (* Frame resources *) iFrame. }
+    
+    iIntros (res) "Hres".
+    
+    
+    (* Release mutex *)
+    wp_loadField.
+    
+    (* Branch based on sender result *)
+    destruct res, vs.
+    
+    + (* SenderCompletedWithReceiver, Valid_start - impossible combination *)
+      done.
+    
+    + (* SenderCompletedWithReceiver, Valid_receiver_ready *)
+      iNamed "Hres".
+      
+      (* Release mutex *)
+      wp_apply (wp_Mutex__Unlock with "[$Hlock value chan_state Hcount HSndCtrAuth HRecvCtrAuth 
+       HCloseTokPostClose HCh $Hlocked]").
+      {
+        iModIntro. unfold isChanInner. 
+        iExists Valid_sender_done, count', first', v, (S send_count'), recv_count'.
+        iFrame. rewrite H. iFrame. replace (send_count' + 1)%nat with (S send_count') by lia.
+        iFrame.
+      }
+      
+      (* Return success *)
+      wp_pures. iModIntro. 
+      
+      iApply "HΦ". simpl. iFrame. subst size. replace (i - 0%nat) with (Z.of_nat i) by lia.
+      iFrame.
+
+    (* More cases - will be admitted for brevity *)
+    + done.
+    + done.
+    + done.
+    + done.
+    
+    (* SenderMadeOffer, Valid_start - check offer result *)
+    + iDestruct "Hres" as "(Hvalue & HCh & Hchan_state & HSndCtrAuth' & HSen & Hsttok)".
+      
+      (* Release mutex *)
+      wp_apply (wp_Mutex__Unlock with "[$Hlock Hvalue Hcount Hchan_state HSndCtrAuth' HRecvCtrAuth 
+       HCloseTokPostClose HCh $Hlocked]").
+      {
+        iModIntro.
+        iExists Valid_sender_ready, count', first', v, send_count', recv_count'.
+        iFrame. rewrite H. iFrame.
+      }
+      
+      (* Check offer result *)
+      wp_pures. wp_loadField.
+      wp_apply (wp_Mutex__Lock with "Hlock"). 
+      iIntros "[locked inv]". wp_pures.
+
+      unfold isChanInner.
+      iNamed "inv". rewrite H. iDestruct "inv" as "[Hemp inv]". iNamed "inv".
+      destruct (decide (vs =?= Valid_closed)) as [Heq|Hneq].
+{
+  replace vs with Valid_closed.
+  {
+   iNamed "HCloseTokPostClose". iDestruct "HCloseTokPostClose" as "[Hct1 Hct2]".
+   iDestruct (own_valid_2 with "[$Hct2] [$HSen]") as "%Hvalid". 
+   apply auth_frag_op_valid_1 in Hvalid.
+  rewrite <- (Some_op (1%Qp, n) (q, i)) in Hvalid.
+  rewrite Some_valid in Hvalid.
+  rewrite <- (pair_op 1%Qp q n i) in Hvalid.
+  rewrite pair_valid in Hvalid. destruct Hvalid as [Hqvalid _].
+  rewrite frac_op in Hqvalid.
+  assert (((1 + q)%Qp ≤ 1)%Qp) by done.
+  apply Qp.not_add_le_l in H0.
+  contradiction.
+  }
+  {
+    destruct vs. all: done.
+  }
+}
+      
+      iDestruct (( sender_token_state_agree γ ch v vs send_count recv_count v0 chan_type
+      is_single_party Psingle Pmulti Qsingle Qmulti R ) with " [Hsttok] [HChanState]") as "%Hct".
+      {
+         destruct vs. all: done.
+      }
+      {
+       iFrame. 
+      }
+      {
+       iFrame. 
+      }
+      destruct Hct as [Hvsr Hvv0].
+      
+      
+      unfold isUnbufferedChan. unfold chan_state_resources.
+        iAssert (own_send_counter_auth γ send_count (send_ctr_frozen vs) ∗ 
+                own_send_counter_frag γ i q ∗ 
+                ⌜if is_single_party then send_count = i else i <= send_count⌝%I)%I
+          with "[HSndCtrAuth HSen]" as "(HSndCtrAuth & HSen & %Hispz)".
+        {
+          destruct is_single_party.
+          - subst q.
+            iDestruct (send_counter_elem with "[$HSndCtrAuth] [$HSen]") as "%Hag2".
+            iFrame. iPureIntro. lia.  
+          - iDestruct (send_counter_lower with "[$HSndCtrAuth] [$HSen]") as "%Hag2".
+            iFrame. iPureIntro. lia. 
+        }
+      
+      wp_apply (wp_Channel__SenderCheckOfferResult ch v  γ chan_type buff 
+              send_count recv_count vs 0%nat is_single_party Psingle Pmulti
+              Qsingle Qmulti R _ i q with "[ HCloseTokPostClose HSndCtrAuth HChanState chan_state value Hsttok HSen]").
+              all: (try done;try word; try lia; try iFrame).
+    { replace ((W64 0)) with ((W64 0%nat)) by word.  inversion Hbuffsize.
+    subst size. inversion H1. done.
+    }
+    { 
+      destruct vs. all: done.
+    }
+    {
+      inversion Hvsr.
+      {
+       right. done. 
+      }
+      left. done.
+    }
+    {
+    replace v0 with v by done. iFrame. 
+      
+    }
+    iIntros (res) "Hvs". destruct res.
+    {
+     simpl. wp_loadField.  
+     destruct vs. all: try done. iNamed "Hvs".
+     wp_apply (wp_Mutex__Unlock with "[$Hlock HRcvCtrAuth count  HSndCtrAuth value chan_state 
+        HCh $locked]").
+      {
+        iModIntro. iExists Valid_start. iFrame. iExists (W64 0). done.
+      }
+      wp_pures. iModIntro. iApply "HΦ". iFrame.
+      unfold P. destruct is_single_party.
+      {
+        subst send_count.
+       iFrame. 
+      }
+      unfold P. done.
+     
+    }
+    {
+      simpl. wp_loadField.  
+      destruct vs. all: try done. iNamed "Hvs".
+      wp_apply (wp_Mutex__Unlock with "[$Hlock HRcvCtrAuth count  HSndCtrAuth value chan_state 
+         HCh $locked]").
+       {
+         iModIntro. iExists Valid_start. iFrame. iExists (W64 0). done.
+       }
+       wp_pures. iModIntro. iApply "HΦ". iFrame.
+       unfold P. destruct is_single_party.
+       {
+         subst send_count.
+        iFrame. subst size. replace (i - 0%nat) with (Z.of_nat i) by lia. done.
+       }
+        iFrame. subst size. replace (i - 0%nat) with (Z.of_nat i) by lia. done.
+
+    }
+    {
+     wp_pures.  
+     simpl. wp_loadField.  
+      destruct vs. all: try done. 
+    }
+    + done.
+    + done.
+    + done.
+    + done.
+    + done.
+    (* what are these last 2 cases *)
+    + iNamed "Hres".
+    
+    wp_apply (wp_Mutex__Unlock with "[$Hlock HRecvCtrAuth Hcount Hfirst  HSndCtrAuth value chan_state 
+    HCh $Hlocked]").
+  {
+    iModIntro. iFrame. rewrite H. iFrame. done.  
+  }
+  {
+   wp_pures. iModIntro. iApply "HΦ". iFrame. 
+  }
+    + iNamed "Hres".
+    
+    wp_apply (wp_Mutex__Unlock with "[$Hlock HRecvCtrAuth Hcount Hfirst  HSndCtrAuth value chan_state 
+    HCh $Hlocked]").
+  {
+    iModIntro. iFrame. rewrite H. iFrame. done.  
+  }
+  {
+   wp_pures. iModIntro. iApply "HΦ". iFrame. 
+  }
+  + iNamed "Hres".
+    
+  wp_apply (wp_Mutex__Unlock with "[$Hlock HRecvCtrAuth Hcount Hfirst  HSndCtrAuth value chan_state 
+  HCh $Hlocked]").
+{
+  iModIntro. iFrame. rewrite H. iFrame. done.  
+}
+{
+ wp_pures. iModIntro. iApply "HΦ". iFrame. 
+}
+  + iNamed "Hres".
+  
+  wp_apply (wp_Mutex__Unlock with "[$Hlock HRecvCtrAuth Hcount Hfirst  HSndCtrAuth value chan_state 
+  HCh $Hlocked]").
+{
+  iModIntro. iFrame. rewrite H. iFrame. done.  
+}
+{
+ wp_pures. iModIntro. iApply "HΦ". iFrame. 
+}
++ iNamed "Hres".
+    
+wp_apply (wp_Mutex__Unlock with "[$Hlock HRecvCtrAuth Hcount Hfirst  HSndCtrAuth value chan_state 
+HCh $Hlocked]").
+{
+iModIntro. iFrame. rewrite H. iFrame. done.  
+}
+{
+wp_pures. iModIntro. iApply "HΦ". iFrame. 
+}
++ iNamed "Hres".
+
+wp_apply (wp_Mutex__Unlock with "[$Hlock HRecvCtrAuth Hcount Hfirst  HSndCtrAuth value chan_state 
+HCh $Hlocked]").
+{
+iModIntro. iFrame. rewrite H. iFrame. done.  
+}
+{
+wp_pures. iModIntro. iApply "HΦ". iFrame. 
+}
+Unshelve.
+{ done. } { done. } 
+Qed.
+
+End proof.
